Added ctr+orset

typeclass/Json1.fst
@@ -3,767 +3,843 @@ module Json1
 open FStar.Seq
 module M = Dependent_map
 module S = Set_extended
-open Library
+module L = Library
 
 type kt : eqtype =
   |Alpha_t : string -> kt
   |Beta_t : string -> kt
 
-type log = seq (pos & (nat & eqtype))
-
-class json (st_a st_b:Type0) (app_op_a app_op_b:eqtype) = {   
-  init_st_a : st_a;
-  init_st_b : st_b;
+class json (sta stb:Type0) (app_opa app_opb:eqtype) = {   
+  init_sta : sta;
+  init_stb : stb;
   
-  eq_a : st_a -> st_a -> Type0;
-  eq_b : st_b -> st_b -> Type0;
-
-  lem_eq_a : a:st_a -> b:st_a ->
-    Lemma (ensures eq_a a b <==> a == b);
-          //[SMTPat (eq_a a b)];
-
-  lem_eq_b : a:st_b -> b:st_b ->
-    Lemma (ensures eq_b a b <==> a == b);
-          //[SMTPat (eq_b a b)];
-          
-  rc_a : (pos & (nat & app_op_a)) -> (pos & (nat & app_op_a)) -> rc_res;
-  rc_b : (pos & (nat & app_op_b)) -> (pos & (nat & app_op_b)) -> rc_res;
+  eqa : sta -> sta -> Type0;
+  eqb : stb -> stb -> Type0;
   
-  do_a : st_a -> (pos & (nat & app_op_a)) -> st_a;
-  do_b : st_b -> (pos & (nat & app_op_b)) -> st_b;
+  rca : (pos & (nat & app_opa)) -> (pos & (nat & app_opa)) -> L.rc_res;
+  rcb : (pos & (nat & app_opb)) -> (pos & (nat & app_opb)) -> L.rc_res;
   
-  merge_a : st_a -> st_a -> st_a -> st_a;
-  merge_b : st_b -> st_b -> st_b -> st_b
+  doa : sta -> (pos & (nat & app_opa)) -> sta;
+  dob : stb -> (pos & (nat & app_opb)) -> stb;
+  
+  mergea : sta -> sta -> sta -> sta;
+  mergeb : stb -> stb -> stb -> stb;
+
+  lem_eqa : a:sta -> b:sta ->
+    Lemma (ensures eqa a b <==> a == b);
+
+  lem_eqb : a:stb -> b:stb ->
+    Lemma (ensures eqb a b <==> a == b);
 }
 
-val vt : #st_a:Type0 -> #st_b:Type0 -> #o_a:eqtype -> #o_b:eqtype -> {|json st_a st_b o_a o_b|} -> (c:kt) -> Type0
-let vt #st_a #st_b #o_a #o_b (c:kt) =
+val vt : #sta:Type0 -> #stb:Type0 -> #oa:eqtype -> #ob:eqtype -> #m:(json sta stb oa ob) -> (c:kt) -> Type0
+let vt #sta #stb #oa #ob #m (c:kt) =
   match c with
-  |Alpha_t _ -> st_a
-  |Beta_t _ -> st_b
+  |Alpha_t _ -> sta
+  |Beta_t _ -> stb
 
-type st #st_a #st_b #o_a #o_b #m = M.t kt (vt #st_a #st_b #o_a #o_b #m)
+type st #sta #stb #oa #ob #m = M.t kt (vt #sta #stb #oa #ob #m)
 
-val init_st_v : #st_a:Type0 -> #st_b:Type0 -> #o_a:eqtype -> #o_b:eqtype -> {|json st_a st_b o_a o_b|} -> k:kt -> vt #st_a #st_b #o_a #o_b k
-let init_st_v #st_a #st_b #o_a #o_b #m (k:kt) : vt k =
+val init_st_v : #sta:Type0 -> #stb:Type0 -> #oa:eqtype -> #ob:eqtype -> #m:(json sta stb oa ob) -> k:kt -> vt #sta #stb #oa #ob #m k
+let init_st_v #sta #stb #oa #ob #m (k:kt) : vt k =
   match k with
-  |Alpha_t _ -> m.init_st_a
-  |Beta_t _ -> m.init_st_b
+  |Alpha_t _ -> m.init_sta
+  |Beta_t _ -> m.init_stb
 
-val init_st : #st_a:Type0 -> #st_b:Type0 -> #o_a:eqtype -> #o_b:eqtype -> #m:(json st_a st_b o_a o_b) -> k:kt -> st #st_a #st_b #o_a #o_b #m
+val init_st : #sta:Type0 -> #stb:Type0 -> #oa:eqtype -> #ob:eqtype -> #m:(json sta stb oa ob) -> k:kt -> st #sta #stb #oa #ob #m
 let init_st (k:kt) : st = M.const_on S.empty (fun k -> init_st_v k)
 
-val sel : #st_a:Type0 -> #st_b:Type0 -> #o_a:eqtype -> #o_b:eqtype -> #m:(json st_a st_b o_a o_b) -> s:st #st_a #st_b #o_a #o_b #m -> k:kt -> vt #st_a #st_b #o_a #o_b k
-let sel #st_a #st_b #o_a #o_b #m (s:st) (k:kt) =
+val sel : #sta:Type0 -> #stb:Type0 -> #oa:eqtype -> #ob:eqtype -> #m:(json sta stb oa ob) -> 
+          s:st #sta #stb #oa #ob #m -> k:kt -> vt #sta #stb #oa #ob #m k
+let sel #sta #stb #oa #ob #m (s:st) (k:kt) =
   match k with
-  |Alpha_t _ -> if M.contains s k then M.sel s k else m.init_st_a
-  |Beta_t _ -> if M.contains s k then M.sel s k else m.init_st_b
+  |Alpha_t _ -> if M.contains s k then M.sel s k else m.init_sta
+  |Beta_t _ -> if M.contains s k then M.sel s k else m.init_stb
 
-val eq : #st_a:Type0 -> #st_b:Type0 -> #o_a:eqtype -> #o_b:eqtype -> #m:(json st_a st_b o_a o_b) -> a:st #st_a #st_b #o_a #o_b #m -> b:st #st_a #st_b #o_a #o_b #m -> Type0
-let eq #st_a #st_b #o_a #o_b #m (a b:st) =
-  //M.equal a b
-  //(forall k. M.contains a k = M.contains b k /\ sel a k == sel b k)
+val eq : #sta:Type0 -> #stb:Type0 -> #oa:eqtype -> #ob:eqtype -> #m:(json sta stb oa ob) -> 
+         a:st #sta #stb #oa #ob #m -> b:st #sta #stb #oa #ob #m -> Type0
+let eq #sta #stb #oa #ob #m (a b:st) =
   (forall k. M.contains a (Alpha_t k) = M.contains b (Alpha_t k) /\ 
         M.contains a (Beta_t k) = M.contains b (Beta_t k) /\
-        m.eq_a (sel a (Alpha_t k)) (sel b (Alpha_t k)) /\
-        m.eq_b (sel a (Beta_t k)) (sel b (Beta_t k)))
+        m.eqa (sel a (Alpha_t k)) (sel b (Alpha_t k)) /\
+        m.eqb (sel a (Beta_t k)) (sel b (Beta_t k)))
 
-type app_op_v (#app_op_a:eqtype) (#app_op_b:eqtype) : eqtype =
-  |Alpha_op : app_op_a -> app_op_v #app_op_a #app_op_b
-  |Beta_op : app_op_b -> app_op_v #app_op_a #app_op_b
+type app_op_v (#app_opa:eqtype) (#app_opb:eqtype) : eqtype =
+  |Alpha_op : app_opa -> app_op_v #app_opa #app_opb
+  |Beta_op : app_opb -> app_op_v #app_opa #app_opb
 
-type app_op (#o_a:eqtype) (#o_b:eqtype) : eqtype =
-  |Set : string (* key *) -> app_op_v #o_a #o_b(* value op *) -> app_op #o_a #o_b
+type app_op (#app_opa:eqtype) (#app_opb:eqtype) : eqtype =
+  |Set : string (* key *) -> app_op_v #app_opa #app_opb(* value op *) -> app_op #app_opa #app_opb
   
-type op (#o_a #o_b:eqtype) = pos (*timestamp*) & (nat (*replica ID*) & app_op #o_a #o_b)
-type op_a (#o_a:eqtype) = pos (*timestamp*) & (nat (*replica ID*) & o_a)
-type op_b (#o_b:eqtype) = pos (*timestamp*) & (nat (*replica ID*) & o_b)
+type jop (#app_opa #app_opb:eqtype) = pos (*timestamp*) & (nat (*replica ID*) & app_op #app_opa #app_opb)
 
-let distinct_ops (#o:eqtype) (op1 op2:(pos & (nat & o))) = fst op1 =!= fst op2
-
-//val get_rid : #o:eqtype -> pos -> nat -> o -> nat
-//let get_rid (_,(rid,_)) = rid
-
-let is_alpha_op (o:op) =
+let is_alpha_op (o:jop) =
   match snd (snd o) with
   |Set _ (Alpha_op _) -> true
   |_ -> false
 
-let is_beta_op (o:op) =
+let is_beta_op (o:jop) =
   match snd (snd o) with
   |Set _ (Beta_op _) -> true
   |_ -> false
 
 let get_key (_,(_,Set k _)) = k
 
-let get_op_a (o:op{is_alpha_op o}) : op_a =
+let get_opa #oa #ob (o:jop #oa #ob{is_alpha_op o}) : (pos & (nat & oa)) =
   match o with
   |ts, (rid, Set _ (Alpha_op op)) -> (ts,(rid,op))
 
-let get_op_b (o:op{is_beta_op o}) : op_b =
+let get_opb #oa #ob (o:jop #oa #ob{is_beta_op o}) : (pos & (nat & ob)) =
   match o with
   |ts, (rid, Set _ (Beta_op op)) -> (ts,(rid,op))
   
-val do : #st_a:Type0 -> #st_b:Type0 -> #o_a:eqtype -> #o_b:eqtype -> #m:(json st_a st_b o_a o_b) -> s:st #st_a #st_b #o_a #o_b #m -> o:op #o_a #o_b -> st #st_a #st_b #o_a #o_b #m
-
-let do #st_a #st_b #o_a #o_b #m (s:st) (o:op) 
+val do : #sta:Type0 -> #stb:Type0 -> #oa:eqtype -> #ob:eqtype -> #m:(json sta stb oa ob) -> 
+         s:st #sta #stb #oa #ob #m -> o:jop #oa #ob -> st #sta #stb #oa #ob #m         
+let do #sta #stb #oa #ob #m (s:st) (o:jop) 
   : (r:st{(is_alpha_op o ==> (forall k. M.contains r k <==> M.contains s k \/ k = Alpha_t (get_key o))) /\
                    (is_beta_op o ==> (forall k. M.contains r k <==> M.contains s k \/ k = Beta_t (get_key o)))}) =
   match snd (snd o) with
-  |Set k (Alpha_op _) -> let v = sel s (Alpha_t k) in M.upd s (Alpha_t k) (m.do_a v (get_op_a o))
-  |Set k (Beta_op _) -> let v = sel s (Beta_t k) in M.upd s (Beta_t k) (m.do_b v (get_op_b o))
+  |Set k (Alpha_op _) -> let v = sel s (Alpha_t k) in M.upd s (Alpha_t k) (m.doa v (get_opa o))
+  |Set k (Beta_op _) -> let v = sel s (Beta_t k) in M.upd s (Beta_t k) (m.dob v (get_opb o))
 
-val rc : #st_a:Type0 -> #st_b:Type0 -> #o_a:eqtype -> #o_b:eqtype -> #m:(json st_a st_b o_a o_b) -> o1:op #o_a #o_b -> o2:op #o_a #o_b -> rc_res
-let rc #st_a #st_b #o_a #o_b #m (o1 o2:op) : rc_res = 
+val rc : #sta:Type0 -> #stb:Type0 -> #oa:eqtype -> #ob:eqtype -> #m:(json sta stb oa ob) -> o1:jop #oa #ob -> o2:jop #oa #ob -> L.rc_res
+let rc #sta #stb #oa #ob #m (o1 o2:jop #oa #ob) : L.rc_res = 
   match snd (snd o1), snd (snd o2) with
-  |Set k1 (Alpha_op _), Set k2 (Alpha_op _) -> if k1 = k2 then m.rc_a (get_op_a o1) (get_op_a o2) else Either
-  |Set k1 (Beta_op _), Set k2 (Beta_op _) -> if k1 = k2 then m.rc_b (get_op_b o1) (get_op_b o2) else Either
-  |_ -> Either
+  |Set k1 (Alpha_op _), Set k2 (Alpha_op _) -> if k1 = k2 then m.rca (get_opa o1) (get_opa o2) else L.Either
+  |Set k1 (Beta_op _), Set k2 (Beta_op _) -> if k1 = k2 then m.rcb (get_opb o1) (get_opb o2) else L.Either
+  |_ -> L.Either
 
-val compose_values : #st_a:Type0 -> #st_b:Type0 -> #o_a:eqtype -> #o_b:eqtype -> #m:(json st_a st_b o_a o_b) -> k:kt -> l:st #st_a #st_b #o_a #o_b #m -> a:st #st_a #st_b #o_a #o_b #m -> b:st #st_a #st_b #o_a #o_b #m -> vt #st_a #st_b #o_a #o_b k
-let compose_values #st_a #st_b #o_a #o_b #m (k:kt) (l a b:st) : vt #st_a #st_b #o_a #o_b k =
+val compose_values : #sta:Type0 -> #stb:Type0 -> #oa:eqtype -> #ob:eqtype -> #m:(json sta stb oa ob) -> 
+                   k:kt -> l:st #sta #stb #oa #ob #m -> a:st #sta #stb #oa #ob #m -> b:st #sta #stb #oa #ob #m -> vt #sta #stb #oa #ob #m k
+let compose_values #sta #stb #oa #ob #m (k:kt) (l a b:st) : vt k =
   if Alpha_t? k then 
-    m.merge_a (sel l k) (sel a k) (sel b k)
-  else m.merge_b (sel l k) (sel a k) (sel b k)
+    m.mergea (sel l k) (sel a k) (sel b k)
+  else m.mergeb (sel l k) (sel a k) (sel b k)
 
-val merge : #st_a:Type0 -> #st_b:Type0 -> #o_a:eqtype -> #o_b:eqtype -> #m:(json st_a st_b o_a o_b) -> l:st #st_a #st_b #o_a #o_b #m -> a:st #st_a #st_b #o_a #o_b #m -> b:st #st_a #st_b #o_a #o_b #m -> st #st_a #st_b #o_a #o_b #m
-let merge #st_a #st_b #o_a #o_b #m (l a b:st) =
+val merge : #sta:Type0 -> #stb:Type0 -> #oa:eqtype -> #ob:eqtype -> #m:(json sta stb oa ob) -> 
+            l:st #sta #stb #oa #ob #m -> a:st #sta #stb #oa #ob #m -> b:st #sta #stb #oa #ob #m -> st #sta #stb #oa #ob #m
+let merge #sta #stb #oa #ob #m (l a b:st) =
   let keys = S.union (M.domain l) (S.union (M.domain a) (M.domain b)) in
-  let u = M.const_on keys (fun k -> init_st #st_a #st_b #o_a #o_b #m k) in
+  let u = M.const_on keys (fun k -> init_st #sta #stb #oa #ob #m k) in
   M.map (fun k _ -> compose_values k l a b) u
   
-val apply_log_a : #st_a:Type0 -> #st_b:Type0 -> #o_a:eqtype -> #o_b:eqtype -> {|json st_a st_b o_a o_b|} -> s:st_a -> l:seq (pos & (nat & o_a)) -> Tot st_a
-let rec apply_log_a #st_a #st_b #o_a #o_b #m (s:st_a) (l:seq (pos & (nat & o_a))) : Tot st_a (decreases length l) =
+val apply_log_a : #sta:Type0 -> #stb:Type0 -> #oa:eqtype -> #ob:eqtype -> #m:(json sta stb oa ob) -> 
+                  s:sta -> l:seq (pos & (nat & oa)) -> Tot sta
+let rec apply_log_a #sta #stb #oa #ob #m (s:sta) (l:seq (pos & (nat & oa))) : Tot sta (decreases length l) =
   match length l with
   |0 -> s
-  |_ -> apply_log_a #st_a #st_b #o_a #o_b #m (m.do_a s (head l)) (tail l) 
+  |_ -> apply_log_a #sta #stb #oa #ob #m (m.doa s (head l)) (tail l) 
 
-val apply_log_b : #st_a:Type0 -> #st_b:Type0 -> #o_a:eqtype -> #o_b:eqtype -> {|json st_a st_b o_a o_b|} -> s:st_b -> l:seq (pos & (nat & o_b)) -> Tot st_b
-let rec apply_log_b #st_a #st_b #o_a #o_b #m (s:st_b) (l:seq (pos & (nat & o_b))) : Tot st_b (decreases length l) =
+val apply_log_b : #sta:Type0 -> #stb:Type0 -> #oa:eqtype -> #ob:eqtype -> #m:(json sta stb oa ob) -> 
+                  s:stb -> l:seq (pos & (nat & ob)) -> Tot stb
+let rec apply_log_b #sta #stb #oa #ob #m (s:stb) (l:seq (pos & (nat & ob))) : Tot stb (decreases length l) =
   match length l with
   |0 -> s
-  |_ -> apply_log_b #st_a #st_b #o_a #o_b #m (m.do_b s (head l)) (tail l) 
+  |_ -> apply_log_b #sta #stb #oa #ob #m (m.dob s (head l)) (tail l) 
 
-val apply_log : #st_a:Type0 -> #st_b:Type0 -> #o_a:eqtype -> #o_b:eqtype -> #m:(json st_a st_b o_a o_b) -> s:st #st_a #st_b #o_a #o_b #m -> l:seq (op #o_a #o_b) -> Tot (st #st_a #st_b #o_a #o_b #m)
-
-let rec apply_log #st_a #st_b #o_a #o_b #m s l : Tot st (decreases length l) =
+val apply_log : #sta:Type0 -> #stb:Type0 -> #oa:eqtype -> #ob:eqtype -> #m:(json sta stb oa ob) -> 
+                s:st #sta #stb #oa #ob #m -> l:seq (jop #oa #ob) -> Tot (st #sta #stb #oa #ob #m)
+let rec apply_log #sta #stb #oa #ob #m s l : Tot st (decreases length l) =
   match length l with
   |0 -> s
   |_ -> apply_log (do s (head l)) (tail l) 
 
-class cond (st_a st_b:Type0) (o_a o_b:eqtype) (m:json st_a st_b o_a o_b) = {
-  rc_non_comm : o1:op -> o2:op ->
-    Lemma (requires distinct_ops o1 o2)
-          (ensures Either? (rc #st_a #st_b #o_a #o_b #m o1 o2) <==> (forall s. eq (do #st_a #st_b #o_a #o_b #m (do s o1) o2) (do (do s o2) o1)));
+class cond (sta stb:Type0) (oa ob:eqtype) (m:json sta stb oa ob) = {
+  rc_non_comm : o1:jop #oa #ob -> o2:jop #oa #ob ->
+    Lemma (requires L.distinct_ops o1 o2)
+          (ensures L.Either? (rc #sta #stb #oa #ob #m o1 o2) <==> (forall s. eq (do #sta #stb #oa #ob #m (do s o1) o2) (do (do s o2) o1)));
 
-  no_rc_chain : o1:op -> o2:op -> o3:op ->
-    Lemma (requires distinct_ops o1 o2 /\ distinct_ops o2 o3)
-          (ensures ~ (Fst_then_snd? (rc #st_a #st_b #o_a #o_b #m o1 o2) /\ Fst_then_snd? (rc #st_a #st_b #o_a #o_b #m o2 o3)));
+  no_rc_chain : o1:jop -> o2:jop -> o3:jop ->
+    Lemma (requires L.distinct_ops o1 o2 /\ L.distinct_ops o2 o3)
+          (ensures ~ (L.Fst_then_snd? (rc #sta #stb #oa #ob #m o1 o2) /\ L.Fst_then_snd? (rc #sta #stb #oa #ob #m o2 o3)));
 
-  cond_comm_base : s:st -> o1:op -> o2:op -> o3:op ->
-    Lemma (requires distinct_ops o1 o2 /\ distinct_ops o2 o3 /\ distinct_ops o1 o3 /\
-                    Fst_then_snd? (rc #st_a #st_b #o_a #o_b #m o1 o2) /\ ~ (Either? (rc #st_a #st_b #o_a #o_b #m o2 o3)))
-          (ensures eq (do (do (do s o1) o2) o3) (do (do #st_a #st_b #o_a #o_b #m (do s o2) o1) o3));
+  cond_comm_base : s:st -> o1:jop -> o2:jop -> o3:jop ->
+    Lemma (requires L.distinct_ops o1 o2 /\ L.distinct_ops o2 o3 /\ L.distinct_ops o1 o3 /\
+                    L.Fst_then_snd? (rc #sta #stb #oa #ob #m o1 o2) /\ ~ (L.Either? (rc #sta #stb #oa #ob #m o2 o3)))
+          (ensures eq (do (do (do s o1) o2) o3) (do (do #sta #stb #oa #ob #m (do s o2) o1) o3));
 
-  cond_comm_ind : s:st -> o1:op -> o2:op -> o3:op -> o:op -> l:seq op ->
-    Lemma (requires distinct_ops o1 o2 /\ distinct_ops o1 o3 /\ distinct_ops o2 o3 /\ 
-                    Fst_then_snd? (rc #st_a #st_b #o_a #o_b #m o1 o2) /\ ~ (Either? (rc #st_a #st_b #o_a #o_b #m o2 o3)) /\
+  cond_comm_ind : s:st -> o1:jop -> o2:jop -> o3:jop -> o:jop -> l:seq jop ->
+    Lemma (requires L.distinct_ops o1 o2 /\ L.distinct_ops o1 o3 /\ L.distinct_ops o2 o3 /\ 
+                    L.Fst_then_snd? (rc #sta #stb #oa #ob #m o1 o2) /\ ~ (L.Either? (rc #sta #stb #oa #ob #m o2 o3)) /\
                     eq (do (apply_log (do (do s o1) o2) l) o3) (do (apply_log (do (do s o2) o1) l) o3))
-          (ensures eq (do (do (apply_log (do (do s o1) o2) l) o) o3) (do (do #st_a #st_b #o_a #o_b #m (apply_log (do (do s o2) o1) l) o) o3))        
+          (ensures eq (do (do (apply_log (do (do s o1) o2) l) o) o3) (do (do #sta #stb #oa #ob #m (apply_log (do (do s o2) o1) l) o) o3))        
 }
 
-val testa : #st_a:Type0 -> #st_b:Type0 -> #o_a:eqtype -> #o_b:eqtype -> #m:(json st_a st_b o_a o_b) -> a:st_a -> b:st_a ->
-  Lemma (ensures (m.eq_a a b <==> a == b)) 
-        [SMTPat (m.eq_a a b)]
-let testa #st_a #st_b #o_a #o_b #m a b = 
-  m.lem_eq_a a b
+val lem_eq_a : #sta:Type0 -> #stb:Type0 -> #oa:eqtype -> #ob:eqtype -> #m:(json sta stb oa ob) -> a:sta -> b:sta ->
+  Lemma (ensures (m.eqa a b <==> a == b)) 
+        [SMTPat (m.eqa a b)]
+let lem_eq_a #sta #stb #oa #ob #m a b = 
+  m.lem_eqa a b
 
-val testb : #st_a:Type0 -> #st_b:Type0 -> #o_a:eqtype -> #o_b:eqtype -> #m:(json st_a st_b o_a o_b) -> a:st_b -> b:st_b ->
-  Lemma (ensures (m.eq_b a b <==> a == b)) 
-        [SMTPat (m.eq_b a b)]
-let testb #st_a #st_b #o_a #o_b #m a b = 
-  m.lem_eq_b a b
+val lem_eq_b : #sta:Type0 -> #stb:Type0 -> #oa:eqtype -> #ob:eqtype -> #m:(json sta stb oa ob) -> a:stb -> b:stb ->
+  Lemma (ensures (m.eqb a b <==> a == b)) 
+        [SMTPat (m.eqb a b)]
+let lem_eq_b #sta #stb #oa #ob #m a b = 
+  m.lem_eqb a b
 
 #set-options "--z3rlimit 300 --ifuel 3"
-class vc (st_a st_b:Type0) (o_a o_b:eqtype) (m:json st_a st_b o_a o_b) = {
- merge_comm_a : l:st_a -> a:st_a -> b:st_a ->
-  Lemma (ensures m.eq_a (m.merge_a l a b) (m.merge_a l b a));
-        //[SMTPat (m.merge_a l a b)];
+class vc (sta stb:Type0) (oa ob:eqtype) (m:json sta stb oa ob) = {
+ merge_comm_a : l:sta -> a:sta -> b:sta ->
+  Lemma (ensures m.eqa (m.mergea l a b) (m.mergea l b a));
 
- merge_comm_b : l:st_b -> a:st_b -> b:st_b ->
-  Lemma (ensures m.eq_b (m.merge_b l a b) (m.merge_b l b a));
-        //[SMTPat (m.merge_b l a b)]
+ merge_comm_b : l:stb -> a:stb -> b:stb ->
+  Lemma (ensures m.eqb (m.mergeb l a b) (m.mergeb l b a));
 
- merge_idem_a : s:st_a ->
-  Lemma (ensures m.eq_a (m.merge_a s s s) s);
-        //[SMTPat (m.merge_a l a b)];
+ merge_idem_a : s:sta ->
+  Lemma (ensures m.eqa (m.mergea s s s) s);
 
- merge_idem_b : s:st_b ->
-  Lemma (ensures m.eq_b (m.merge_b s s s) s);
-        //[SMTPat (m.merge_b l a b)]
+ merge_idem_b : s:stb ->
+  Lemma (ensures m.eqb (m.mergeb s s s) s);
 
- base_2op_a : o1:op_a -> o2:op_a ->
-  Lemma (requires (Fst_then_snd? (rc_a #st_a #st_b #o_a #o_b #m o2 o1) \/ Either? (rc_a #st_a #st_b #o_a #o_b #m o2 o1)) /\ get_rid o1 <> get_rid o2 /\ distinct_ops o1 o2)
-        (ensures m.eq_a (m.merge_a m.init_st_a (m.do_a m.init_st_a o1) (m.do_a m.init_st_a o2)) 
-                      (m.do_a (m.merge_a m.init_st_a m.init_st_a (m.do_a m.init_st_a o2)) o1));
+ base_2opa : o1:L.op #oa -> o2:L.op #oa ->
+  Lemma (requires (L.Fst_then_snd? (rca #sta #stb #oa #ob #m o2 o1) \/ L.Either? (rca #sta #stb #oa #ob #m o2 o1)) /\ 
+                   L.get_rid o1 <> L.get_rid o2 /\ L.distinct_ops o1 o2)
+        (ensures m.eqa (m.mergea m.init_sta (m.doa m.init_sta o1) (m.doa m.init_sta o2)) 
+                       (m.doa (m.mergea m.init_sta m.init_sta (m.doa m.init_sta o2)) o1));
 
- base_2op_b : o1:op_b -> o2:op_b ->
-  Lemma (requires (Fst_then_snd? (rc_b #st_a #st_b #o_a #o_b #m o2 o1) \/ Either? (rc_b #st_a #st_b #o_a #o_b #m o2 o1)) /\ get_rid o1 <> get_rid o2 /\ distinct_ops o1 o2)
-        (ensures m.eq_b (m.merge_b m.init_st_b (m.do_b m.init_st_b o1) (m.do_b m.init_st_b o2)) 
-                      (m.do_b (m.merge_b m.init_st_b m.init_st_b (m.do_b m.init_st_b o2)) o1));
+ base_2opb : o1:L.op #ob -> o2:L.op #ob ->
+  Lemma (requires (L.Fst_then_snd? (rcb #sta #stb #oa #ob #m o2 o1) \/ L.Either? (rcb #sta #stb #oa #ob #m o2 o1)) /\ 
+                   L.get_rid o1 <> L.get_rid o2 /\ L.distinct_ops o1 o2)
+        (ensures m.eqb (m.mergeb m.init_stb (m.dob m.init_stb o1) (m.dob m.init_stb o2)) 
+                       (m.dob (m.mergeb m.init_stb m.init_stb (m.dob m.init_stb o2)) o1));
 
- base_2op' : o1:op -> o2:op -> t:kt ->
-   Lemma (requires Either? (rc #st_a #st_b #o_a #o_b #m o2 o1) /\ get_rid o1 <> get_rid o2 /\ distinct_ops o1 o2 /\
-                    ~ (get_key o1 = get_key o2 /\ 
-                       is_alpha_op o1 /\ is_alpha_op o2 /\ (Fst_then_snd? (m.rc_a (get_op_a o2) (get_op_a o1)) || Either? (m.rc_a (get_op_a o2) (get_op_a o1))) /\
-                       is_beta_op o1 /\ is_beta_op o2 /\ (Fst_then_snd? (m.rc_b (get_op_b o2) (get_op_b o1)) || Either? (m.rc_b (get_op_b o2) (get_op_b o1)))))                
+ base_2op' : o1:jop -> o2:jop -> t:kt ->
+   Lemma (requires L.Either? (rc #sta #stb #oa #ob #m o2 o1) /\ L.get_rid o1 <> L.get_rid o2 /\ L.distinct_ops o1 o2 /\
+                   ~ (get_key o1 = get_key o2 /\ 
+                      is_alpha_op o1 /\ is_alpha_op o2 /\ (L.Fst_then_snd? (m.rca (get_opa o2) (get_opa o1)) || L.Either? (m.rca (get_opa o2) (get_opa o1))) /\
+                      is_beta_op o1 /\ is_beta_op o2 /\ (L.Fst_then_snd? (m.rcb (get_opb o2) (get_opb o1)) || L.Either? (m.rcb (get_opb o2) (get_opb o1)))))                
           (ensures eq (merge (init_st t) (do (init_st t) o1) (do (init_st t) o2)) 
-                      (do #st_a #st_b #o_a #o_b #m (merge (init_st t) (init_st t) (do (init_st t) o2)) o1));
+                      (do #sta #stb #oa #ob #m (merge (init_st t) (init_st t) (do (init_st t) o2)) o1));
 
- ind_lca_2op_a : l:st_a -> o1:op_a -> o2:op_a -> ol:op_a ->
-   Lemma (requires (Fst_then_snd? (rc_a #st_a #st_b #o_a #o_b #m o2 o1) \/ Either? (rc_a #st_a #st_b #o_a #o_b #m o2 o1)) /\ get_rid o1 <> get_rid o2 /\
-                    distinct_ops o1 o2 /\ distinct_ops o1 ol /\ distinct_ops o2 ol /\
-                    m.eq_a (m.merge_a l (m.do_a l o1) (m.do_a l o2)) (m.do_a (m.merge_a l l (m.do_a l o2)) o1))
-         (ensures m.eq_a (m.merge_a (m.do_a l ol) (m.do_a (m.do_a l ol) o1) (m.do_a (m.do_a l ol) o2)) (m.do_a (m.merge_a (m.do_a l ol) (m.do_a l ol) (m.do_a (m.do_a l ol) o2)) o1));
+ ind_lca_2opa : l:sta -> o1:L.op #oa -> o2:L.op #oa -> ol:L.op #oa ->
+   Lemma (requires (L.Fst_then_snd? (rca #sta #stb #oa #ob #m o2 o1) \/ L.Either? (rca #sta #stb #oa #ob #m o2 o1)) /\ 
+                    L.get_rid o1 <> L.get_rid o2 /\ L.distinct_ops o1 o2 /\ L.distinct_ops o1 ol /\ L.distinct_ops o2 ol /\
+                    m.eqa (m.mergea l (m.doa l o1) (m.doa l o2)) (m.doa (m.mergea l l (m.doa l o2)) o1))
+         (ensures m.eqa (m.mergea (m.doa l ol) (m.doa (m.doa l ol) o1) (m.doa (m.doa l ol) o2)) 
+                        (m.doa (m.mergea (m.doa l ol) (m.doa l ol) (m.doa (m.doa l ol) o2)) o1));
 
- ind_lca_2op_b : l:st_b -> o1:op_b -> o2:op_b -> ol:op_b ->
-   Lemma (requires (Fst_then_snd? (m.rc_b o2 o1) \/ Either? (m.rc_b o2 o1)) /\ get_rid o1 <> get_rid o2 /\
-                    distinct_ops o1 o2 /\ distinct_ops o1 ol /\ distinct_ops o2 ol /\
-                    m.eq_b (m.merge_b l (m.do_b l o1) (m.do_b l o2)) (m.do_b (m.merge_b l l (m.do_b l o2)) o1))
-         (ensures m.eq_b (m.merge_b (m.do_b l ol) (m.do_b (m.do_b l ol) o1) (m.do_b (m.do_b l ol) o2)) (m.do_b (m.merge_b (m.do_b l ol) (m.do_b l ol) (m.do_b (m.do_b l ol) o2)) o1));
+ ind_lca_2opb : l:stb -> o1:L.op #ob -> o2:L.op #ob -> ol:L.op #ob ->
+   Lemma (requires (L.Fst_then_snd? (m.rcb o2 o1) \/ L.Either? (m.rcb o2 o1)) /\ L.get_rid o1 <> L.get_rid o2 /\
+                    L.distinct_ops o1 o2 /\ L.distinct_ops o1 ol /\ L.distinct_ops o2 ol /\
+                    m.eqb (m.mergeb l (m.dob l o1) (m.dob l o2)) (m.dob (m.mergeb l l (m.dob l o2)) o1))
+         (ensures m.eqb (m.mergeb (m.dob l ol) (m.dob (m.dob l ol) o1) (m.dob (m.dob l ol) o2)) 
+                        (m.dob (m.mergeb (m.dob l ol) (m.dob l ol) (m.dob (m.dob l ol) o2)) o1));
 
- ind_lca_2op' : l:st -> o1:op -> o2:op -> ol:op ->
-   Lemma (requires Either? (rc #st_a #st_b #o_a #o_b #m o2 o1) /\ get_rid o1 <> get_rid o2 /\
-                    distinct_ops o1 o2 /\ distinct_ops o1 ol /\ distinct_ops o2 ol /\
-                    ~ (get_key o1 = get_key ol && get_key o2 = get_key ol /\
-                       is_alpha_op o1 /\ is_alpha_op o2 /\ is_alpha_op ol /\ (Fst_then_snd? (m.rc_a (get_op_a o2) (get_op_a o1)) || Either? (m.rc_a (get_op_a o2) (get_op_a o1))) /\
-                       is_beta_op o1 /\ is_beta_op o2 /\ is_beta_op ol /\ (Fst_then_snd? (m.rc_b (get_op_b o2) (get_op_b o1)) || Either? (m.rc_b (get_op_b o2) (get_op_b o1)))) /\
+ ind_lca_2op' : l:st -> o1:jop -> o2:jop -> ol:jop ->
+   Lemma (requires L.Either? (rc #sta #stb #oa #ob #m o2 o1) /\ L.get_rid o1 <> L.get_rid o2 /\
+                   L.distinct_ops o1 o2 /\ L.distinct_ops o1 ol /\ L.distinct_ops o2 ol /\
+                   ~ (get_key o1 = get_key ol && get_key o2 = get_key ol /\
+                      is_alpha_op o1 /\ is_alpha_op o2 /\ is_alpha_op ol /\ (L.Fst_then_snd? (m.rca (get_opa o2) (get_opa o1)) || L.Either? (m.rca (get_opa o2) (get_opa o1))) /\
+                      is_beta_op o1 /\ is_beta_op o2 /\ is_beta_op ol /\ (L.Fst_then_snd? (m.rcb (get_opb o2) (get_opb o1)) || L.Either? (m.rcb (get_opb o2) (get_opb o1)))) /\
                     eq (merge l (do l o1) (do l o2)) (do (merge l l (do l o2)) o1))
-          (ensures eq (merge (do #st_a #st_b #o_a #o_b #m l ol) (do (do l ol) o1) (do (do l ol) o2)) (do (merge (do l ol) (do l ol) (do (do l ol) o2)) o1));
+          (ensures eq (merge (do #sta #stb #oa #ob #m l ol) (do (do l ol) o1) (do (do l ol) o2)) 
+                      (do (merge (do l ol) (do l ol) (do (do l ol) o2)) o1));
 
- inter_right_base_2op_a : l:st_a -> a:st_a -> b:st_a -> o1:op_a -> o2:op_a -> ob:op_a -> ol:op_a ->
-   Lemma (requires (Fst_then_snd? (m.rc_a o2 o1) \/ Either? (m.rc_a o2 o1)) /\ get_rid o1 <> get_rid o2 /\ Fst_then_snd? (m.rc_a ob ol) /\ get_rid ob <> get_rid ol /\
-                    distinct_ops o1 o2 /\ distinct_ops o1 ob /\ distinct_ops o1 ol /\ distinct_ops o2 ob /\ distinct_ops o2 ol /\ distinct_ops ob ol /\
-                    m.eq_a (m.merge_a l (m.do_a a o1) (m.do_a b o2)) (m.do_a (m.merge_a l a (m.do_a b o2)) o1) /\ //from pre-cond of ind_right_2op
-                    m.eq_a (m.merge_a l (m.do_a a o1) (m.do_a (m.do_a b ob) o2)) (m.do_a (m.merge_a l a (m.do_a (m.do_a b ob) o2)) o1) /\ //from ind_right_2op
-                    m.eq_a (m.merge_a (m.do_a l ol) (m.do_a (m.do_a a ol) o1) (m.do_a (m.do_a b ol) o2)) (m.do_a (m.merge_a (m.do_a l ol) (m.do_a a ol) (m.do_a (m.do_a b ol) o2)) o1))
-         (ensures m.eq_a (m.merge_a (m.do_a l ol) (m.do_a (m.do_a a ol) o1) (m.do_a (m.do_a (m.do_a b ob) ol) o2)) (m.do_a (m.merge_a (m.do_a l ol) (m.do_a a ol) (m.do_a (m.do_a (m.do_a b ob) ol) o2)) o1));
+ inter_right_base_2opa : l:sta -> a:sta -> b:sta -> o1:L.op #oa -> o2:L.op #oa -> ob:L.op #oa -> ol:L.op #oa ->
+   Lemma (requires (L.Fst_then_snd? (m.rca o2 o1) \/ L.Either? (m.rca o2 o1)) /\ L.Fst_then_snd? (m.rca ob ol) /\ 
+                    L.get_rid o1 <> L.get_rid o2 /\ L.get_rid ob <> L.get_rid ol /\
+                    L.distinct_ops o1 o2 /\ L.distinct_ops o1 ob /\ L.distinct_ops o1 ol /\ L.distinct_ops o2 ob /\ L.distinct_ops o2 ol /\ L.distinct_ops ob ol /\
+                    m.eqa (m.mergea l (m.doa a o1) (m.doa b o2)) (m.doa (m.mergea l a (m.doa b o2)) o1) /\ //from pre-cond of ind_right_2op
+                    m.eqa (m.mergea l (m.doa a o1) (m.doa (m.doa b ob) o2)) (m.doa (m.mergea l a (m.doa (m.doa b ob) o2)) o1) /\ //from ind_right_2op
+                    m.eqa (m.mergea (m.doa l ol) (m.doa (m.doa a ol) o1) (m.doa (m.doa b ol) o2)) 
+                          (m.doa (m.mergea (m.doa l ol) (m.doa a ol) (m.doa (m.doa b ol) o2)) o1))
+         (ensures m.eqa (m.mergea (m.doa l ol) (m.doa (m.doa a ol) o1) (m.doa (m.doa (m.doa b ob) ol) o2)) 
+                        (m.doa (m.mergea (m.doa l ol) (m.doa a ol) (m.doa (m.doa (m.doa b ob) ol) o2)) o1));
 
- inter_right_base_2op_b : l:st_b -> a:st_b -> b:st_b -> o1:op_b -> o2:op_b -> ob:op_b -> ol:op_b ->
-   Lemma (requires (Fst_then_snd? (m.rc_b o2 o1) \/ Either? (m.rc_b o2 o1)) /\ get_rid o1 <> get_rid o2 /\ Fst_then_snd? (m.rc_b ob ol) /\ get_rid ob <> get_rid ol /\
-                    distinct_ops o1 o2 /\ distinct_ops o1 ob /\ distinct_ops o1 ol /\ distinct_ops o2 ob /\ distinct_ops o2 ol /\ distinct_ops ob ol /\
-                    m.eq_b (m.merge_b l (m.do_b a o1) (m.do_b b o2)) (m.do_b (m.merge_b l a (m.do_b b o2)) o1) /\ //from pre-cond of ind_right_2op
-                    m.eq_b (m.merge_b l (m.do_b a o1) (m.do_b (m.do_b b ob) o2)) (m.do_b (m.merge_b l a (m.do_b (m.do_b b ob) o2)) o1) /\ //from ind_right_2op
-                    m.eq_b (m.merge_b (m.do_b l ol) (m.do_b (m.do_b a ol) o1) (m.do_b (m.do_b b ol) o2)) (m.do_b (m.merge_b (m.do_b l ol) (m.do_b a ol) (m.do_b (m.do_b b ol) o2)) o1))
-         (ensures m.eq_b (m.merge_b (m.do_b l ol) (m.do_b (m.do_b a ol) o1) (m.do_b (m.do_b (m.do_b b ob) ol) o2)) (m.do_b (m.merge_b (m.do_b l ol) (m.do_b a ol) (m.do_b (m.do_b (m.do_b b ob) ol) o2)) o1));
+ inter_right_base_2opb : l:stb -> a:stb -> b:stb -> o1:L.op #ob -> o2:L.op #ob -> ob':L.op #ob -> ol:L.op #ob ->
+   Lemma (requires (L.Fst_then_snd? (m.rcb o2 o1) \/ L.Either? (m.rcb o2 o1)) /\ L.Fst_then_snd? (m.rcb ob' ol) /\ 
+                    L.get_rid o1 <> L.get_rid o2 /\ L.get_rid ob' <> L.get_rid ol /\
+                    L.distinct_ops o1 o2 /\ L.distinct_ops o1 ob' /\ L.distinct_ops o1 ol /\ L.distinct_ops o2 ob' /\ L.distinct_ops o2 ol /\ L.distinct_ops ob' ol /\
+                    m.eqb (m.mergeb l (m.dob a o1) (m.dob b o2)) (m.dob (m.mergeb l a (m.dob b o2)) o1) /\ //from pre-cond of ind_right_2op
+                    m.eqb (m.mergeb l (m.dob a o1) (m.dob (m.dob b ob') o2)) (m.dob (m.mergeb l a (m.dob (m.dob b ob') o2)) o1) /\ //from ind_right_2op
+                    m.eqb (m.mergeb (m.dob l ol) (m.dob (m.dob a ol) o1) (m.dob (m.dob b ol) o2)) 
+                          (m.dob (m.mergeb (m.dob l ol) (m.dob a ol) (m.dob (m.dob b ol) o2)) o1))
+         (ensures m.eqb (m.mergeb (m.dob l ol) (m.dob (m.dob a ol) o1) (m.dob (m.dob (m.dob b ob') ol) o2)) 
+                        (m.dob (m.mergeb (m.dob l ol) (m.dob a ol) (m.dob (m.dob (m.dob b ob') ol) o2)) o1));
           
- inter_right_base_2op' : l:st -> a:st -> b:st -> o1:op -> o2:op -> ob:op -> ol:op ->
-   Lemma (requires Either? (rc #st_a #st_b #o_a #o_b #m o2 o1) /\ get_rid o1 <> get_rid o2 /\ Fst_then_snd? (rc #st_a #st_b #o_a #o_b #m ob ol) /\ get_rid ob <> get_rid ol /\
-                    distinct_ops o1 o2 /\ distinct_ops o1 ob /\ distinct_ops o1 ol /\ distinct_ops o2 ob /\ distinct_ops o2 ol /\ distinct_ops ob ol /\
-                    ~ (get_key o1 = get_key ol && get_key o2 = get_key ol /\ get_key ob = get_key ol /\
-                       is_alpha_op o1 /\ is_alpha_op o2 /\ is_alpha_op ob /\ is_alpha_op ol /\ (Fst_then_snd? (m.rc_a (get_op_a o2) (get_op_a o1)) || Either? (m.rc_a (get_op_a o2) (get_op_a o1))) /\ Fst_then_snd? (m.rc_a (get_op_a ob) (get_op_a ol)) /\
-                       is_beta_op o1 /\ is_beta_op o2 /\ is_beta_op ob /\ is_beta_op ol /\ (Fst_then_snd? (m.rc_b (get_op_b o2) (get_op_b o1)) || Either? (m.rc_b (get_op_b o2) (get_op_b o1))) /\ Fst_then_snd? (m.rc_b (get_op_b ob) (get_op_b ol))) /\
+ inter_right_base_2op' : l:st -> a:st -> b:st -> o1:jop -> o2:jop -> ob':jop -> ol:jop ->
+   Lemma (requires L.Either? (rc #sta #stb #oa #ob #m o2 o1) /\ L.Fst_then_snd? (rc #sta #stb #oa #ob #m ob' ol) /\ 
+                   L.get_rid o1 <> L.get_rid o2 /\ L.get_rid ob' <> L.get_rid ol /\
+                   L.distinct_ops o1 o2 /\ L.distinct_ops o1 ob' /\ L.distinct_ops o1 ol /\ L.distinct_ops o2 ob' /\ L.distinct_ops o2 ol /\ L.distinct_ops ob' ol /\
+                   ~ (get_key o1 = get_key ol && get_key o2 = get_key ol /\ get_key ob' = get_key ol /\
+                      is_alpha_op o1 /\ is_alpha_op o2 /\ is_alpha_op ob' /\ is_alpha_op ol /\ (L.Fst_then_snd? (m.rca (get_opa o2) (get_opa o1)) || L.Either? (m.rca (get_opa o2) (get_opa o1))) /\ L.Fst_then_snd? (m.rca (get_opa ob') (get_opa ol)) /\
+                      is_beta_op o1 /\ is_beta_op o2 /\ is_beta_op ob' /\ is_beta_op ol /\ (L.Fst_then_snd? (m.rcb (get_opb o2) (get_opb o1)) || L.Either? (m.rcb (get_opb o2) (get_opb o1))) /\ L.Fst_then_snd? (m.rcb (get_opb ob') (get_opb ol))) /\
                     eq (merge l (do a o1) (do b o2)) (do (merge l a (do b o2)) o1) /\ //from pre-cond of ind_right_2op
-                    eq (merge l (do a o1) (do (do b ob) o2)) (do (merge l a (do (do b ob) o2)) o1) /\ //from ind_right_2op
+                    eq (merge l (do a o1) (do (do b ob') o2)) (do (merge l a (do (do b ob') o2)) o1) /\ //from ind_right_2op
                     eq (merge (do l ol) (do (do a ol) o1) (do (do b ol) o2)) (do (merge (do l ol) (do a ol) (do (do b ol) o2)) o1))
-         (ensures eq (merge (do l ol) (do (do a ol) o1) (do (do (do b ob) ol) o2)) (do (merge (do #st_a #st_b #o_a #o_b #m l ol) (do a ol) (do (do (do b ob) ol) o2)) o1));
+         (ensures eq (merge (do l ol) (do (do a ol) o1) (do (do (do b ob') ol) o2)) 
+                     (do (merge (do #sta #stb #oa #ob #m l ol) (do a ol) (do (do (do b ob') ol) o2)) o1));
 
-  inter_left_base_2op_a : l:st_a -> a:st_a -> b:st_a -> o1:op_a -> o2:op_a -> ob:op_a -> ol:op_a ->
-   Lemma (requires (Fst_then_snd? (m.rc_a o2 o1) \/ Either? (m.rc_a o2 o1)) /\ get_rid o1 <> get_rid o2 /\ Fst_then_snd? (m.rc_a ob ol) /\ get_rid ob <> get_rid ol /\
-                    distinct_ops o1 o2 /\ distinct_ops o1 ob /\ distinct_ops o1 ol /\ distinct_ops o2 ob /\ distinct_ops o2 ol /\ distinct_ops ob ol /\
-                    m.eq_a (m.merge_a (m.do_a l ol) (m.do_a (m.do_a a ol) o1) (m.do_a (m.do_a b ol) o2)) (m.do_a (m.merge_a (m.do_a l ol) (m.do_a a ol) (m.do_a (m.do_a b ol) o2)) o1))
-         (ensures m.eq_a (m.merge_a (m.do_a l ol) (m.do_a (m.do_a (m.do_a a ob) ol) o1) (m.do_a (m.do_a b ol) o2)) (m.do_a (m.merge_a (m.do_a l ol) (m.do_a (m.do_a a ob) ol) (m.do_a (m.do_a b ol) o2)) o1));
+  inter_left_base_2opa : l:sta -> a:sta -> b:sta -> o1:L.op #oa -> o2:L.op #oa -> ob:L.op #oa -> ol:L.op #oa ->
+   Lemma (requires (L.Fst_then_snd? (m.rca o2 o1) \/ L.Either? (m.rca o2 o1)) /\ L.Fst_then_snd? (m.rca ob ol) /\ 
+                    L.get_rid o1 <> L.get_rid o2 /\ L.get_rid ob <> L.get_rid ol /\
+                    L.distinct_ops o1 o2 /\ L.distinct_ops o1 ob /\ L.distinct_ops o1 ol /\ L.distinct_ops o2 ob /\ L.distinct_ops o2 ol /\ L.distinct_ops ob ol /\
+                    m.eqa (m.mergea (m.doa l ol) (m.doa (m.doa a ol) o1) (m.doa (m.doa b ol) o2)) 
+                          (m.doa (m.mergea (m.doa l ol) (m.doa a ol) (m.doa (m.doa b ol) o2)) o1))
+         (ensures m.eqa (m.mergea (m.doa l ol) (m.doa (m.doa (m.doa a ob) ol) o1) (m.doa (m.doa b ol) o2)) 
+                        (m.doa (m.mergea (m.doa l ol) (m.doa (m.doa a ob) ol) (m.doa (m.doa b ol) o2)) o1));
 
- inter_left_base_2op_b : l:st_b -> a:st_b -> b:st_b -> o1:op_b -> o2:op_b -> ob:op_b -> ol:op_b ->
-   Lemma (requires (Fst_then_snd? (m.rc_b o2 o1) \/ Either? (m.rc_b o2 o1)) /\ get_rid o1 <> get_rid o2 /\ Fst_then_snd? (m.rc_b ob ol) /\ get_rid ob <> get_rid ol /\
-                    distinct_ops o1 o2 /\ distinct_ops o1 ob /\ distinct_ops o1 ol /\ distinct_ops o2 ob /\ distinct_ops o2 ol /\ distinct_ops ob ol /\
-                    m.eq_b (m.merge_b (m.do_b l ol) (m.do_b (m.do_b a ol) o1) (m.do_b (m.do_b b ol) o2)) (m.do_b (m.merge_b (m.do_b l ol) (m.do_b a ol) (m.do_b (m.do_b b ol) o2)) o1))
-         (ensures m.eq_b (m.merge_b (m.do_b l ol) (m.do_b (m.do_b (m.do_b a ob) ol) o1) (m.do_b (m.do_b b ol) o2)) (m.do_b (m.merge_b (m.do_b l ol) (m.do_b (m.do_b a ob) ol) (m.do_b (m.do_b b ol) o2)) o1));
+ inter_left_base_2opb : l:stb -> a:stb -> b:stb -> o1:L.op #ob -> o2:L.op #ob -> ob':L.op #ob -> ol:L.op #ob ->
+   Lemma (requires (L.Fst_then_snd? (m.rcb o2 o1) \/ L.Either? (m.rcb o2 o1)) /\ L.Fst_then_snd? (m.rcb ob' ol) /\ 
+                    L.get_rid o1 <> L.get_rid o2 /\ L.get_rid ob' <> L.get_rid ol /\
+                    L.distinct_ops o1 o2 /\ L.distinct_ops o1 ob' /\ L.distinct_ops o1 ol /\ L.distinct_ops o2 ob' /\ L.distinct_ops o2 ol /\ L.distinct_ops ob' ol /\
+                    m.eqb (m.mergeb (m.dob l ol) (m.dob (m.dob a ol) o1) (m.dob (m.dob b ol) o2)) 
+                          (m.dob (m.mergeb (m.dob l ol) (m.dob a ol) (m.dob (m.dob b ol) o2)) o1))
+         (ensures m.eqb (m.mergeb (m.dob l ol) (m.dob (m.dob (m.dob a ob') ol) o1) (m.dob (m.dob b ol) o2)) 
+                        (m.dob (m.mergeb (m.dob l ol) (m.dob (m.dob a ob') ol) (m.dob (m.dob b ol) o2)) o1));
           
- inter_left_base_2op' : l:st -> a:st -> b:st -> o1:op -> o2:op -> ob:op -> ol:op ->
-   Lemma (requires Either? (rc #st_a #st_b #o_a #o_b #m o2 o1) /\ get_rid o1 <> get_rid o2 /\ Fst_then_snd? (rc #st_a #st_b #o_a #o_b #m ob ol) /\ get_rid ob <> get_rid ol /\
-                    distinct_ops o1 o2 /\ distinct_ops o1 ob /\ distinct_ops o1 ol /\ distinct_ops o2 ob /\ distinct_ops o2 ol /\ distinct_ops ob ol /\
-                    ~ (get_key o1 = get_key ol && get_key o2 = get_key ol /\ get_key ob = get_key ol /\
-                       is_alpha_op o1 /\ is_alpha_op o2 /\ is_alpha_op ob /\ is_alpha_op ol /\ (Fst_then_snd? (m.rc_a (get_op_a o2) (get_op_a o1)) || Either? (m.rc_a (get_op_a o2) (get_op_a o1))) /\ Fst_then_snd? (m.rc_a (get_op_a ob) (get_op_a ol)) /\
-                       is_beta_op o1 /\ is_beta_op o2 /\ is_beta_op ob /\ is_beta_op ol /\ (Fst_then_snd? (m.rc_b (get_op_b o2) (get_op_b o1)) || Either? (m.rc_b (get_op_b o2) (get_op_b o1))) /\ Fst_then_snd? (m.rc_b (get_op_b ob) (get_op_b ol))) /\
+ inter_left_base_2op' : l:st -> a:st -> b:st -> o1:jop -> o2:jop -> ob':jop -> ol:jop ->
+   Lemma (requires L.Either? (rc #sta #stb #oa #ob #m o2 o1) /\ L.Fst_then_snd? (rc #sta #stb #oa #ob #m ob' ol) /\ 
+                   L.get_rid o1 <> L.get_rid o2 /\ L.get_rid ob' <> L.get_rid ol /\
+                   L.distinct_ops o1 o2 /\ L.distinct_ops o1 ob' /\ L.distinct_ops o1 ol /\ L.distinct_ops o2 ob' /\ L.distinct_ops o2 ol /\ L.distinct_ops ob' ol /\
+                   ~ (get_key o1 = get_key ol && get_key o2 = get_key ol /\ get_key ob' = get_key ol /\
+                      is_alpha_op o1 /\ is_alpha_op o2 /\ is_alpha_op ob' /\ is_alpha_op ol /\ (L.Fst_then_snd? (m.rca (get_opa o2) (get_opa o1)) || L.Either? (m.rca (get_opa o2) (get_opa o1))) /\ L.Fst_then_snd? (m.rca (get_opa ob') (get_opa ol)) /\
+                      is_beta_op o1 /\ is_beta_op o2 /\ is_beta_op ob' /\ is_beta_op ol /\ (L.Fst_then_snd? (m.rcb (get_opb o2) (get_opb o1)) || L.Either? (m.rcb (get_opb o2) (get_opb o1))) /\ L.Fst_then_snd? (m.rcb (get_opb ob') (get_opb ol))) /\
                     eq (merge (do l ol) (do (do a ol) o1) (do (do b ol) o2)) (do (merge (do l ol) (do a ol) (do (do b ol) o2)) o1))
-         (ensures eq (merge (do l ol) (do (do (do a ob) ol) o1) (do (do b ol) o2)) (do (merge (do #st_a #st_b #o_a #o_b #m l ol) (do (do a ob) ol) (do (do b ol) o2)) o1));
+         (ensures eq (merge (do l ol) (do (do (do a ob') ol) o1) (do (do b ol) o2)) 
+                     (do (merge (do #sta #stb #oa #ob #m l ol) (do (do a ob') ol) (do (do b ol) o2)) o1));
 
- inter_right_2op_a : l:st_a -> a:st_a -> b:st_a -> o1:op_a -> o2:op_a -> ob:op_a -> ol:op_a -> o:op_a ->
-   Lemma (requires (Fst_then_snd? (m.rc_a o2 o1) \/ Either? (m.rc_a o2 o1)) /\ get_rid o1 <> get_rid o2 /\ Fst_then_snd? (m.rc_a ob ol) /\ get_rid ob <> get_rid ol /\
-                    (~ (Either? (m.rc_a o ob)) \/ Fst_then_snd? (m.rc_a o ol)) /\
-                    distinct_ops o1 o2 /\ distinct_ops o1 ob /\ distinct_ops o1 ol /\ distinct_ops o1 o /\ distinct_ops o2 ob /\ distinct_ops o2 ol /\ distinct_ops o2 o /\ distinct_ops ob ol /\ distinct_ops ob o /\ distinct_ops ol o /\
-                    get_rid o <> get_rid ol /\
-                    m.eq_a (m.merge_a (m.do_a l ol) (m.do_a (m.do_a a ol) o1) (m.do_a (m.do_a (m.do_a b ob) ol) o2)) (m.do_a (m.merge_a (m.do_a l ol) (m.do_a a ol) (m.do_a (m.do_a (m.do_a b ob) ol) o2)) o1))
-         (ensures m.eq_a (m.merge_a (m.do_a l ol) (m.do_a (m.do_a a ol) o1) (m.do_a (m.do_a (m.do_a (m.do_a b o) ob) ol) o2)) (m.do_a (m.merge_a (m.do_a l ol) (m.do_a a ol) (m.do_a (m.do_a (m.do_a (m.do_a b o) ob) ol) o2)) o1));
+ inter_right_2opa : l:sta -> a:sta -> b:sta -> o1:L.op #oa -> o2:L.op #oa -> ob:L.op #oa -> ol:L.op #oa -> o:L.op #oa ->
+   Lemma (requires (L.Fst_then_snd? (m.rca o2 o1) \/ L.Either? (m.rca o2 o1)) /\ L.Fst_then_snd? (m.rca ob ol) /\ 
+                    L.get_rid o1 <> L.get_rid o2 /\ L.get_rid ob <> L.get_rid ol /\
+                    (~ (L.Either? (m.rca o ob)) \/ L.Fst_then_snd? (m.rca o ol)) /\
+                    L.distinct_ops o1 o2 /\ L.distinct_ops o1 ob /\ L.distinct_ops o1 ol /\ L.distinct_ops o1 o /\ L.distinct_ops o2 ob /\
+                    L.distinct_ops o2 ol /\ L.distinct_ops o2 o /\ L.distinct_ops ob ol /\ L.distinct_ops ob o /\ L.distinct_ops ol o /\
+                    L.get_rid o <> L.get_rid ol /\
+                    m.eqa (m.mergea (m.doa l ol) (m.doa (m.doa a ol) o1) (m.doa (m.doa (m.doa b ob) ol) o2)) 
+                          (m.doa (m.mergea (m.doa l ol) (m.doa a ol) (m.doa (m.doa (m.doa b ob) ol) o2)) o1))
+         (ensures m.eqa (m.mergea (m.doa l ol) (m.doa (m.doa a ol) o1) (m.doa (m.doa (m.doa (m.doa b o) ob) ol) o2)) 
+                        (m.doa (m.mergea (m.doa l ol) (m.doa a ol) (m.doa (m.doa (m.doa (m.doa b o) ob) ol) o2)) o1));
 
- inter_right_2op_b : l:st_b -> a:st_b -> b:st_b -> o1:op_b -> o2:op_b -> ob:op_b -> ol:op_b -> o:op_b ->
-   Lemma (requires (Fst_then_snd? (m.rc_b o2 o1) \/ Either? (m.rc_b o2 o1)) /\ get_rid o1 <> get_rid o2 /\ Fst_then_snd? (m.rc_b ob ol) /\ get_rid ob <> get_rid ol /\
-                    (~ (Either? (m.rc_b o ob)) \/ Fst_then_snd? (m.rc_b o ol)) /\
-                    distinct_ops o1 o2 /\ distinct_ops o1 ob /\ distinct_ops o1 ol /\ distinct_ops o1 o /\ distinct_ops o2 ob /\ distinct_ops o2 ol /\ distinct_ops o2 o /\ distinct_ops ob ol /\ distinct_ops ob o /\ distinct_ops ol o /\
-                    get_rid o <> get_rid ol /\
-                    m.eq_b (m.merge_b (m.do_b l ol) (m.do_b (m.do_b a ol) o1) (m.do_b (m.do_b (m.do_b b ob) ol) o2)) (m.do_b (m.merge_b (m.do_b l ol) (m.do_b a ol) (m.do_b (m.do_b (m.do_b b ob) ol) o2)) o1))
-         (ensures m.eq_b (m.merge_b (m.do_b l ol) (m.do_b (m.do_b a ol) o1) (m.do_b (m.do_b (m.do_b (m.do_b b o) ob) ol) o2)) (m.do_b (m.merge_b (m.do_b l ol) (m.do_b a ol) (m.do_b (m.do_b (m.do_b (m.do_b b o) ob) ol) o2)) o1));
+ inter_right_2opb : l:stb -> a:stb -> b:stb -> o1:L.op #ob -> o2:L.op #ob -> ob':L.op #ob -> ol:L.op #ob -> o:L.op #ob ->
+   Lemma (requires (L.Fst_then_snd? (m.rcb o2 o1) \/ L.Either? (m.rcb o2 o1)) /\ L.Fst_then_snd? (m.rcb ob' ol) /\ 
+                    L.get_rid o1 <> L.get_rid o2 /\ L.get_rid ob' <> L.get_rid ol /\
+                    (~ (L.Either? (m.rcb o ob')) \/ L.Fst_then_snd? (m.rcb o ol)) /\
+                    L.distinct_ops o1 o2 /\ L.distinct_ops o1 ob' /\ L.distinct_ops o1 ol /\ L.distinct_ops o1 o /\ L.distinct_ops o2 ob' /\
+                    L.distinct_ops o2 ol /\ L.distinct_ops o2 o /\ L.distinct_ops ob' ol /\ L.distinct_ops ob' o /\ L.distinct_ops ol o /\
+                    L.get_rid o <> L.get_rid ol /\
+                    m.eqb (m.mergeb (m.dob l ol) (m.dob (m.dob a ol) o1) (m.dob (m.dob (m.dob b ob') ol) o2)) 
+                          (m.dob (m.mergeb (m.dob l ol) (m.dob a ol) (m.dob (m.dob (m.dob b ob') ol) o2)) o1))
+         (ensures m.eqb (m.mergeb (m.dob l ol) (m.dob (m.dob a ol) o1) (m.dob (m.dob (m.dob (m.dob b o) ob') ol) o2)) 
+                        (m.dob (m.mergeb (m.dob l ol) (m.dob a ol) (m.dob (m.dob (m.dob (m.dob b o) ob') ol) o2)) o1));
           
-  inter_right_2op' : l:st -> a:st -> b:st -> o1:op -> o2:op -> ob:op -> ol:op -> o:op ->
-    Lemma (requires Either? (rc #st_a #st_b #o_a #o_b #m o2 o1) /\ get_rid o1 <> get_rid o2 /\ Fst_then_snd? (rc #st_a #st_b #o_a #o_b #m ob ol) /\ get_rid ob <> get_rid ol /\
-                    (~ (Either? (rc #st_a #st_b #o_a #o_b #m o ob)) \/ Fst_then_snd? (rc #st_a #st_b #o_a #o_b #m o ol)) /\
-                    distinct_ops o1 o2 /\ distinct_ops o1 ob /\ distinct_ops o1 ol /\ distinct_ops o1 o /\ distinct_ops o2 ob /\ distinct_ops o2 ol /\ distinct_ops o2 o /\ distinct_ops ob ol /\ distinct_ops ob o /\ distinct_ops ol o /\
-                    get_rid o <> get_rid ol /\
-                    ~ (get_key o1 = get_key o && get_key o2 = get_key o /\ get_key ob = get_key o /\ get_key ol = get_key o /\
-                       is_alpha_op o1 /\ is_alpha_op o2 /\ is_alpha_op ob /\ is_alpha_op ol /\ is_alpha_op o /\ (Fst_then_snd? (m.rc_a (get_op_a o2) (get_op_a o1)) \/ Either? (m.rc_a (get_op_a o2) (get_op_a o1))) /\ Fst_then_snd? (m.rc_a (get_op_a ob) (get_op_a ol)) /\ (Fst_then_snd? (m.rc_a (get_op_a o) (get_op_a ob)) \/ Snd_then_fst? (m.rc_a (get_op_a o) (get_op_a ob)) \/ Fst_then_snd? (m.rc_a (get_op_a o) (get_op_a ol))) /\
-                       is_beta_op o1 /\ is_beta_op o2 /\ is_beta_op ob /\ is_beta_op ol /\ is_beta_op o /\ (Fst_then_snd? (m.rc_b (get_op_b o2) (get_op_b o1)) \/ Either? (m.rc_b (get_op_b o2) (get_op_b o1))) /\ Fst_then_snd? (m.rc_b (get_op_b ob) (get_op_b ol)) /\ (Fst_then_snd? (m.rc_b (get_op_b o) (get_op_b ob)) \/ Snd_then_fst? (m.rc_b (get_op_b o) (get_op_b ob)) \/ Fst_then_snd? (m.rc_b (get_op_b o) (get_op_b ol)))) /\
-                    eq (merge (do l ol) (do (do a ol) o1) (do (do (do b ob) ol) o2)) (do (merge (do l ol) (do a ol) (do (do (do b ob) ol) o2)) o1))
-         (ensures eq (merge (do l ol) (do (do a ol) o1) (do (do (do (do b o) ob) ol) o2)) (do (merge (do #st_a #st_b #o_a #o_b #m l ol) (do a ol) (do (do (do (do b o) ob) ol) o2)) o1));
+  inter_right_2op' : l:st -> a:st -> b:st -> o1:jop -> o2:jop -> ob':jop -> ol:jop -> o:jop ->
+    Lemma (requires L.Either? (rc #sta #stb #oa #ob #m o2 o1) /\ L.Fst_then_snd? (rc #sta #stb #oa #ob #m ob' ol) /\ 
+                    L.get_rid o1 <> L.get_rid o2 /\ L.get_rid ob' <> L.get_rid ol /\
+                    (~ (L.Either? (rc #sta #stb #oa #ob #m o ob')) \/ L.Fst_then_snd? (rc #sta #stb #oa #ob #m o ol)) /\
+                    L.distinct_ops o1 o2 /\ L.distinct_ops o1 ob' /\ L.distinct_ops o1 ol /\ L.distinct_ops o1 o /\ L.distinct_ops o2 ob' /\
+                    L.distinct_ops o2 ol /\ L.distinct_ops o2 o /\ L.distinct_ops ob' ol /\ L.distinct_ops ob' o /\ L.distinct_ops ol o /\
+                    L.get_rid o <> L.get_rid ol /\
+                    ~ (get_key o1 = get_key o && get_key o2 = get_key o /\ get_key ob' = get_key o /\ get_key ol = get_key o /\
+                       is_alpha_op o1 /\ is_alpha_op o2 /\ is_alpha_op ob' /\ is_alpha_op ol /\ is_alpha_op o /\ (L.Fst_then_snd? (m.rca (get_opa o2) (get_opa o1)) \/ L.Either? (m.rca (get_opa o2) (get_opa o1))) /\ L.Fst_then_snd? (m.rca (get_opa ob') (get_opa ol)) /\ (L.Fst_then_snd? (m.rca (get_opa o) (get_opa ob')) \/ L.Snd_then_fst? (m.rca (get_opa o) (get_opa ob')) \/ L.Fst_then_snd? (m.rca (get_opa o) (get_opa ol))) /\
+                       is_beta_op o1 /\ is_beta_op o2 /\ is_beta_op ob' /\ is_beta_op ol /\ is_beta_op o /\ (L.Fst_then_snd? (m.rcb (get_opb o2) (get_opb o1)) \/ L.Either? (m.rcb (get_opb o2) (get_opb o1))) /\ L.Fst_then_snd? (m.rcb (get_opb ob') (get_opb ol)) /\ (L.Fst_then_snd? (m.rcb (get_opb o) (get_opb ob')) \/ L.Snd_then_fst? (m.rcb (get_opb o) (get_opb ob')) \/ L.Fst_then_snd? (m.rcb (get_opb o) (get_opb ol)))) /\
+                    eq (merge (do l ol) (do (do a ol) o1) (do (do (do b ob') ol) o2)) 
+                       (do (merge (do l ol) (do a ol) (do (do (do b ob') ol) o2)) o1))
+         (ensures eq (merge (do l ol) (do (do a ol) o1) (do (do (do (do b o) ob') ol) o2)) 
+                     (do (merge (do #sta #stb #oa #ob #m l ol) (do a ol) (do (do (do (do b o) ob') ol) o2)) o1));
 
- inter_left_2op_a : l:st_a -> a:st_a -> b:st_a -> o1:op_a -> o2:op_a -> ob:op_a -> ol:op_a -> o:op_a ->
-   Lemma (requires (Fst_then_snd? (m.rc_a o2 o1) \/ Either? (m.rc_a o2 o1)) /\ get_rid o1 <> get_rid o2 /\ Fst_then_snd? (m.rc_a ob ol) /\ get_rid ob <> get_rid ol /\
-                    (~ (Either? (m.rc_a o ob)) \/ Fst_then_snd? (m.rc_a o ol)) /\
-                    distinct_ops o1 o2 /\ distinct_ops o1 ob /\ distinct_ops o1 ol /\ distinct_ops o1 o /\ distinct_ops o2 ob /\ distinct_ops o2 ol /\ distinct_ops o2 o /\ distinct_ops ob ol /\ distinct_ops ob o /\ distinct_ops ol o /\
-                    get_rid o <> get_rid ol /\
-                    m.eq_a (m.merge_a (m.do_a l ol) (m.do_a (m.do_a a ol) o1) (m.do_a (m.do_a (m.do_a b ob) ol) o2)) (m.do_a (m.merge_a (m.do_a l ol) (m.do_a a ol) (m.do_a (m.do_a (m.do_a b ob) ol) o2)) o1))
-          (ensures m.eq_a (m.merge_a (m.do_a l ol) (m.do_a (m.do_a (m.do_a a o) ol) o1) (m.do_a (m.do_a (m.do_a b ob) ol) o2)) (m.do_a (m.merge_a (m.do_a l ol) (m.do_a (m.do_a a o) ol) (m.do_a (m.do_a (m.do_a b ob) ol) o2)) o1));
+ inter_left_2opa : l:sta -> a:sta -> b:sta -> o1:L.op #oa -> o2:L.op #oa -> ob:L.op #oa -> ol:L.op #oa -> o:L.op #oa ->
+   Lemma (requires (L.Fst_then_snd? (m.rca o2 o1) \/ L.Either? (m.rca o2 o1)) /\ L.Fst_then_snd? (m.rca ob ol) /\ 
+                    L.get_rid o1 <> L.get_rid o2 /\ L.get_rid ob <> L.get_rid ol /\
+                    (~ (L.Either? (m.rca o ob)) \/ L.Fst_then_snd? (m.rca o ol)) /\
+                    L.distinct_ops o1 o2 /\ L.distinct_ops o1 ob /\ L.distinct_ops o1 ol /\ L.distinct_ops o1 o /\ L.distinct_ops o2 ob /\
+                    L.distinct_ops o2 ol /\ L.distinct_ops o2 o /\ L.distinct_ops ob ol /\ L.distinct_ops ob o /\ L.distinct_ops ol o /\
+                    L.get_rid o <> L.get_rid ol /\
+                    m.eqa (m.mergea (m.doa l ol) (m.doa (m.doa a ol) o1) (m.doa (m.doa (m.doa b ob) ol) o2)) 
+                          (m.doa (m.mergea (m.doa l ol) (m.doa a ol) (m.doa (m.doa (m.doa b ob) ol) o2)) o1))
+          (ensures m.eqa (m.mergea (m.doa l ol) (m.doa (m.doa (m.doa a o) ol) o1) (m.doa (m.doa (m.doa b ob) ol) o2)) 
+                         (m.doa (m.mergea (m.doa l ol) (m.doa (m.doa a o) ol) (m.doa (m.doa (m.doa b ob) ol) o2)) o1));
 
- inter_left_2op_b : l:st_b -> a:st_b -> b:st_b -> o1:op_b -> o2:op_b -> ob:op_b -> ol:op_b -> o:op_b ->
-   Lemma (requires (Fst_then_snd? (m.rc_b o2 o1) \/ Either? (m.rc_b o2 o1)) /\ get_rid o1 <> get_rid o2 /\ Fst_then_snd? (m.rc_b ob ol) /\ get_rid ob <> get_rid ol /\
-                    (~ (Either? (m.rc_b o ob)) \/ Fst_then_snd? (m.rc_b o ol)) /\
-                    distinct_ops o1 o2 /\ distinct_ops o1 ob /\ distinct_ops o1 ol /\ distinct_ops o1 o /\ distinct_ops o2 ob /\ distinct_ops o2 ol /\ distinct_ops o2 o /\ distinct_ops ob ol /\ distinct_ops ob o /\ distinct_ops ol o /\
-                    get_rid o <> get_rid ol /\
-                    m.eq_b (m.merge_b (m.do_b l ol) (m.do_b (m.do_b a ol) o1) (m.do_b (m.do_b (m.do_b b ob) ol) o2)) (m.do_b (m.merge_b (m.do_b l ol) (m.do_b a ol) (m.do_b (m.do_b (m.do_b b ob) ol) o2)) o1))
-         (ensures m.eq_b (m.merge_b (m.do_b l ol) (m.do_b (m.do_b (m.do_b a o) ol) o1) (m.do_b (m.do_b (m.do_b b ob) ol) o2)) (m.do_b (m.merge_b (m.do_b l ol) (m.do_b (m.do_b a o) ol) (m.do_b (m.do_b (m.do_b b ob) ol) o2)) o1));
+ inter_left_2opb : l:stb -> a:stb -> b:stb -> o1:L.op #ob -> o2:L.op #ob -> ob':L.op #ob -> ol:L.op #ob -> o:L.op #ob ->
+   Lemma (requires (L.Fst_then_snd? (m.rcb o2 o1) \/ L.Either? (m.rcb o2 o1)) /\ L.Fst_then_snd? (m.rcb ob' ol) /\ 
+                    L.get_rid o1 <> L.get_rid o2 /\ L.get_rid ob' <> L.get_rid ol /\
+                    (~ (L.Either? (m.rcb o ob')) \/ L.Fst_then_snd? (m.rcb o ol)) /\
+                    L.distinct_ops o1 o2 /\ L.distinct_ops o1 ob' /\ L.distinct_ops o1 ol /\ L.distinct_ops o1 o /\ L.distinct_ops o2 ob' /\
+                    L.distinct_ops o2 ol /\ L.distinct_ops o2 o /\ L.distinct_ops ob' ol /\ L.distinct_ops ob' o /\ L.distinct_ops ol o /\
+                    L.get_rid o <> L.get_rid ol /\
+                    m.eqb (m.mergeb (m.dob l ol) (m.dob (m.dob a ol) o1) (m.dob (m.dob (m.dob b ob') ol) o2)) 
+                          (m.dob (m.mergeb (m.dob l ol) (m.dob a ol) (m.dob (m.dob (m.dob b ob') ol) o2)) o1))
+         (ensures m.eqb (m.mergeb (m.dob l ol) (m.dob (m.dob (m.dob a o) ol) o1) (m.dob (m.dob (m.dob b ob') ol) o2)) 
+                        (m.dob (m.mergeb (m.dob l ol) (m.dob (m.dob a o) ol) (m.dob (m.dob (m.dob b ob') ol) o2)) o1));
           
- inter_left_2op' : l:st -> a:st -> b:st -> o1:op -> o2:op -> ob:op -> ol:op -> o:op ->
-   Lemma (requires Either? (rc #st_a #st_b #o_a #o_b #m o2 o1) /\ get_rid o1 <> get_rid o2 /\ Fst_then_snd? (rc #st_a #st_b #o_a #o_b #m ob ol) /\ get_rid ob <> get_rid ol /\
-                    distinct_ops o1 o2 /\ distinct_ops o1 ob /\ distinct_ops o1 ol /\ distinct_ops o1 o /\ distinct_ops o2 ob /\ distinct_ops o2 ol /\ distinct_ops o2 o /\ distinct_ops ob ol /\ distinct_ops ob o /\ distinct_ops ol o /\
-                    get_rid o <> get_rid ol /\
-                    ~ (get_key o1 = get_key o && get_key o2 = get_key o /\ get_key ob = get_key o /\ get_key ol = get_key o /\
-                       is_alpha_op o1 /\ is_alpha_op o2 /\ is_alpha_op ob /\ is_alpha_op ol /\ is_alpha_op o /\ (Fst_then_snd? (m.rc_a (get_op_a o2) (get_op_a o1)) \/ Either? (m.rc_a (get_op_a o2) (get_op_a o1))) /\ Fst_then_snd? (m.rc_a (get_op_a ob) (get_op_a ol)) /\ (Fst_then_snd? (m.rc_a (get_op_a o) (get_op_a ob)) \/ Snd_then_fst? (m.rc_a (get_op_a o) (get_op_a ob)) \/ Fst_then_snd? (m.rc_a (get_op_a o) (get_op_a ol))) /\
-                       is_beta_op o1 /\ is_beta_op o2 /\ is_beta_op ob /\ is_beta_op ol /\ is_beta_op o /\ (Fst_then_snd? (m.rc_b (get_op_b o2) (get_op_b o1)) \/ Either? (m.rc_b (get_op_b o2) (get_op_b o1))) /\ Fst_then_snd? (m.rc_b (get_op_b ob) (get_op_b ol)) /\ (Fst_then_snd? (m.rc_b (get_op_b o) (get_op_b ob)) \/ Snd_then_fst? (m.rc_b (get_op_b o) (get_op_b ob)) \/ Fst_then_snd? (m.rc_b (get_op_b o) (get_op_b ol)))) /\
-                    eq (merge (do l ol) (do (do a ol) o1) (do (do (do b ob) ol) o2)) (do (merge (do l ol) (do a ol) (do (do (do b ob) ol) o2)) o1))
-         (ensures eq (merge (do l ol) (do (do (do a o) ol) o1) (do (do (do b ob) ol) o2)) (do (merge (do #st_a #st_b #o_a #o_b #m l ol) (do (do a o) ol) (do (do (do b ob) ol) o2)) o1));
+ inter_left_2op' : l:st -> a:st -> b:st -> o1:jop -> o2:jop -> ob':jop -> ol:jop -> o:jop ->
+   Lemma (requires L.Either? (rc #sta #stb #oa #ob #m o2 o1) /\ L.Fst_then_snd? (rc #sta #stb #oa #ob #m ob' ol) /\ 
+                    L.get_rid o1 <> L.get_rid o2 /\ L.get_rid ob' <> L.get_rid ol /\
+                    L.distinct_ops o1 o2 /\ L.distinct_ops o1 ob' /\ L.distinct_ops o1 ol /\ L.distinct_ops o1 o /\ L.distinct_ops o2 ob' /\
+                    L.distinct_ops o2 ol /\ L.distinct_ops o2 o /\ L.distinct_ops ob' ol /\ L.distinct_ops ob' o /\ L.distinct_ops ol o /\
+                    L.get_rid o <> L.get_rid ol /\
+                    ~ (get_key o1 = get_key o && get_key o2 = get_key o /\ get_key ob' = get_key o /\ get_key ol = get_key o /\
+                       is_alpha_op o1 /\ is_alpha_op o2 /\ is_alpha_op ob' /\ is_alpha_op ol /\ is_alpha_op o /\ (L.Fst_then_snd? (m.rca (get_opa o2) (get_opa o1)) \/ L.Either? (m.rca (get_opa o2) (get_opa o1))) /\ L.Fst_then_snd? (m.rca (get_opa ob') (get_opa ol)) /\ (L.Fst_then_snd? (m.rca (get_opa o) (get_opa ob')) \/ L.Snd_then_fst? (m.rca (get_opa o) (get_opa ob')) \/ L.Fst_then_snd? (m.rca (get_opa o) (get_opa ol))) /\
+                       is_beta_op o1 /\ is_beta_op o2 /\ is_beta_op ob' /\ is_beta_op ol /\ is_beta_op o /\ (L.Fst_then_snd? (m.rcb (get_opb o2) (get_opb o1)) \/ L.Either? (m.rcb (get_opb o2) (get_opb o1))) /\ L.Fst_then_snd? (m.rcb (get_opb ob') (get_opb ol)) /\ (L.Fst_then_snd? (m.rcb (get_opb o) (get_opb ob')) \/ L.Snd_then_fst? (m.rcb (get_opb o) (get_opb ob')) \/ L.Fst_then_snd? (m.rcb (get_opb o) (get_opb ol)))) /\
+                    eq (merge (do l ol) (do (do a ol) o1) (do (do (do b ob') ol) o2)) 
+                       (do (merge (do l ol) (do a ol) (do (do (do b ob') ol) o2)) o1))
+         (ensures eq (merge (do l ol) (do (do (do a o) ol) o1) (do (do (do b ob') ol) o2)) 
+                     (do (merge (do #sta #stb #oa #ob #m l ol) (do (do a o) ol) (do (do (do b ob') ol) o2)) o1));
           
- ind_right_2op_a : l:st_a -> a:st_a -> b:st_a -> o1:op_a -> o2:op_a -> o2':op_a ->
-  Lemma (requires Fst_then_snd? (m.rc_a o2 o1) /\ get_rid o1 <> get_rid o2 /\
-                    distinct_ops o1 o2 /\ distinct_ops o1 o2' /\ distinct_ops o2 o2' /\
-                    m.eq_a (m.merge_a l (m.do_a a o1) (m.do_a b o2)) (m.do_a (m.merge_a l a (m.do_a b o2)) o1))
-         (ensures m.eq_a (m.merge_a l (m.do_a a o1) (m.do_a (m.do_a b o2') o2)) (m.do_a (m.merge_a l a (m.do_a (m.do_a b o2') o2)) o1));
+ ind_right_2opa : l:sta -> a:sta -> b:sta -> o1:L.op #oa -> o2:L.op #oa -> o2':L.op #oa ->
+  Lemma (requires L.Fst_then_snd? (m.rca o2 o1) /\ L.get_rid o1 <> L.get_rid o2 /\
+                  L.distinct_ops o1 o2 /\ L.distinct_ops o1 o2' /\ L.distinct_ops o2 o2' /\
+                  m.eqa (m.mergea l (m.doa a o1) (m.doa b o2)) (m.doa (m.mergea l a (m.doa b o2)) o1))
+        (ensures m.eqa (m.mergea l (m.doa a o1) (m.doa (m.doa b o2') o2)) (m.doa (m.mergea l a (m.doa (m.doa b o2') o2)) o1));
 
- ind_right_2op_b : l:st_b -> a:st_b -> b:st_b -> o1:op_b -> o2:op_b -> o2':op_b ->
-   Lemma (requires Fst_then_snd? (m.rc_b o2 o1) /\ get_rid o1 <> get_rid o2 /\
-                    distinct_ops o1 o2 /\ distinct_ops o1 o2' /\ distinct_ops o2 o2' /\
-                    m.eq_b (m.merge_b l (m.do_b a o1) (m.do_b b o2)) (m.do_b (m.merge_b l a (m.do_b b o2)) o1))
-         (ensures m.eq_b (m.merge_b l (m.do_b a o1) (m.do_b (m.do_b b o2') o2)) (m.do_b (m.merge_b l a (m.do_b (m.do_b b o2') o2)) o1));
+ ind_right_2opb : l:stb -> a:stb -> b:stb -> o1:L.op #ob -> o2:L.op #ob -> o2':L.op #ob ->
+   Lemma (requires L.Fst_then_snd? (m.rcb o2 o1) /\ L.get_rid o1 <> L.get_rid o2 /\
+                   L.distinct_ops o1 o2 /\ L.distinct_ops o1 o2' /\ L.distinct_ops o2 o2' /\
+                   m.eqb (m.mergeb l (m.dob a o1) (m.dob b o2)) (m.dob (m.mergeb l a (m.dob b o2)) o1))
+         (ensures m.eqb (m.mergeb l (m.dob a o1) (m.dob (m.dob b o2') o2)) (m.dob (m.mergeb l a (m.dob (m.dob b o2') o2)) o1));
 
- ind_left_2op_a : l:st_a -> a:st_a -> b:st_a -> o1:op_a -> o2:op_a -> o1':op_a ->
-   Lemma (requires Fst_then_snd? (m.rc_a o2 o1) /\ get_rid o1 <> get_rid o2 /\
-                    distinct_ops o1 o2 /\ distinct_ops o1 o1' /\ distinct_ops o2 o1' /\
-                    m.eq_a (m.merge_a l (m.do_a a o1) (m.do_a b o2)) (m.do_a (m.merge_a l a (m.do_a b o2)) o1))
-         (ensures m.eq_a (m.merge_a l (m.do_a (m.do_a a o1') o1) (m.do_a b o2)) (m.do_a (m.merge_a l (m.do_a a o1') (m.do_a b o2)) o1));
+ ind_left_2opa : l:sta -> a:sta -> b:sta -> o1:L.op #oa -> o2:L.op #oa -> o1':L.op #oa ->
+   Lemma (requires L.Fst_then_snd? (m.rca o2 o1) /\ L.get_rid o1 <> L.get_rid o2 /\
+                   L.distinct_ops o1 o2 /\ L.distinct_ops o1 o1' /\ L.distinct_ops o2 o1' /\
+                   m.eqa (m.mergea l (m.doa a o1) (m.doa b o2)) (m.doa (m.mergea l a (m.doa b o2)) o1))
+         (ensures m.eqa (m.mergea l (m.doa (m.doa a o1') o1) (m.doa b o2)) (m.doa (m.mergea l (m.doa a o1') (m.doa b o2)) o1));
 
- ind_left_2op_b : l:st_b -> a:st_b -> b:st_b -> o1:op_b -> o2:op_b -> o1':op_b ->
-   Lemma (requires Fst_then_snd? (m.rc_b o2 o1) /\ get_rid o1 <> get_rid o2 /\
-                    distinct_ops o1 o2 /\ distinct_ops o1 o1' /\ distinct_ops o2 o1' /\
-                    m.eq_b (m.merge_b l (m.do_b a o1) (m.do_b b o2)) (m.do_b (m.merge_b l a (m.do_b b o2)) o1))
-         (ensures m.eq_b (m.merge_b l (m.do_b (m.do_b a o1') o1) (m.do_b b o2)) (m.do_b (m.merge_b l (m.do_b a o1') (m.do_b b o2)) o1));
+ ind_left_2opb : l:stb -> a:stb -> b:stb -> o1:L.op #ob -> o2:L.op #ob -> o1':L.op #ob ->
+   Lemma (requires L.Fst_then_snd? (m.rcb o2 o1) /\ L.get_rid o1 <> L.get_rid o2 /\
+                   L.distinct_ops o1 o2 /\ L.distinct_ops o1 o1' /\ L.distinct_ops o2 o1' /\
+                   m.eqb (m.mergeb l (m.dob a o1) (m.dob b o2)) (m.dob (m.mergeb l a (m.dob b o2)) o1))
+         (ensures m.eqb (m.mergeb l (m.dob (m.dob a o1') o1) (m.dob b o2)) (m.dob (m.mergeb l (m.dob a o1') (m.dob b o2)) o1));
 
- base_1op_a : o1:op_a -> 
-  Lemma (ensures m.eq_a (m.merge_a m.init_st_a (m.do_a m.init_st_a o1) m.init_st_a) (m.do_a (m.merge_a m.init_st_a m.init_st_a m.init_st_a) o1));
+ base_1opa : o1:L.op #oa -> 
+  Lemma (ensures m.eqa (m.mergea m.init_sta (m.doa m.init_sta o1) m.init_sta) (m.doa (m.mergea m.init_sta m.init_sta m.init_sta) o1));
 
- base_1op_b : o1:op_b -> 
-  Lemma (ensures m.eq_b (m.merge_b m.init_st_b (m.do_b m.init_st_b o1) m.init_st_b) (m.do_b (m.merge_b m.init_st_b m.init_st_b m.init_st_b) o1));
+ base_1opb : o1:L.op #ob -> 
+  Lemma (ensures m.eqb (m.mergeb m.init_stb (m.dob m.init_stb o1) m.init_stb) (m.dob (m.mergeb m.init_stb m.init_stb m.init_stb) o1));
 
- ind_lca_1op_a : l:st_a -> o1:op_a -> ol:op_a ->
-   Lemma (requires distinct_ops o1 ol /\ 
-                    m.eq_a (m.merge_a l (m.do_a l o1) l) (m.do_a (m.merge_a l l l) o1))
-         (ensures m.eq_a (m.merge_a (m.do_a l ol) (m.do_a (m.do_a l ol) o1) (m.do_a l ol)) (m.do_a (m.merge_a (m.do_a l ol) (m.do_a l ol) (m.do_a l ol)) o1));
+ ind_lca_1opa : l:sta -> o1:L.op #oa -> ol:L.op #oa ->
+   Lemma (requires L.distinct_ops o1 ol /\ 
+                    m.eqa (m.mergea l (m.doa l o1) l) (m.doa (m.mergea l l l) o1))
+         (ensures m.eqa (m.mergea (m.doa l ol) (m.doa (m.doa l ol) o1) (m.doa l ol)) 
+                        (m.doa (m.mergea (m.doa l ol) (m.doa l ol) (m.doa l ol)) o1));
 
- ind_lca_1op_b : l:st_b -> o1:op_b -> ol:op_b ->
-   Lemma (requires distinct_ops o1 ol /\
-                    m.eq_b (m.merge_b l (m.do_b l o1) l) (m.do_b (m.merge_b l l l) o1))
-         (ensures m.eq_b (m.merge_b (m.do_b l ol) (m.do_b (m.do_b l ol) o1) (m.do_b l ol)) (m.do_b (m.merge_b (m.do_b l ol) (m.do_b l ol) (m.do_b l ol)) o1));
+ ind_lca_1opb : l:stb -> o1:L.op #ob -> ol:L.op #ob ->
+   Lemma (requires L.distinct_ops o1 ol /\
+                    m.eqb (m.mergeb l (m.dob l o1) l) (m.dob (m.mergeb l l l) o1))
+         (ensures m.eqb (m.mergeb (m.dob l ol) (m.dob (m.dob l ol) o1) (m.dob l ol)) 
+                        (m.dob (m.mergeb (m.dob l ol) (m.dob l ol) (m.dob l ol)) o1));
 
- inter_right_base_1op_a : l:st_a -> a:st_a -> b:st_a -> o1:op_a -> ob:op_a -> ol:op_a ->
-   Lemma (requires Fst_then_snd? (m.rc_a ob ol) /\ get_rid ob <> get_rid ol /\
-                   distinct_ops o1 ob /\ distinct_ops o1 ol /\ distinct_ops ob ol /\
-                   m.eq_a (m.merge_a (m.do_a l ol) (m.do_a (m.do_a a ol) o1) (m.do_a b ol)) (m.do_a (m.merge_a (m.do_a l ol) (m.do_a a ol) (m.do_a b ol)) o1))
-         (ensures m.eq_a (m.merge_a (m.do_a l ol) (m.do_a (m.do_a a ol) o1) (m.do_a (m.do_a b ob) ol)) (m.do_a (m.merge_a (m.do_a l ol) (m.do_a a ol) (m.do_a (m.do_a b ob) ol)) o1));
+ inter_right_base_1opa : l:sta -> a:sta -> b:sta -> o1:L.op #oa -> ob:L.op #oa -> ol:L.op #oa ->
+   Lemma (requires L.Fst_then_snd? (m.rca ob ol) /\ L.get_rid ob <> L.get_rid ol /\
+                   L.distinct_ops o1 ob /\ L.distinct_ops o1 ol /\ L.distinct_ops ob ol /\
+                   m.eqa (m.mergea (m.doa l ol) (m.doa (m.doa a ol) o1) (m.doa b ol)) 
+                         (m.doa (m.mergea (m.doa l ol) (m.doa a ol) (m.doa b ol)) o1))
+         (ensures m.eqa (m.mergea (m.doa l ol) (m.doa (m.doa a ol) o1) (m.doa (m.doa b ob) ol)) 
+                        (m.doa (m.mergea (m.doa l ol) (m.doa a ol) (m.doa (m.doa b ob) ol)) o1));
 
- inter_right_base_1op_b : l:st_b -> a:st_b -> b:st_b -> o1:op_b -> ob:op_b -> ol:op_b ->
-   Lemma (requires Fst_then_snd? (m.rc_b ob ol) /\ get_rid ob <> get_rid ol /\
-                   distinct_ops o1 ob /\ distinct_ops o1 ol /\ distinct_ops ob ol /\
-                   m.eq_b (m.merge_b (m.do_b l ol) (m.do_b (m.do_b a ol) o1) (m.do_b b ol)) (m.do_b (m.merge_b (m.do_b l ol) (m.do_b a ol) (m.do_b b ol)) o1))
-         (ensures m.eq_b (m.merge_b (m.do_b l ol) (m.do_b (m.do_b a ol) o1) (m.do_b (m.do_b b ob) ol)) (m.do_b (m.merge_b (m.do_b l ol) (m.do_b a ol) (m.do_b (m.do_b b ob) ol)) o1));
+ inter_right_base_1opb : l:stb -> a:stb -> b:stb -> o1:L.op #ob -> ob':L.op #ob -> ol:L.op #ob ->
+   Lemma (requires L.Fst_then_snd? (m.rcb ob' ol) /\ L.get_rid ob' <> L.get_rid ol /\
+                   L.distinct_ops o1 ob' /\ L.distinct_ops o1 ol /\ L.distinct_ops ob' ol /\
+                   m.eqb (m.mergeb (m.dob l ol) (m.dob (m.dob a ol) o1) (m.dob b ol)) 
+                         (m.dob (m.mergeb (m.dob l ol) (m.dob a ol) (m.dob b ol)) o1))
+         (ensures m.eqb (m.mergeb (m.dob l ol) (m.dob (m.dob a ol) o1) (m.dob (m.dob b ob') ol)) 
+                        (m.dob (m.mergeb (m.dob l ol) (m.dob a ol) (m.dob (m.dob b ob') ol)) o1));
 
- inter_left_base_1op_a : l:st_a -> a:st_a -> b:st_a -> o1:op_a -> ob:op_a -> ol:op_a ->
-   Lemma (requires Fst_then_snd? (m.rc_a ob ol) /\ get_rid ob <> get_rid ol /\
-                   distinct_ops o1 ob /\ distinct_ops o1 ol /\ distinct_ops ob ol /\
-                   m.eq_a (m.merge_a (m.do_a l ol) (m.do_a (m.do_a a ol) o1) (m.do_a b ol)) (m.do_a (m.merge_a (m.do_a l ol) (m.do_a a ol) (m.do_a b ol)) o1))
-         (ensures m.eq_a (m.merge_a (m.do_a l ol) (m.do_a (m.do_a (m.do_a a ob) ol) o1) (m.do_a b ol)) (m.do_a (m.merge_a (m.do_a l ol) (m.do_a (m.do_a a ob) ol) (m.do_a b ol)) o1));
+ inter_left_base_1opa : l:sta -> a:sta -> b:sta -> o1:L.op #oa -> ob:L.op #oa -> ol:L.op #oa ->
+   Lemma (requires L.Fst_then_snd? (m.rca ob ol) /\ L.get_rid ob <> L.get_rid ol /\
+                   L.distinct_ops o1 ob /\ L.distinct_ops o1 ol /\ L.distinct_ops ob ol /\
+                   m.eqa (m.mergea (m.doa l ol) (m.doa (m.doa a ol) o1) (m.doa b ol)) 
+                         (m.doa (m.mergea (m.doa l ol) (m.doa a ol) (m.doa b ol)) o1))
+         (ensures m.eqa (m.mergea (m.doa l ol) (m.doa (m.doa (m.doa a ob) ol) o1) (m.doa b ol)) 
+                        (m.doa (m.mergea (m.doa l ol) (m.doa (m.doa a ob) ol) (m.doa b ol)) o1));
 
- inter_left_base_1op_b : l:st_b -> a:st_b -> b:st_b -> o1:op_b -> ob:op_b -> ol:op_b ->
-   Lemma (requires Fst_then_snd? (m.rc_b ob ol) /\ get_rid ob <> get_rid ol /\
-                   distinct_ops o1 ob /\ distinct_ops o1 ol /\ distinct_ops ob ol /\
-                   m.eq_b (m.merge_b (m.do_b l ol) (m.do_b (m.do_b a ol) o1) (m.do_b b ol)) (m.do_b (m.merge_b (m.do_b l ol) (m.do_b a ol) (m.do_b b ol)) o1))
-         (ensures m.eq_b (m.merge_b (m.do_b l ol) (m.do_b (m.do_b (m.do_b a ob) ol) o1) (m.do_b b ol)) (m.do_b (m.merge_b (m.do_b l ol) (m.do_b (m.do_b a ob) ol) (m.do_b b ol)) o1));
+ inter_left_base_1opb : l:stb -> a:stb -> b:stb -> o1:L.op #ob -> ob':L.op #ob -> ol:L.op #ob ->
+   Lemma (requires L.Fst_then_snd? (m.rcb ob' ol) /\ L.get_rid ob' <> L.get_rid ol /\
+                   L.distinct_ops o1 ob' /\ L.distinct_ops o1 ol /\ L.distinct_ops ob' ol /\
+                   m.eqb (m.mergeb (m.dob l ol) (m.dob (m.dob a ol) o1) (m.dob b ol)) 
+                         (m.dob (m.mergeb (m.dob l ol) (m.dob a ol) (m.dob b ol)) o1))
+         (ensures m.eqb (m.mergeb (m.dob l ol) (m.dob (m.dob (m.dob a ob') ol) o1) (m.dob b ol)) 
+                        (m.dob (m.mergeb (m.dob l ol) (m.dob (m.dob a ob') ol) (m.dob b ol)) o1));
 
- inter_right_1op_a : l:st_a -> a:st_a -> b:st_a -> o1:op_a -> ob:op_a -> ol:op_a -> o:op_a ->
-   Lemma (requires Fst_then_snd? (m.rc_a ob ol) /\ get_rid ob <> get_rid ol /\
-                   (~ (Either? (m.rc_a o ob)) \/ Fst_then_snd? (m.rc_a o ol)) /\
-                   distinct_ops o1 ob /\ distinct_ops o1 ol /\ distinct_ops o1 o /\ distinct_ops ob ol /\ distinct_ops ob o /\ distinct_ops ol o /\
-                    get_rid o <> get_rid ol /\
-                    m.eq_a (m.merge_a (m.do_a l ol) (m.do_a (m.do_a a ol) o1) (m.do_a (m.do_a b ob) ol)) (m.do_a (m.merge_a (m.do_a l ol) (m.do_a a ol) (m.do_a (m.do_a b ob) ol)) o1))
-         (ensures m.eq_a (m.merge_a (m.do_a l ol) (m.do_a (m.do_a a ol) o1) (m.do_a (m.do_a (m.do_a b o) ob) ol)) (m.do_a (m.merge_a (m.do_a l ol) (m.do_a a ol) (m.do_a (m.do_a (m.do_a b o) ob) ol)) o1));
+ inter_right_1opa : l:sta -> a:sta -> b:sta -> o1:L.op #oa -> ob:L.op #oa -> ol:L.op #oa -> o:L.op #oa ->
+   Lemma (requires L.Fst_then_snd? (m.rca ob ol) /\ L.get_rid ob <> L.get_rid ol /\
+                   (~ (L.Either? (m.rca o ob)) \/ L.Fst_then_snd? (m.rca o ol)) /\
+                   L.distinct_ops o1 ob /\ L.distinct_ops o1 ol /\ L.distinct_ops o1 o /\ 
+                   L.distinct_ops ob ol /\ L.distinct_ops ob o /\ L.distinct_ops ol o /\
+                   L.get_rid o <> L.get_rid ol /\
+                   m.eqa (m.mergea (m.doa l ol) (m.doa (m.doa a ol) o1) (m.doa (m.doa b ob) ol)) 
+                         (m.doa (m.mergea (m.doa l ol) (m.doa a ol) (m.doa (m.doa b ob) ol)) o1))
+         (ensures m.eqa (m.mergea (m.doa l ol) (m.doa (m.doa a ol) o1) (m.doa (m.doa (m.doa b o) ob) ol)) 
+                        (m.doa (m.mergea (m.doa l ol) (m.doa a ol) (m.doa (m.doa (m.doa b o) ob) ol)) o1));
 
- inter_right_1op_b : l:st_b -> a:st_b -> b:st_b -> o1:op_b -> ob:op_b -> ol:op_b -> o:op_b ->
-   Lemma (requires Fst_then_snd? (m.rc_b ob ol) /\ get_rid ob <> get_rid ol /\
-                   (~ (Either? (m.rc_b o ob)) \/ Fst_then_snd? (m.rc_b o ol)) /\
-                   distinct_ops o1 ob /\ distinct_ops o1 ol /\ distinct_ops o1 o /\ distinct_ops ob ol /\ distinct_ops ob o /\ distinct_ops ol o /\
-                    get_rid o <> get_rid ol /\
-                    m.eq_b (m.merge_b (m.do_b l ol) (m.do_b (m.do_b a ol) o1) (m.do_b (m.do_b b ob) ol)) (m.do_b (m.merge_b (m.do_b l ol) (m.do_b a ol) (m.do_b (m.do_b b ob) ol)) o1))
-         (ensures m.eq_b (m.merge_b (m.do_b l ol) (m.do_b (m.do_b a ol) o1) (m.do_b (m.do_b (m.do_b b o) ob) ol)) (m.do_b (m.merge_b (m.do_b l ol) (m.do_b a ol) (m.do_b (m.do_b (m.do_b b o) ob) ol)) o1));
+ inter_right_1opb : l:stb -> a:stb -> b:stb -> o1:L.op #ob -> ob':L.op #ob -> ol:L.op #ob -> o:L.op #ob ->
+   Lemma (requires L.Fst_then_snd? (m.rcb ob' ol) /\ L.get_rid ob' <> L.get_rid ol /\
+                   (~ (L.Either? (m.rcb o ob')) \/ L.Fst_then_snd? (m.rcb o ol)) /\
+                   L.distinct_ops o1 ob' /\ L.distinct_ops o1 ol /\ L.distinct_ops o1 o /\ 
+                   L.distinct_ops ob' ol /\ L.distinct_ops ob' o /\ L.distinct_ops ol o /\
+                   L.get_rid o <> L.get_rid ol /\
+                   m.eqb (m.mergeb (m.dob l ol) (m.dob (m.dob a ol) o1) (m.dob (m.dob b ob') ol)) 
+                         (m.dob (m.mergeb (m.dob l ol) (m.dob a ol) (m.dob (m.dob b ob') ol)) o1))
+         (ensures m.eqb (m.mergeb (m.dob l ol) (m.dob (m.dob a ol) o1) (m.dob (m.dob (m.dob b o) ob') ol)) 
+                  (m.dob (m.mergeb (m.dob l ol) (m.dob a ol) (m.dob (m.dob (m.dob b o) ob') ol)) o1));
 
- inter_left_1op_a : l:st_a -> a:st_a -> b:st_a -> o1:op_a -> ob:op_a -> ol:op_a -> o:op_a ->
-   Lemma (requires Fst_then_snd? (m.rc_a ob ol) /\ get_rid ob <> get_rid ol /\
-                    (~ (Either? (m.rc_a o ob)) \/ Fst_then_snd? (m.rc_a o ol)) /\
-                    distinct_ops o1 ob /\ distinct_ops o1 ol /\ distinct_ops o1 o /\ distinct_ops ob ol /\ distinct_ops ob o /\ distinct_ops ol o /\
-                    get_rid o <> get_rid ol /\
-                    m.eq_a (m.merge_a (m.do_a l ol) (m.do_a (m.do_a (m.do_a a ob) ol) o1) (m.do_a b ol)) (m.do_a (m.merge_a (m.do_a l ol) (m.do_a (m.do_a a ob) ol) (m.do_a b ol)) o1))
-         (ensures m.eq_a (m.merge_a (m.do_a l ol) (m.do_a (m.do_a (m.do_a (m.do_a a o) ob) ol) o1) (m.do_a b ol)) (m.do_a (m.merge_a (m.do_a l ol) (m.do_a (m.do_a (m.do_a a o) ob) ol) (m.do_a b ol)) o1));
+ inter_left_1opa : l:sta -> a:sta -> b:sta -> o1:L.op #oa -> ob:L.op #oa -> ol:L.op #oa -> o:L.op #oa ->
+   Lemma (requires L.Fst_then_snd? (m.rca ob ol) /\ L.get_rid ob <> L.get_rid ol /\
+                   (~ (L.Either? (m.rca o ob)) \/ L.Fst_then_snd? (m.rca o ol)) /\
+                   L.distinct_ops o1 ob /\ L.distinct_ops o1 ol /\ L.distinct_ops o1 o /\ 
+                   L.distinct_ops ob ol /\ L.distinct_ops ob o /\ L.distinct_ops ol o /\
+                   L.get_rid o <> L.get_rid ol /\
+                   m.eqa (m.mergea (m.doa l ol) (m.doa (m.doa (m.doa a ob) ol) o1) (m.doa b ol)) 
+                         (m.doa (m.mergea (m.doa l ol) (m.doa (m.doa a ob) ol) (m.doa b ol)) o1))
+         (ensures m.eqa (m.mergea (m.doa l ol) (m.doa (m.doa (m.doa (m.doa a o) ob) ol) o1) (m.doa b ol)) 
+                        (m.doa (m.mergea (m.doa l ol) (m.doa (m.doa (m.doa a o) ob) ol) (m.doa b ol)) o1));
 
- inter_left_1op_b : l:st_b -> a:st_b -> b:st_b -> o1:op_b -> ob:op_b -> ol:op_b -> o:op_b ->
-   Lemma (requires Fst_then_snd? (m.rc_b ob ol) /\ get_rid ob <> get_rid ol /\
-                    (~ (Either? (m.rc_b o ob)) \/ Fst_then_snd? (m.rc_b o ol)) /\
-                    distinct_ops o1 ob /\ distinct_ops o1 ol /\ distinct_ops o1 o /\ distinct_ops ob ol /\ distinct_ops ob o /\ distinct_ops ol o /\
-                    get_rid o <> get_rid ol /\
-                    m.eq_b (m.merge_b (m.do_b l ol) (m.do_b (m.do_b (m.do_b a ob) ol) o1) (m.do_b b ol)) (m.do_b (m.merge_b (m.do_b l ol) (m.do_b (m.do_b a ob) ol) (m.do_b b ol)) o1))
-         (ensures m.eq_b (m.merge_b (m.do_b l ol) (m.do_b (m.do_b (m.do_b (m.do_b a o) ob) ol) o1) (m.do_b b ol)) (m.do_b (m.merge_b (m.do_b l ol) (m.do_b (m.do_b (m.do_b a o) ob) ol) (m.do_b b ol)) o1));
+ inter_left_1opb : l:stb -> a:stb -> b:stb -> o1:L.op #ob -> ob':L.op #ob -> ol:L.op #ob -> o:L.op #ob ->
+   Lemma (requires L.Fst_then_snd? (m.rcb ob' ol) /\ L.get_rid ob' <> L.get_rid ol /\
+                   (~ (L.Either? (m.rcb o ob')) \/ L.Fst_then_snd? (m.rcb o ol)) /\
+                   L.distinct_ops o1 ob' /\ L.distinct_ops o1 ol /\ L.distinct_ops o1 o /\ 
+                   L.distinct_ops ob' ol /\ L.distinct_ops ob' o /\ L.distinct_ops ol o /\
+                   L.get_rid o <> L.get_rid ol /\
+                   m.eqb (m.mergeb (m.dob l ol) (m.dob (m.dob (m.dob a ob') ol) o1) (m.dob b ol)) 
+                         (m.dob (m.mergeb (m.dob l ol) (m.dob (m.dob a ob') ol) (m.dob b ol)) o1))
+         (ensures m.eqb (m.mergeb (m.dob l ol) (m.dob (m.dob (m.dob (m.dob a o) ob') ol) o1) (m.dob b ol)) 
+                        (m.dob (m.mergeb (m.dob l ol) (m.dob (m.dob (m.dob a o) ob') ol) (m.dob b ol)) o1));
 
- ind_right_1op_a : l:st_a -> a:st_a -> b:st_a -> o2:op_a -> o2':op_a -> ol:op_a ->
-   Lemma (requires distinct_ops o2 o2' /\ distinct_ops o2 ol /\ distinct_ops o2' ol /\
-                    m.eq_a (m.merge_a (m.do_a l ol) (m.do_a a ol) (m.do_a b o2)) (m.do_a (m.merge_a (m.do_a l ol) (m.do_a a ol) b) o2))
-         (ensures m.eq_a (m.merge_a (m.do_a l ol) (m.do_a a ol) (m.do_a (m.do_a b o2') o2)) (m.do_a (m.merge_a (m.do_a l ol) (m.do_a a ol) (m.do_a b o2')) o2));
+ ind_right_1opa : l:sta -> a:sta -> b:sta -> o2:L.op #oa -> o2':L.op #oa -> ol:L.op #oa ->
+   Lemma (requires L.distinct_ops o2 o2' /\ L.distinct_ops o2 ol /\ L.distinct_ops o2' ol /\
+                   m.eqa (m.mergea (m.doa l ol) (m.doa a ol) (m.doa b o2)) (m.doa (m.mergea (m.doa l ol) (m.doa a ol) b) o2))
+         (ensures m.eqa (m.mergea (m.doa l ol) (m.doa a ol) (m.doa (m.doa b o2') o2)) 
+                        (m.doa (m.mergea (m.doa l ol) (m.doa a ol) (m.doa b o2')) o2));
 
- ind_right_1op_b : l:st_b -> a:st_b -> b:st_b -> o2:op_b -> o2':op_b -> ol:op_b -> 
-   Lemma (requires distinct_ops o2 o2' /\ distinct_ops o2 ol /\ distinct_ops o2' ol /\
-                    m.eq_b (m.merge_b (m.do_b l ol) (m.do_b a ol) (m.do_b b o2)) (m.do_b (m.merge_b (m.do_b l ol) (m.do_b a ol) b) o2))
-         (ensures m.eq_b (m.merge_b (m.do_b l ol) (m.do_b a ol) (m.do_b (m.do_b b o2') o2)) (m.do_b (m.merge_b (m.do_b l ol) (m.do_b a ol) (m.do_b b o2')) o2));
+ ind_right_1opb : l:stb -> a:stb -> b:stb -> o2:L.op #ob -> o2':L.op #ob -> ol:L.op #ob -> 
+   Lemma (requires L.distinct_ops o2 o2' /\ L.distinct_ops o2 ol /\ L.distinct_ops o2' ol /\
+                   m.eqb (m.mergeb (m.dob l ol) (m.dob a ol) (m.dob b o2)) (m.dob (m.mergeb (m.dob l ol) (m.dob a ol) b) o2))
+         (ensures m.eqb (m.mergeb (m.dob l ol) (m.dob a ol) (m.dob (m.dob b o2') o2)) 
+                        (m.dob (m.mergeb (m.dob l ol) (m.dob a ol) (m.dob b o2')) o2));
 
- ind_right_1op' : l:st -> a:st -> b:st -> o2:op -> o2':op -> ol:op ->
-   Lemma (requires distinct_ops o2 o2' /\ distinct_ops o2 ol /\ distinct_ops o2' ol /\
+ ind_right_1op' : l:st -> a:st -> b:st -> o2:jop -> o2':jop -> ol:jop ->
+   Lemma (requires L.distinct_ops o2 o2' /\ L.distinct_ops o2 ol /\ L.distinct_ops o2' ol /\
                    ~ (get_key o2 = get_key o2' /\ get_key o2 = get_key ol /\
                    is_alpha_op o2 /\ is_alpha_op o2' /\ is_alpha_op ol /\
                    is_beta_op o2 /\ is_beta_op o2' /\ is_beta_op ol) /\
                    eq (merge (do l ol) (do a ol) (do b o2)) (do (merge (do l ol) (do a ol) b) o2))
-         (ensures eq (merge (do l ol) (do a ol) (do (do b o2') o2)) (do #st_a #st_b #o_a #o_b #m (merge (do l ol) (do a ol) (do b o2')) o2));
+         (ensures eq (merge (do l ol) (do a ol) (do (do b o2') o2)) 
+                     (do #sta #stb #oa #ob #m (merge (do l ol) (do a ol) (do b o2')) o2));
           
- ind_left_1op_a : l:st_a -> a:st_a -> b:st_a -> o1:op_a -> o1':op_a -> ol:op_a ->
-   Lemma (requires distinct_ops o1 o1' /\ distinct_ops o1 ol /\ distinct_ops o1' ol /\
-                    m.eq_a (m.merge_a (m.do_a l ol) (m.do_a a o1) (m.do_a b ol)) (m.do_a (m.merge_a (m.do_a l ol) a (m.do_a b ol)) o1))
-         (ensures m.eq_a (m.merge_a (m.do_a l ol) (m.do_a (m.do_a a o1') o1) (m.do_a b ol)) (m.do_a (m.merge_a (m.do_a l ol) (m.do_a a o1') (m.do_a b ol)) o1));
+ ind_left_1opa : l:sta -> a:sta -> b:sta -> o1:L.op #oa -> o1':L.op #oa -> ol:L.op #oa ->
+   Lemma (requires L.distinct_ops o1 o1' /\ L.distinct_ops o1 ol /\ L.distinct_ops o1' ol /\
+                   m.eqa (m.mergea (m.doa l ol) (m.doa a o1) (m.doa b ol)) (m.doa (m.mergea (m.doa l ol) a (m.doa b ol)) o1))
+         (ensures m.eqa (m.mergea (m.doa l ol) (m.doa (m.doa a o1') o1) (m.doa b ol)) (m.doa (m.mergea (m.doa l ol) (m.doa a o1') (m.doa b ol)) o1));
 
- ind_left_1op_b : l:st_b -> a:st_b -> b:st_b -> o1:op_b -> o1':op_b -> ol:op_b -> 
-   Lemma (requires distinct_ops o1 o1' /\ distinct_ops o1 ol /\ distinct_ops o1' ol /\
-                    m.eq_b (m.merge_b (m.do_b l ol) (m.do_b a o1) (m.do_b b ol)) (m.do_b (m.merge_b (m.do_b l ol) a (m.do_b b ol)) o1))
-         (ensures m.eq_b (m.merge_b (m.do_b l ol) (m.do_b (m.do_b a o1') o1) (m.do_b b ol)) (m.do_b (m.merge_b (m.do_b l ol) (m.do_b a o1') (m.do_b b ol)) o1));
+ ind_left_1opb : l:stb -> a:stb -> b:stb -> o1:L.op #ob -> o1':L.op #ob -> ol:L.op #ob -> 
+   Lemma (requires L.distinct_ops o1 o1' /\ L.distinct_ops o1 ol /\ L.distinct_ops o1' ol /\
+                   m.eqb (m.mergeb (m.dob l ol) (m.dob a o1) (m.dob b ol)) (m.dob (m.mergeb (m.dob l ol) a (m.dob b ol)) o1))
+         (ensures m.eqb (m.mergeb (m.dob l ol) (m.dob (m.dob a o1') o1) (m.dob b ol)) 
+                        (m.dob (m.mergeb (m.dob l ol) (m.dob a o1') (m.dob b ol)) o1));
 
- ind_left_1op' : l:st -> a:st -> b:st -> o1:op -> o1':op -> ol:op ->
-   Lemma (requires distinct_ops o1 o1' /\ distinct_ops o1 ol /\ distinct_ops o1' ol /\
+ ind_left_1op' : l:st -> a:st -> b:st -> o1:jop -> o1':jop -> ol:jop ->
+   Lemma (requires L.distinct_ops o1 o1' /\ L.distinct_ops o1 ol /\ L.distinct_ops o1' ol /\
                    ~ (get_key o1 = get_key o1' /\ get_key o1 = get_key ol /\
                    is_alpha_op o1 /\ is_alpha_op o1' /\ is_alpha_op ol /\
                    is_beta_op o1 /\ is_beta_op o1' /\ is_beta_op ol) /\
                    eq (merge (do l ol) (do a o1) (do b ol)) (do (merge (do l ol) a (do b ol)) o1))
-         (ensures eq (merge (do l ol) (do (do a o1') o1) (do b ol)) (do #st_a #st_b #o_a #o_b #m (merge (do l ol) (do a o1') (do b ol)) o1));
+         (ensures eq (merge (do l ol) (do (do a o1') o1) (do b ol)) 
+                     (do #sta #stb #oa #ob #m (merge (do l ol) (do a o1') (do b ol)) o1));
           
- lem_0op_a : l:st_a -> a:st_a -> b:st_a -> ol:op_a  ->
-   Lemma (ensures m.eq_a (m.merge_a (m.do_a l ol) (m.do_a a ol) (m.do_a b ol)) (m.do_a (m.merge_a l a b) ol));
+ lem_0opa : l:sta -> a:sta -> b:sta -> ol:L.op #oa  ->
+   Lemma (ensures m.eqa (m.mergea (m.doa l ol) (m.doa a ol) (m.doa b ol)) (m.doa (m.mergea l a b) ol));
 
- lem_0op_b : l:st_b -> a:st_b -> b:st_b -> ol:op_b ->
-   Lemma (ensures m.eq_b (m.merge_b (m.do_b l ol) (m.do_b a ol) (m.do_b b ol)) (m.do_b (m.merge_b l a b) ol))
+ lem_0opb : l:stb -> a:stb -> b:stb -> ol:L.op #ob ->
+   Lemma (ensures m.eqb (m.mergeb (m.dob l ol) (m.dob a ol) (m.dob b ol)) (m.dob (m.mergeb l a b) ol))
 }
 
-val comma : #st_a:Type0 -> #st_b:Type0 -> #o_a:eqtype -> #o_b:eqtype -> #m:(json st_a st_b o_a o_b) -> #v:(vc st_a st_b o_a o_b m) -> l:st_a -> a:st_a -> b:st_a ->
-  Lemma (ensures (m.eq_a (m.merge_a l a b) (m.merge_a l b a))) 
-        [SMTPat (m.merge_a l a b)]        
-let comma #st_a #st_b #o_a #o_b #m #v l a b = 
-  v.merge_comm_a l a b
+val comma : #sta:Type0 -> #stb:Type0 -> #oa:eqtype -> #ob:eqtype -> #m:(json sta stb oa ob) -> #v:(vc sta stb oa ob m) -> 
+            l:sta -> a:sta -> b:sta ->
+  Lemma (ensures (m.eqa (m.mergea l a b) (m.mergea l b a))) 
+        [SMTPat (m.mergea l a b)]        
+let comma #sta #stb #oa #ob #m #v l a b = v.merge_comm_a l a b
 
-val commb : #st_a:Type0 -> #st_b:Type0 -> #o_a:eqtype -> #o_b:eqtype -> #m:(json st_a st_b o_a o_b) -> #v:(vc st_a st_b o_a o_b m) -> l:st_b -> a:st_b -> b:st_b ->
-  Lemma (ensures (m.eq_b (m.merge_b l a b) (m.merge_b l b a))) 
-        [SMTPat (m.merge_b l a b)]       
-let commb #st_a #st_b #o_a #o_b #m #v l a b = 
-  v.merge_comm_b l a b
+val commb : #sta:Type0 -> #stb:Type0 -> #oa:eqtype -> #ob:eqtype -> #m:(json sta stb oa ob) -> #v:(vc sta stb oa ob m) -> 
+            l:stb -> a:stb -> b:stb ->
+  Lemma (ensures (m.eqb (m.mergeb l a b) (m.mergeb l b a))) 
+        [SMTPat (m.mergeb l a b)]       
+let commb #sta #stb #oa #ob #m #v l a b = v.merge_comm_b l a b
 
-val idema : #st_a:Type0 -> #st_b:Type0 -> #o_a:eqtype -> #o_b:eqtype -> #m:(json st_a st_b o_a o_b) -> #v:(vc st_a st_b o_a o_b m) -> s:st_a ->
-  Lemma (ensures (m.eq_a (m.merge_a s s s) s)) 
-        [SMTPat (m.merge_a s s s)]        
-let idema #st_a #st_b #o_a #o_b #m #v s = 
-  v.merge_idem_a s
+val idema : #sta:Type0 -> #stb:Type0 -> #oa:eqtype -> #ob:eqtype -> #m:(json sta stb oa ob) -> #v:(vc sta stb oa ob m) -> s:sta ->
+  Lemma (ensures (m.eqa (m.mergea s s s) s)) 
+        [SMTPat (m.mergea s s s)]        
+let idema #sta #stb #oa #ob #m #v s = v.merge_idem_a s
 
-val idemb : #st_a:Type0 -> #st_b:Type0 -> #o_a:eqtype -> #o_b:eqtype -> #m:(json st_a st_b o_a o_b) -> #v:(vc st_a st_b o_a o_b m) -> s:st_b ->
-  Lemma (ensures (m.eq_b (m.merge_b s s s) s)) 
-        [SMTPat (m.merge_b s s s)]        
-let idemb #st_a #st_b #o_a #o_b #m #v s = 
-  v.merge_idem_b s
+val idemb : #sta:Type0 -> #stb:Type0 -> #oa:eqtype -> #ob:eqtype -> #m:(json sta stb oa ob) -> #v:(vc sta stb oa ob m) -> s:stb ->
+  Lemma (ensures (m.eqb (m.mergeb s s s) s)) 
+        [SMTPat (m.mergeb s s s)]        
+let idemb #sta #stb #oa #ob #m #v s = v.merge_idem_b s
   
-val merge_comm : #st_a:Type0 -> #st_b:Type0 -> #o_a:eqtype -> #o_b:eqtype -> #m:(json st_a st_b o_a o_b) -> #v:(vc st_a st_b o_a o_b m) -> l:st #st_a #st_b #o_a #o_b #m -> a:st #st_a #st_b #o_a #o_b #m -> b:st #st_a #st_b #o_a #o_b #m ->
+val merge_comm : #sta:Type0 -> #stb:Type0 -> #oa:eqtype -> #ob:eqtype -> #m:(json sta stb oa ob) -> #v:(vc sta stb oa ob m) -> l:st #sta #stb #oa #ob #m -> a:st #sta #stb #oa #ob #m -> b:st #sta #stb #oa #ob #m ->
   Lemma (ensures (eq (merge l a b) (merge l b a)))
-let merge_comm #st_a #st_b #o_a #o_b #m #v l a b 
-  :  Lemma (ensures (eq (merge l a b) (merge l b a))) = ()
+let merge_comm #sta #stb #oa #ob #m #v l a b = ()
 
-val merge_idem : #st_a:Type0 -> #st_b:Type0 -> #o_a:eqtype -> #o_b:eqtype -> #m:(json st_a st_b o_a o_b) -> #v:(vc st_a st_b o_a o_b m) -> s:st #st_a #st_b #o_a #o_b #m -> 
+val merge_idem : #sta:Type0 -> #stb:Type0 -> #oa:eqtype -> #ob:eqtype -> #m:(json sta stb oa ob) -> #v:(vc sta stb oa ob m) -> s:st #sta #stb #oa #ob #m -> 
   Lemma (ensures (eq (merge s s s) s))
-let merge_idem #st_a #st_b #o_a #o_b #m #v s
-  :  Lemma (ensures (eq (merge s s s) s)) = ()
+let merge_idem #sta #stb #oa #ob #m #v s = ()
 
-val base_2op : #st_a:Type0 -> #st_b:Type0 -> #o_a:eqtype -> #o_b:eqtype -> #m:(json st_a st_b o_a o_b) -> #v:(vc st_a st_b o_a o_b m) -> o1:op -> o2:op -> t:kt -> 
-  Lemma (requires (Fst_then_snd? (rc #st_a #st_b #o_a #o_b #m o2 o1) \/ Either? (rc #st_a #st_b #o_a #o_b #m o2 o1)) /\ get_rid o1 <> get_rid o2 /\
-                    distinct_ops o1 o2)
-          (ensures eq (merge (init_st t) (do (init_st t) o1) (do (init_st t) o2)) 
-                      (do #st_a #st_b #o_a #o_b #m (merge (init_st t) (init_st t) (do (init_st t) o2)) o1))                     
-let base_2op #st_a #st_b #o_a #o_b #m #v o1 o2 t =
+val base_2op : #sta:Type0 -> #stb:Type0 -> #oa:eqtype -> #ob:eqtype -> #m:(json sta stb oa ob) -> #v:(vc sta stb oa ob m) -> 
+               o1:jop -> o2:jop -> t:kt -> 
+  Lemma (requires (L.Fst_then_snd? (rc #sta #stb #oa #ob #m o2 o1) \/ L.Either? (rc #sta #stb #oa #ob #m o2 o1)) /\ 
+                   L.get_rid o1 <> L.get_rid o2 /\ L.distinct_ops o1 o2)
+        (ensures eq (merge (init_st t) (do (init_st t) o1) (do (init_st t) o2)) 
+                    (do #sta #stb #oa #ob #m (merge (init_st t) (init_st t) (do (init_st t) o2)) o1))                     
+let base_2op #sta #stb #oa #ob #m #v o1 o2 t =
   if get_key o1 = get_key o2 && is_alpha_op o1 && is_alpha_op o2 then
-    v.base_2op_a (get_op_a o1) (get_op_a o2) 
+    v.base_2opa (get_opa o1) (get_opa o2) 
   else if get_key o1 = get_key o2 && is_beta_op o1 && is_beta_op o2 then
-    v.base_2op_b (get_op_b o1) (get_op_b o2) 
-  else if Either? (rc #st_a #st_b #o_a #o_b #m o2 o1) then v.base_2op' o1 o2 t
+    v.base_2opb (get_opb o1) (get_opb o2) 
+  else if L.Either? (rc #sta #stb #oa #ob #m o2 o1) then v.base_2op' o1 o2 t
   else ()
 
-val ind_lca_2op : #st_a:Type0 -> #st_b:Type0 -> #o_a:eqtype -> #o_b:eqtype -> #m:(json st_a st_b o_a o_b) -> #v:(vc st_a st_b o_a o_b m) -> l:st #st_a #st_b #o_a #o_b #m -> o1:op -> o2:op -> ol:op ->
-  Lemma (requires (Fst_then_snd? (rc #st_a #st_b #o_a #o_b #m o2 o1) \/ Either? (rc #st_a #st_b #o_a #o_b #m o2 o1)) /\ get_rid o1 <> get_rid o2 /\
-                    distinct_ops o1 o2 /\ distinct_ops o1 ol /\ distinct_ops o2 ol /\
-                    eq (merge l (do l o1) (do l o2)) (do (merge l l (do l o2)) o1))
-          (ensures eq (merge (do l ol) (do (do l ol) o1) (do (do l ol) o2)) (do (merge (do l ol) (do l ol) (do (do l ol) o2)) o1))
-          
-let ind_lca_2op #st_a #st_b #o_a #o_b #m #v l o1 o2 ol =
+val ind_lca_2op : #sta:Type0 -> #stb:Type0 -> #oa:eqtype -> #ob:eqtype -> #m:(json sta stb oa ob) -> #v:(vc sta stb oa ob m) -> 
+                  l:st #sta #stb #oa #ob #m -> o1:jop -> o2:jop -> ol:jop ->
+  Lemma (requires (L.Fst_then_snd? (rc #sta #stb #oa #ob #m o2 o1) \/ L.Either? (rc #sta #stb #oa #ob #m o2 o1)) /\ 
+                   L.get_rid o1 <> L.get_rid o2 /\ L.distinct_ops o1 o2 /\ L.distinct_ops o1 ol /\ L.distinct_ops o2 ol /\
+                   eq (merge l (do l o1) (do l o2)) (do (merge l l (do l o2)) o1))
+        (ensures eq (merge (do l ol) (do (do l ol) o1) (do (do l ol) o2)) (do (merge (do l ol) (do l ol) (do (do l ol) o2)) o1))
+let ind_lca_2op #sta #stb #oa #ob #m #v l o1 o2 ol =
   let k = get_key ol in
   let ka = Alpha_t k in let kb = Beta_t k in
-  if get_key o1 = k && get_key o2 = k && is_alpha_op o1 && is_alpha_op o2 && is_alpha_op ol && (Fst_then_snd? (m.rc_a (get_op_a o2) (get_op_a o1)) || Either? (m.rc_a (get_op_a o2) (get_op_a o1))) then
-      v.ind_lca_2op_a (sel l ka) (get_op_a o1) (get_op_a o2) (get_op_a ol)
-  else if get_key o1 = k && get_key o2 = k && is_beta_op o1 && is_beta_op o2 && is_beta_op ol && (Fst_then_snd? (m.rc_b (get_op_b o2) (get_op_b o1)) || Either? (m.rc_b (get_op_b o2) (get_op_b o1))) then
-      v.ind_lca_2op_b (sel l kb) (get_op_b o1) (get_op_b o2) (get_op_b ol)
-  else if Either? (rc #st_a #st_b #o_a #o_b #m o2 o1) then v.ind_lca_2op' l o1 o2 ol
+  if get_key o1 = k && get_key o2 = k && is_alpha_op o1 && is_alpha_op o2 && is_alpha_op ol && (L.Fst_then_snd? (m.rca (get_opa o2) (get_opa o1)) || L.Either? (m.rca (get_opa o2) (get_opa o1))) then
+      v.ind_lca_2opa (sel l ka) (get_opa o1) (get_opa o2) (get_opa ol)
+  else if get_key o1 = k && get_key o2 = k && is_beta_op o1 && is_beta_op o2 && is_beta_op ol && (L.Fst_then_snd? (m.rcb (get_opb o2) (get_opb o1)) || L.Either? (m.rcb (get_opb o2) (get_opb o1))) then
+      v.ind_lca_2opb (sel l kb) (get_opb o1) (get_opb o2) (get_opb ol)
+  else if L.Either? (rc #sta #stb #oa #ob #m o2 o1) then v.ind_lca_2op' l o1 o2 ol
   else ()
 
-val inter_right_base_2op : #st_a:Type0 -> #st_b:Type0 -> #o_a:eqtype -> #o_b:eqtype -> #m:(json st_a st_b o_a o_b) -> #v:(vc st_a st_b o_a o_b m) -> l:st #st_a #st_b #o_a #o_b #m -> a:st -> b:st -> o1:op -> o2:op -> ob:op -> ol:op ->
-  Lemma (requires (Fst_then_snd? (rc #st_a #st_b #o_a #o_b #m o2 o1) \/ Either? (rc #st_a #st_b #o_a #o_b #m o2 o1)) /\ get_rid o1 <> get_rid o2 /\ Fst_then_snd? (rc #st_a #st_b #o_a #o_b #m ob ol) /\ get_rid ob <> get_rid ol /\
-                    distinct_ops o1 o2 /\ distinct_ops o1 ob /\ distinct_ops o1 ol /\ distinct_ops o2 ob /\ distinct_ops o2 ol /\ distinct_ops ob ol /\
-                    eq (merge l (do a o1) (do b o2)) (do (merge l a (do b o2)) o1) /\ //from pre-cond of ind_right_2op
-                    eq (merge l (do a o1) (do (do b ob) o2)) (do (merge l a (do (do b ob) o2)) o1) /\ //from ind_right_2op
-                    eq (merge (do l ol) (do (do a ol) o1) (do (do b ol) o2)) (do (merge (do l ol) (do a ol) (do (do b ol) o2)) o1))
-          (ensures eq (merge (do l ol) (do (do a ol) o1) (do (do (do b ob) ol) o2)) (do (merge (do l ol) (do a ol) (do (do (do b ob) ol) o2)) o1))
-          
-let inter_right_base_2op #st_a #st_b #o_a #o_b #m #v l a b o1 o2 ob ol =
+val inter_right_base_2op : #sta:Type0 -> #stb:Type0 -> #oa:eqtype -> #ob:eqtype -> #m:(json sta stb oa ob) -> #v:(vc sta stb oa ob m) ->
+                           l:st #sta #stb #oa #ob #m -> a:st -> b:st -> o1:jop -> o2:jop -> ob':jop -> ol:jop ->
+  Lemma (requires (L.Fst_then_snd? (rc #sta #stb #oa #ob #m o2 o1) \/ L.Either? (rc #sta #stb #oa #ob #m o2 o1)) /\ 
+                   L.get_rid o1 <> L.get_rid o2 /\ L.Fst_then_snd? (rc #sta #stb #oa #ob #m ob' ol) /\ L.get_rid ob' <> L.get_rid ol /\
+                   L.distinct_ops o1 o2 /\ L.distinct_ops o1 ob' /\ L.distinct_ops o1 ol /\ 
+                   L.distinct_ops o2 ob' /\ L.distinct_ops o2 ol /\ L.distinct_ops ob' ol /\
+                   eq (merge l (do a o1) (do b o2)) (do (merge l a (do b o2)) o1) /\ //from pre-cond of ind_right_2op
+                   eq (merge l (do a o1) (do (do b ob') o2)) (do (merge l a (do (do b ob') o2)) o1) /\ //from ind_right_2op
+                   eq (merge (do l ol) (do (do a ol) o1) (do (do b ol) o2)) (do (merge (do l ol) (do a ol) (do (do b ol) o2)) o1))
+        (ensures eq (merge (do l ol) (do (do a ol) o1) (do (do (do b ob') ol) o2)) (do (merge (do l ol) (do a ol) (do (do (do b ob') ol) o2)) o1))         
+let inter_right_base_2op #sta #stb #oa #ob #m #v l a b o1 o2 ob' ol =
   let k = get_key ol in
   let ka = Alpha_t k in let kb = Beta_t k in
-  if get_key o1 = k && get_key o2 = k && get_key ob = k && is_alpha_op o1 && is_alpha_op o2 && is_alpha_op ob && is_alpha_op ol && (Fst_then_snd? (m.rc_a (get_op_a o2) (get_op_a o1)) || Either? (m.rc_a (get_op_a o2) (get_op_a o1))) && Fst_then_snd? (m.rc_a (get_op_a ob) (get_op_a ol)) then
-      v.inter_right_base_2op_a (sel l ka) (sel a ka) (sel b ka) (get_op_a o1) (get_op_a o2) (get_op_a ob) (get_op_a ol)
-  else if get_key o1 = k && get_key o2 = k && get_key ob = k && is_beta_op o1 && is_beta_op o2 && is_beta_op ob && is_beta_op ol && (Fst_then_snd? (m.rc_b (get_op_b o2) (get_op_b o1)) || Either? (m.rc_b (get_op_b o2) (get_op_b o1))) && Fst_then_snd? (m.rc_b (get_op_b ob) (get_op_b ol)) then
-      v.inter_right_base_2op_b (sel l kb) (sel a kb) (sel b kb) (get_op_b o1) (get_op_b o2) (get_op_b ob) (get_op_b ol)
-  else if Either? (rc #st_a #st_b #o_a #o_b #m o2 o1) then v.inter_right_base_2op' l a b o1 o2 ob ol
+  if get_key o1 = k && get_key o2 = k && get_key ob' = k && is_alpha_op o1 && is_alpha_op o2 && is_alpha_op ob' && is_alpha_op ol && (L.Fst_then_snd? (m.rca (get_opa o2) (get_opa o1)) || L.Either? (m.rca (get_opa o2) (get_opa o1))) && L.Fst_then_snd? (m.rca (get_opa ob') (get_opa ol)) then
+      v.inter_right_base_2opa (sel l ka) (sel a ka) (sel b ka) (get_opa o1) (get_opa o2) (get_opa ob') (get_opa ol)
+  else if get_key o1 = k && get_key o2 = k && get_key ob' = k && is_beta_op o1 && is_beta_op o2 && is_beta_op ob' && is_beta_op ol && (L.Fst_then_snd? (m.rcb (get_opb o2) (get_opb o1)) || L.Either? (m.rcb (get_opb o2) (get_opb o1))) && L.Fst_then_snd? (m.rcb (get_opb ob') (get_opb ol)) then
+      v.inter_right_base_2opb (sel l kb) (sel a kb) (sel b kb) (get_opb o1) (get_opb o2) (get_opb ob') (get_opb ol)
+  else if L.Either? (rc #sta #stb #oa #ob #m o2 o1) then v.inter_right_base_2op' l a b o1 o2 ob' ol
   else ()
 
-val inter_left_base_2op : #st_a:Type0 -> #st_b:Type0 -> #o_a:eqtype -> #o_b:eqtype -> #m:(json st_a st_b o_a o_b) -> #v:(vc st_a st_b o_a o_b m) -> l:st #st_a #st_b #o_a #o_b #m -> a:st -> b:st -> o1:op -> o2:op -> ob:op -> ol:op ->
-  Lemma (requires (Fst_then_snd? (rc #st_a #st_b #o_a #o_b #m o2 o1) \/ Either? (rc #st_a #st_b #o_a #o_b #m o2 o1)) /\ get_rid o1 <> get_rid o2 /\ Fst_then_snd? (rc #st_a #st_b #o_a #o_b #m ob ol) /\ get_rid ob <> get_rid ol /\
-                    distinct_ops o1 o2 /\ distinct_ops o1 ob /\ distinct_ops o1 ol /\ distinct_ops o2 ob /\ distinct_ops o2 ol /\ distinct_ops ob ol /\
-                    eq (merge (do l ol) (do (do a ol) o1) (do (do b ol) o2)) (do (merge (do l ol) (do a ol) (do (do b ol) o2)) o1))
-          (ensures eq (merge (do l ol) (do (do (do a ob) ol) o1) (do (do b ol) o2)) (do (merge (do l ol) (do (do a ob) ol) (do (do b ol) o2)) o1))
-          
-let inter_left_base_2op #st_a #st_b #o_a #o_b #m #v l a b o1 o2 ob ol =
+val inter_left_base_2op : #sta:Type0 -> #stb:Type0 -> #oa:eqtype -> #ob:eqtype -> #m:(json sta stb oa ob) -> #v:(vc sta stb oa ob m) ->
+                          l:st #sta #stb #oa #ob #m -> a:st -> b:st -> o1:jop -> o2:jop -> ob':jop -> ol:jop ->
+  Lemma (requires (L.Fst_then_snd? (rc #sta #stb #oa #ob #m o2 o1) \/ L.Either? (rc #sta #stb #oa #ob #m o2 o1)) /\ 
+                   L.get_rid o1 <> L.get_rid o2 /\ L.Fst_then_snd? (rc #sta #stb #oa #ob #m ob' ol) /\ L.get_rid ob' <> L.get_rid ol /\
+                   L.distinct_ops o1 o2 /\ L.distinct_ops o1 ob' /\ L.distinct_ops o1 ol /\ 
+                   L.distinct_ops o2 ob' /\ L.distinct_ops o2 ol /\ L.distinct_ops ob' ol /\
+                   eq (merge (do l ol) (do (do a ol) o1) (do (do b ol) o2)) (do (merge (do l ol) (do a ol) (do (do b ol) o2)) o1))
+        (ensures eq (merge (do l ol) (do (do (do a ob') ol) o1) (do (do b ol) o2)) 
+                    (do (merge (do l ol) (do (do a ob') ol) (do (do b ol) o2)) o1))         
+let inter_left_base_2op #sta #stb #oa #ob #m #v l a b o1 o2 ob' ol =
   let k = get_key ol in
   let ka = Alpha_t k in let kb = Beta_t k in
-  if get_key o1 = k && get_key o2 = k && get_key ob = k && is_alpha_op o1 && is_alpha_op o2 && is_alpha_op ob && is_alpha_op ol && (Fst_then_snd? (m.rc_a (get_op_a o2) (get_op_a o1)) || Either? (m.rc_a (get_op_a o2) (get_op_a o1))) && Fst_then_snd? (m.rc_a (get_op_a ob) (get_op_a ol)) then
-      v.inter_left_base_2op_a (sel l ka) (sel a ka) (sel b ka) (get_op_a o1) (get_op_a o2) (get_op_a ob) (get_op_a ol)
-  else if get_key o1 = k && get_key o2 = k && get_key ob = k && is_beta_op o1 && is_beta_op o2 && is_beta_op ob && is_beta_op ol && (Fst_then_snd? (m.rc_b (get_op_b o2) (get_op_b o1)) || Either? (m.rc_b (get_op_b o2) (get_op_b o1))) && Fst_then_snd? (m.rc_b (get_op_b ob) (get_op_b ol)) then
-      v.inter_left_base_2op_b (sel l kb) (sel a kb) (sel b kb) (get_op_b o1) (get_op_b o2) (get_op_b ob) (get_op_b ol)
-  else if Either? (rc #st_a #st_b #o_a #o_b #m o2 o1) then v.inter_left_base_2op' l a b o1 o2 ob ol
+  if get_key o1 = k && get_key o2 = k && get_key ob' = k && is_alpha_op o1 && is_alpha_op o2 && is_alpha_op ob' && is_alpha_op ol && (L.Fst_then_snd? (m.rca (get_opa o2) (get_opa o1)) || L.Either? (m.rca (get_opa o2) (get_opa o1))) && L.Fst_then_snd? (m.rca (get_opa ob') (get_opa ol)) then
+      v.inter_left_base_2opa (sel l ka) (sel a ka) (sel b ka) (get_opa o1) (get_opa o2) (get_opa ob') (get_opa ol)
+  else if get_key o1 = k && get_key o2 = k && get_key ob' = k && is_beta_op o1 && is_beta_op o2 && is_beta_op ob' && is_beta_op ol && (L.Fst_then_snd? (m.rcb (get_opb o2) (get_opb o1)) || L.Either? (m.rcb (get_opb o2) (get_opb o1))) && L.Fst_then_snd? (m.rcb (get_opb ob') (get_opb ol)) then
+      v.inter_left_base_2opb (sel l kb) (sel a kb) (sel b kb) (get_opb o1) (get_opb o2) (get_opb ob') (get_opb ol)
+  else if L.Either? (rc #sta #stb #oa #ob #m o2 o1) then v.inter_left_base_2op' l a b o1 o2 ob' ol
   else ()
 
-val inter_right_2op : #st_a:Type0 -> #st_b:Type0 -> #o_a:eqtype -> #o_b:eqtype -> #m:(json st_a st_b o_a o_b) -> #v:(vc st_a st_b o_a o_b m) -> l:st #st_a #st_b #o_a #o_b #m -> a:st -> b:st -> o1:op -> o2:op -> ob:op -> ol:op -> o:op ->
-  Lemma (requires (Fst_then_snd? (rc #st_a #st_b #o_a #o_b #m o2 o1) \/ Either? (rc #st_a #st_b #o_a #o_b #m o2 o1)) /\ get_rid o1 <> get_rid o2 /\ Fst_then_snd? (rc #st_a #st_b #o_a #o_b #m ob ol) /\ get_rid ob <> get_rid ol /\
-                    (~ (Either? (rc #st_a #st_b #o_a #o_b #m o ob)) \/ Fst_then_snd? (rc #st_a #st_b #o_a #o_b #m o ol)) /\               
-                    distinct_ops o1 o2 /\ distinct_ops o1 ob /\ distinct_ops o1 ol /\ distinct_ops o1 o /\ distinct_ops o2 ob /\ distinct_ops o2 ol /\ distinct_ops o2 o /\ distinct_ops ob ol /\ distinct_ops ob o /\ distinct_ops ol o /\
-                    get_rid o <> get_rid ol /\ //from app.fsti
-                    eq (merge (do l ol) (do (do a ol) o1) (do (do (do b ob) ol) o2)) (do (merge (do l ol) (do a ol) (do (do (do b ob) ol) o2)) o1))
-          (ensures eq (merge (do l ol) (do (do a ol) o1) (do (do (do (do b o) ob) ol) o2)) (do (merge (do l ol) (do a ol) (do (do (do (do b o) ob) ol) o2)) o1))
-          
-let inter_right_2op #st_a #st_b #o_a #o_b #m #v l a b o1 o2 ob ol o =
+val inter_right_2op : #sta:Type0 -> #stb:Type0 -> #oa:eqtype -> #ob:eqtype -> #m:(json sta stb oa ob) -> #v:(vc sta stb oa ob m) -> 
+                      l:st #sta #stb #oa #ob #m -> a:st -> b:st -> o1:jop -> o2:jop -> ob':jop -> ol:jop -> o:jop ->
+  Lemma (requires (L.Fst_then_snd? (rc #sta #stb #oa #ob #m o2 o1) \/ L.Either? (rc #sta #stb #oa #ob #m o2 o1)) /\ 
+                   L.get_rid o1 <> L.get_rid o2 /\ L.Fst_then_snd? (rc #sta #stb #oa #ob #m ob' ol) /\ L.get_rid ob' <> L.get_rid ol /\
+                   (~ (L.Either? (rc #sta #stb #oa #ob #m o ob')) \/ L.Fst_then_snd? (rc #sta #stb #oa #ob #m o ol)) /\               
+                   L.distinct_ops o1 o2 /\ L.distinct_ops o1 ob' /\ L.distinct_ops o1 ol /\ L.distinct_ops o1 o /\ L.distinct_ops o2 ob' /\
+                   L.distinct_ops o2 ol /\ L.distinct_ops o2 o /\ L.distinct_ops ob' ol /\ L.distinct_ops ob' o /\ L.distinct_ops ol o /\
+                   L.get_rid o <> L.get_rid ol /\ //from app.L.Fsti
+                   eq (merge (do l ol) (do (do a ol) o1) (do (do (do b ob') ol) o2)) 
+                      (do (merge (do l ol) (do a ol) (do (do (do b ob') ol) o2)) o1))
+        (ensures eq (merge (do l ol) (do (do a ol) o1) (do (do (do (do b o) ob') ol) o2)) 
+                    (do (merge (do l ol) (do a ol) (do (do (do (do b o) ob') ol) o2)) o1))          
+let inter_right_2op #sta #stb #oa #ob #m #v l a b o1 o2 ob' ol o =
   let k = get_key o in
   let ka = Alpha_t k in let kb = Beta_t k in
-  if get_key o1 = k && get_key o2 = k && get_key ob = k && get_key ol = k && is_alpha_op o1 && is_alpha_op o2 && is_alpha_op ob && is_alpha_op ol && is_alpha_op o && (Fst_then_snd? (m.rc_a (get_op_a o2) (get_op_a o1)) || Either? (m.rc_a (get_op_a o2) (get_op_a o1))) && Fst_then_snd? (m.rc_a (get_op_a ob) (get_op_a ol)) && (Fst_then_snd? (m.rc_a (get_op_a o) (get_op_a ob)) || Snd_then_fst? (m.rc_a (get_op_a o) (get_op_a ob)) || Fst_then_snd? (m.rc_a (get_op_a o) (get_op_a ol))) then 
-    v.inter_right_2op_a (sel l ka) (sel a ka) (sel b ka) (get_op_a o1) (get_op_a o2) (get_op_a ob) (get_op_a ol) (get_op_a o)
-  else if get_key o1 = k && get_key o2 = k && get_key ob = k && get_key ol = k && is_beta_op o1 && is_beta_op o2 && is_beta_op ob && is_beta_op ol && is_beta_op o && (Fst_then_snd? (m.rc_b (get_op_b o2) (get_op_b o1)) || Either? (m.rc_b (get_op_b o2) (get_op_b o1))) && Fst_then_snd? (m.rc_b (get_op_b ob) (get_op_b ol)) && (Fst_then_snd? (m.rc_b (get_op_b o) (get_op_b ob)) || Snd_then_fst? (m.rc_b (get_op_b o) (get_op_b ob)) || Fst_then_snd? (m.rc_b (get_op_b o) (get_op_b ol))) then
-    v.inter_right_2op_b (sel l kb) (sel a kb) (sel b kb) (get_op_b o1) (get_op_b o2) (get_op_b ob) (get_op_b ol) (get_op_b o)
-  else if Either? (rc #st_a #st_b #o_a #o_b #m o2 o1) then v.inter_right_2op' l a b o1 o2 ob ol o
+  if get_key o1 = k && get_key o2 = k && get_key ob' = k && get_key ol = k && is_alpha_op o1 && is_alpha_op o2 && is_alpha_op ob' && is_alpha_op ol && is_alpha_op o && (L.Fst_then_snd? (m.rca (get_opa o2) (get_opa o1)) || L.Either? (m.rca (get_opa o2) (get_opa o1))) && L.Fst_then_snd? (m.rca (get_opa ob') (get_opa ol)) && (L.Fst_then_snd? (m.rca (get_opa o) (get_opa ob')) || L.Snd_then_fst? (m.rca (get_opa o) (get_opa ob')) || L.Fst_then_snd? (m.rca (get_opa o) (get_opa ol))) then 
+    v.inter_right_2opa (sel l ka) (sel a ka) (sel b ka) (get_opa o1) (get_opa o2) (get_opa ob') (get_opa ol) (get_opa o)
+  else if get_key o1 = k && get_key o2 = k && get_key ob' = k && get_key ol = k && is_beta_op o1 && is_beta_op o2 && is_beta_op ob' && is_beta_op ol && is_beta_op o && (L.Fst_then_snd? (m.rcb (get_opb o2) (get_opb o1)) || L.Either? (m.rcb (get_opb o2) (get_opb o1))) && L.Fst_then_snd? (m.rcb (get_opb ob') (get_opb ol)) && (L.Fst_then_snd? (m.rcb (get_opb o) (get_opb ob')) || L.Snd_then_fst? (m.rcb (get_opb o) (get_opb ob')) || L.Fst_then_snd? (m.rcb (get_opb o) (get_opb ol))) then
+    v.inter_right_2opb (sel l kb) (sel a kb) (sel b kb) (get_opb o1) (get_opb o2) (get_opb ob') (get_opb ol) (get_opb o)
+  else if L.Either? (rc #sta #stb #oa #ob #m o2 o1) then v.inter_right_2op' l a b o1 o2 ob' ol o
   else ()
 
-val inter_left_2op : #st_a:Type0 -> #st_b:Type0 -> #o_a:eqtype -> #o_b:eqtype -> #m:(json st_a st_b o_a o_b) -> #v:(vc st_a st_b o_a o_b m) -> l:st #st_a #st_b #o_a #o_b #m -> a:st -> b:st -> o1:op -> o2:op -> ob:op -> ol:op -> o:op ->
-  Lemma (requires (Fst_then_snd? (rc #st_a #st_b #o_a #o_b #m o2 o1) \/ Either? (rc #st_a #st_b #o_a #o_b #m o2 o1)) /\ get_rid o1 <> get_rid o2 /\ Fst_then_snd? (rc #st_a #st_b #o_a #o_b #m ob ol) /\ get_rid ob <> get_rid ol /\
-                    (~ (Either? (rc #st_a #st_b #o_a #o_b #m o ob)) \/ Fst_then_snd? (rc #st_a #st_b #o_a #o_b #m o ol)) /\               
-                    distinct_ops o1 o2 /\ distinct_ops o1 ob /\ distinct_ops o1 ol /\ distinct_ops o1 o /\ distinct_ops o2 ob /\ distinct_ops o2 ol /\ distinct_ops o2 o /\ distinct_ops ob ol /\ distinct_ops ob o /\ distinct_ops ol o /\
-                    get_rid o <> get_rid ol /\ //from app.fsti
-                    eq (merge (do l ol) (do (do a ol) o1) (do (do (do b ob) ol) o2)) (do (merge (do l ol) (do a ol) (do (do (do b ob) ol) o2)) o1))
-          (ensures eq (merge (do l ol) (do (do (do a o) ol) o1) (do (do (do b ob) ol) o2)) (do (merge (do l ol) (do (do a o) ol) (do (do (do b ob) ol) o2)) o1)) 
-
-let inter_left_2op #st_a #st_b #o_a #o_b #m #v l a b o1 o2 ob ol o =
+val inter_left_2op : #sta:Type0 -> #stb:Type0 -> #oa:eqtype -> #ob:eqtype -> #m:(json sta stb oa ob) -> #v:(vc sta stb oa ob m) -> 
+                     l:st #sta #stb #oa #ob #m -> a:st -> b:st -> o1:jop -> o2:jop -> ob':jop -> ol:jop -> o:jop ->
+  Lemma (requires (L.Fst_then_snd? (rc #sta #stb #oa #ob #m o2 o1) \/ L.Either? (rc #sta #stb #oa #ob #m o2 o1)) /\ 
+                   L.get_rid o1 <> L.get_rid o2 /\ L.Fst_then_snd? (rc #sta #stb #oa #ob #m ob' ol) /\ L.get_rid ob' <> L.get_rid ol /\
+                   (~ (L.Either? (rc #sta #stb #oa #ob #m o ob')) \/ L.Fst_then_snd? (rc #sta #stb #oa #ob #m o ol)) /\               
+                   L.distinct_ops o1 o2 /\ L.distinct_ops o1 ob' /\ L.distinct_ops o1 ol /\ L.distinct_ops o1 o /\ L.distinct_ops o2 ob' /\
+                   L.distinct_ops o2 ol /\ L.distinct_ops o2 o /\ L.distinct_ops ob' ol /\ L.distinct_ops ob' o /\ L.distinct_ops ol o /\
+                   L.get_rid o <> L.get_rid ol /\ //from app.L.Fsti
+                   eq (merge (do l ol) (do (do a ol) o1) (do (do (do b ob') ol) o2)) 
+                      (do (merge (do l ol) (do a ol) (do (do (do b ob') ol) o2)) o1))
+        (ensures eq (merge (do l ol) (do (do (do a o) ol) o1) (do (do (do b ob') ol) o2)) 
+                    (do (merge (do l ol) (do (do a o) ol) (do (do (do b ob') ol) o2)) o1)) 
+let inter_left_2op #sta #stb #oa #ob #m #v l a b o1 o2 ob' ol o =
   let k = get_key o in
   let ka = Alpha_t k in let kb = Beta_t k in
-  if get_key o1 = k && get_key o2 = k && get_key ob = k && get_key ol = k && is_alpha_op o1 && is_alpha_op o2 && is_alpha_op ob && is_alpha_op ol && is_alpha_op o && (Fst_then_snd? (m.rc_a (get_op_a o2) (get_op_a o1)) || Either? (m.rc_a (get_op_a o2) (get_op_a o1))) && Fst_then_snd? (m.rc_a (get_op_a ob) (get_op_a ol)) && (Fst_then_snd? (m.rc_a (get_op_a o) (get_op_a ob)) || Snd_then_fst? (m.rc_a (get_op_a o) (get_op_a ob)) || Fst_then_snd? (m.rc_a (get_op_a o) (get_op_a ol))) then 
-    v.inter_left_2op_a (sel l ka) (sel a ka) (sel b ka) (get_op_a o1) (get_op_a o2) (get_op_a ob) (get_op_a ol) (get_op_a o)
-  else if get_key o1 = k && get_key o2 = k && get_key ob = k && get_key ol = k && is_beta_op o1 && is_beta_op o2 && is_beta_op ob && is_beta_op ol && is_beta_op o && (Fst_then_snd? (m.rc_b (get_op_b o2) (get_op_b o1)) || Either? (m.rc_b (get_op_b o2) (get_op_b o1))) && Fst_then_snd? (m.rc_b (get_op_b ob) (get_op_b ol)) && (Fst_then_snd? (m.rc_b (get_op_b o) (get_op_b ob)) || Snd_then_fst? (m.rc_b (get_op_b o) (get_op_b ob)) || Fst_then_snd? (m.rc_b (get_op_b o) (get_op_b ol))) then
-    v.inter_left_2op_b (sel l kb) (sel a kb) (sel b kb) (get_op_b o1) (get_op_b o2) (get_op_b ob) (get_op_b ol) (get_op_b o)
-  else if Either? (rc #st_a #st_b #o_a #o_b #m o2 o1) then v.inter_left_2op' l a b o1 o2 ob ol o
+  if get_key o1 = k && get_key o2 = k && get_key ob' = k && get_key ol = k && is_alpha_op o1 && is_alpha_op o2 && is_alpha_op ob' && is_alpha_op ol && is_alpha_op o && (L.Fst_then_snd? (m.rca (get_opa o2) (get_opa o1)) || L.Either? (m.rca (get_opa o2) (get_opa o1))) && L.Fst_then_snd? (m.rca (get_opa ob') (get_opa ol)) && (L.Fst_then_snd? (m.rca (get_opa o) (get_opa ob')) || L.Snd_then_fst? (m.rca (get_opa o) (get_opa ob')) || L.Fst_then_snd? (m.rca (get_opa o) (get_opa ol))) then 
+    v.inter_left_2opa (sel l ka) (sel a ka) (sel b ka) (get_opa o1) (get_opa o2) (get_opa ob') (get_opa ol) (get_opa o)
+  else if get_key o1 = k && get_key o2 = k && get_key ob' = k && get_key ol = k && is_beta_op o1 && is_beta_op o2 && is_beta_op ob' && is_beta_op ol && is_beta_op o && (L.Fst_then_snd? (m.rcb (get_opb o2) (get_opb o1)) || L.Either? (m.rcb (get_opb o2) (get_opb o1))) && L.Fst_then_snd? (m.rcb (get_opb ob') (get_opb ol)) && (L.Fst_then_snd? (m.rcb (get_opb o) (get_opb ob')) || L.Snd_then_fst? (m.rcb (get_opb o) (get_opb ob')) || L.Fst_then_snd? (m.rcb (get_opb o) (get_opb ol))) then
+    v.inter_left_2opb (sel l kb) (sel a kb) (sel b kb) (get_opb o1) (get_opb o2) (get_opb ob') (get_opb ol) (get_opb o)
+  else if L.Either? (rc #sta #stb #oa #ob #m o2 o1) then v.inter_left_2op' l a b o1 o2 ob' ol o
   else ()
 
-val ind_right_2op : #st_a:Type0 -> #st_b:Type0 -> #o_a:eqtype -> #o_b:eqtype -> #m:(json st_a st_b o_a o_b) -> #v:(vc st_a st_b o_a o_b m) -> l:st #st_a #st_b #o_a #o_b #m -> a:st #st_a #st_b #o_a #o_b #m -> b:st #st_a #st_b #o_a #o_b #m -> o1:op -> o2:op -> o2':op -> 
-  Lemma (requires Fst_then_snd? (rc #st_a #st_b #o_a #o_b #m o2 o1) /\ get_rid o1 <> get_rid o2 /\
-                    distinct_ops o1 o2 /\ distinct_ops o1 o2' /\ distinct_ops o2 o2' /\
-                    eq (merge l (do a o1) (do b o2)) (do (merge l a (do b o2)) o1))
-          (ensures eq (merge l (do a o1) (do (do b o2') o2)) (do (merge l a (do (do b o2') o2)) o1))
-          
-let ind_right_2op #st_a #st_b #o_a #o_b #m #v l a b o1 o2 o2' =
+val ind_right_2op : #sta:Type0 -> #stb:Type0 -> #oa:eqtype -> #ob:eqtype -> #m:(json sta stb oa ob) -> #v:(vc sta stb oa ob m) -> 
+                    l:st #sta #stb #oa #ob #m -> a:st #sta #stb #oa #ob #m -> b:st #sta #stb #oa #ob #m -> o1:jop -> o2:jop -> o2':jop -> 
+  Lemma (requires L.Fst_then_snd? (rc #sta #stb #oa #ob #m o2 o1) /\ L.get_rid o1 <> L.get_rid o2 /\
+                  L.distinct_ops o1 o2 /\ L.distinct_ops o1 o2' /\ L.distinct_ops o2 o2' /\
+                  eq (merge l (do a o1) (do b o2)) (do (merge l a (do b o2)) o1))
+        (ensures eq (merge l (do a o1) (do (do b o2') o2)) (do (merge l a (do (do b o2') o2)) o1))          
+let ind_right_2op #sta #stb #oa #ob #m #v l a b o1 o2 o2' =
   let k = get_key o2' in
   let ka = Alpha_t k in let kb = Beta_t k in
-  if get_key o1 = k && get_key o2 = k && is_alpha_op o1 && is_alpha_op o2 && is_alpha_op o2' && Fst_then_snd? (m.rc_a (get_op_a o2) (get_op_a o1)) then
-      v.ind_right_2op_a (sel l ka) (sel a ka) (sel b ka) (get_op_a o1) (get_op_a o2) (get_op_a o2')
-  else if get_key o1 = k && get_key o2 = k && is_beta_op o1 && is_beta_op o2 && is_beta_op o2' && Fst_then_snd? (m.rc_b (get_op_b o2) (get_op_b o1)) then
-      v.ind_right_2op_b (sel l kb) (sel a kb) (sel b kb) (get_op_b o1) (get_op_b o2) (get_op_b o2')
+  if get_key o1 = k && get_key o2 = k && is_alpha_op o1 && is_alpha_op o2 && is_alpha_op o2' && L.Fst_then_snd? (m.rca (get_opa o2) (get_opa o1)) then
+      v.ind_right_2opa (sel l ka) (sel a ka) (sel b ka) (get_opa o1) (get_opa o2) (get_opa o2')
+  else if get_key o1 = k && get_key o2 = k && is_beta_op o1 && is_beta_op o2 && is_beta_op o2' && L.Fst_then_snd? (m.rcb (get_opb o2) (get_opb o1)) then
+      v.ind_right_2opb (sel l kb) (sel a kb) (sel b kb) (get_opb o1) (get_opb o2) (get_opb o2')
   else ()
 
-val ind_left_2op : #st_a:Type0 -> #st_b:Type0 -> #o_a:eqtype -> #o_b:eqtype -> #m:(json st_a st_b o_a o_b) -> #v:(vc st_a st_b o_a o_b m) -> l:st #st_a #st_b #o_a #o_b #m -> a:st #st_a #st_b #o_a #o_b #m -> b:st #st_a #st_b #o_a #o_b #m -> o1:op -> o2:op -> o1':op -> 
-  Lemma (requires Fst_then_snd? (rc #st_a #st_b #o_a #o_b #m o2 o1) /\ get_rid o1 <> get_rid o2 /\
-                    distinct_ops o1 o2 /\ distinct_ops o1 o1' /\ distinct_ops o2 o1' /\
-                    eq (merge l (do a o1) (do b o2)) (do (merge l a (do b o2)) o1))
-          (ensures eq (merge l (do (do a o1') o1) (do b o2)) (do (merge l (do a o1') (do b o2)) o1))
-
-let ind_left_2op #st_a #st_b #o_a #o_b #m #v l a b o1 o2 o1' =
+val ind_left_2op : #sta:Type0 -> #stb:Type0 -> #oa:eqtype -> #ob:eqtype -> #m:(json sta stb oa ob) -> #v:(vc sta stb oa ob m) -> 
+                   l:st #sta #stb #oa #ob #m -> a:st #sta #stb #oa #ob #m -> b:st #sta #stb #oa #ob #m -> o1:jop -> o2:jop -> o1':jop -> 
+  Lemma (requires L.Fst_then_snd? (rc #sta #stb #oa #ob #m o2 o1) /\ L.get_rid o1 <> L.get_rid o2 /\
+                  L.distinct_ops o1 o2 /\ L.distinct_ops o1 o1' /\ L.distinct_ops o2 o1' /\
+                  eq (merge l (do a o1) (do b o2)) (do (merge l a (do b o2)) o1))
+        (ensures eq (merge l (do (do a o1') o1) (do b o2)) (do (merge l (do a o1') (do b o2)) o1))
+let ind_left_2op #sta #stb #oa #ob #m #v l a b o1 o2 o1' =
   let k = get_key o1' in
   let ka = Alpha_t k in let kb = Beta_t k in
-  if get_key o1 = k && get_key o2 = k && is_alpha_op o1 && is_alpha_op o2 && is_alpha_op o1' && Fst_then_snd? (m.rc_a (get_op_a o2) (get_op_a o1)) then
-      v.ind_left_2op_a (sel l ka) (sel a ka) (sel b ka) (get_op_a o1) (get_op_a o2) (get_op_a o1')
-  else if get_key o1 = k && get_key o2 = k && is_beta_op o1 && is_beta_op o2 && is_beta_op o1' && Fst_then_snd? (m.rc_b (get_op_b o2) (get_op_b o1)) then
-      v.ind_left_2op_b (sel l kb) (sel a kb) (sel b kb) (get_op_b o1) (get_op_b o2) (get_op_b o1')
+  if get_key o1 = k && get_key o2 = k && is_alpha_op o1 && is_alpha_op o2 && is_alpha_op o1' && L.Fst_then_snd? (m.rca (get_opa o2) (get_opa o1)) then
+      v.ind_left_2opa (sel l ka) (sel a ka) (sel b ka) (get_opa o1) (get_opa o2) (get_opa o1')
+  else if get_key o1 = k && get_key o2 = k && is_beta_op o1 && is_beta_op o2 && is_beta_op o1' && L.Fst_then_snd? (m.rcb (get_opb o2) (get_opb o1)) then
+      v.ind_left_2opb (sel l kb) (sel a kb) (sel b kb) (get_opb o1) (get_opb o2) (get_opb o1')
   else ()
 
-val base_1op : #st_a:Type0 -> #st_b:Type0 -> #o_a:eqtype -> #o_b:eqtype -> #m:(json st_a st_b o_a o_b) -> #v:(vc st_a st_b o_a o_b m) -> o1:op -> t:kt ->
-  Lemma (ensures eq (merge (init_st t) (do (init_st t) o1) (init_st t)) (do #st_a #st_b #o_a #o_b #m (merge (init_st t) (init_st t) (init_st t)) o1))
-
-let base_1op #st_a #st_b #o_a #o_b #m #v o1 t =
-  if is_alpha_op o1 then v.base_1op_a (get_op_a o1)
-  else if is_beta_op o1 then v.base_1op_b (get_op_b o1)
+val base_1op : #sta:Type0 -> #stb:Type0 -> #oa:eqtype -> #ob:eqtype -> #m:(json sta stb oa ob) -> #v:(vc sta stb oa ob m) -> 
+               o1:jop -> t:kt ->
+  Lemma (ensures eq (merge (init_st t) (do (init_st t) o1) (init_st t)) 
+                    (do #sta #stb #oa #ob #m (merge (init_st t) (init_st t) (init_st t)) o1))
+let base_1op #sta #stb #oa #ob #m #v o1 t =
+  if is_alpha_op o1 then v.base_1opa (get_opa o1)
+  else if is_beta_op o1 then v.base_1opb (get_opb o1)
   else ()
 
-val ind_lca_1op : #st_a:Type0 -> #st_b:Type0 -> #o_a:eqtype -> #o_b:eqtype -> #m:(json st_a st_b o_a o_b) -> #v:(vc st_a st_b o_a o_b m) -> l:st -> o1:op -> ol:op ->
-  Lemma (requires distinct_ops o1 ol /\
-                    eq (merge l (do l o1) l) (do (merge l l l) o1))
-          (ensures eq (merge (do l ol) (do (do l ol) o1) (do l ol)) (do #st_a #st_b #o_a #o_b #m (merge (do l ol) (do l ol) (do l ol)) o1))
-
-let ind_lca_1op #st_a #st_b #o_a #o_b #m #v l o1 ol =
+val ind_lca_1op : #sta:Type0 -> #stb:Type0 -> #oa:eqtype -> #ob:eqtype -> #m:(json sta stb oa ob) -> #v:(vc sta stb oa ob m) -> 
+                  l:st -> o1:jop -> ol:jop ->
+  Lemma (requires L.distinct_ops o1 ol /\ eq (merge l (do l o1) l) (do (merge l l l) o1))
+        (ensures eq (merge (do l ol) (do (do l ol) o1) (do l ol)) (do #sta #stb #oa #ob #m (merge (do l ol) (do l ol) (do l ol)) o1))
+let ind_lca_1op #sta #stb #oa #ob #m #v l o1 ol =
   let k = get_key ol in
   let ka = Alpha_t k in let kb = Beta_t k in
   if get_key o1 = k && is_alpha_op o1 && is_alpha_op ol then
-      v.ind_lca_1op_a (sel l ka) (get_op_a o1) (get_op_a ol)
+      v.ind_lca_1opa (sel l ka) (get_opa o1) (get_opa ol)
   else if get_key o1 = k && is_beta_op o1 && is_beta_op ol then
-      v.ind_lca_1op_b (sel l kb) (get_op_b o1) (get_op_b ol)
+      v.ind_lca_1opb (sel l kb) (get_opb o1) (get_opb ol)
   else ()
 
-val inter_right_base_1op : #st_a:Type0 -> #st_b:Type0 -> #o_a:eqtype -> #o_b:eqtype -> #m:(json st_a st_b o_a o_b) -> #v:(vc st_a st_b o_a o_b m) -> l:st #st_a #st_b #o_a #o_b #m -> a:st -> b:st -> o1:op -> ob:op -> ol:op ->
-  Lemma (requires Fst_then_snd? (rc #st_a #st_b #o_a #o_b #m ob ol) /\ get_rid ob <> get_rid ol /\
-                  distinct_ops o1 ob /\ distinct_ops o1 ol /\ distinct_ops ob ol /\
+val inter_right_base_1op : #sta:Type0 -> #stb:Type0 -> #oa:eqtype -> #ob:eqtype -> #m:(json sta stb oa ob) -> #v:(vc sta stb oa ob m) ->
+                           l:st #sta #stb #oa #ob #m -> a:st -> b:st -> o1:jop -> ob':jop -> ol:jop ->
+  Lemma (requires L.Fst_then_snd? (rc #sta #stb #oa #ob #m ob' ol) /\ L.get_rid ob' <> L.get_rid ol /\
+                  L.distinct_ops o1 ob' /\ L.distinct_ops o1 ol /\ L.distinct_ops ob' ol /\
                   eq (merge (do l ol) (do (do a ol) o1) (do b ol)) (do (merge (do l ol) (do a ol) (do b ol)) o1))
-        (ensures eq (merge (do l ol) (do (do a ol) o1) (do (do b ob) ol)) (do (merge (do l ol) (do a ol) (do (do b ob) ol)) o1))
-          
-let inter_right_base_1op #st_a #st_b #o_a #o_b #m #v l a b o1 ob ol =
+        (ensures eq (merge (do l ol) (do (do a ol) o1) (do (do b ob') ol)) (do (merge (do l ol) (do a ol) (do (do b ob') ol)) o1))
+let inter_right_base_1op #sta #stb #oa #ob #m #v l a b o1 ob' ol =
   let k = get_key ol in
   let ka = Alpha_t k in let kb = Beta_t k in
-  if get_key o1 = k && get_key ob = k && is_alpha_op o1 && is_alpha_op ob && is_alpha_op ol && Fst_then_snd? (m.rc_a (get_op_a ob) (get_op_a ol)) then
-      v.inter_right_base_1op_a (sel l ka) (sel a ka) (sel b ka) (get_op_a o1) (get_op_a ob) (get_op_a ol)
-  else if get_key o1 = k && get_key ob = k && is_beta_op o1 && is_beta_op ob && is_beta_op ol && Fst_then_snd? (m.rc_b (get_op_b ob) (get_op_b ol)) then
-      v.inter_right_base_1op_b (sel l kb) (sel a kb) (sel b kb) (get_op_b o1) (get_op_b ob) (get_op_b ol)
+  if get_key o1 = k && get_key ob' = k && is_alpha_op o1 && is_alpha_op ob' && is_alpha_op ol && L.Fst_then_snd? (m.rca (get_opa ob') (get_opa ol)) then
+      v.inter_right_base_1opa (sel l ka) (sel a ka) (sel b ka) (get_opa o1) (get_opa ob') (get_opa ol)
+  else if get_key o1 = k && get_key ob' = k && is_beta_op o1 && is_beta_op ob' && is_beta_op ol && L.Fst_then_snd? (m.rcb (get_opb ob') (get_opb ol)) then
+      v.inter_right_base_1opb (sel l kb) (sel a kb) (sel b kb) (get_opb o1) (get_opb ob') (get_opb ol)
   else ()
 
-val inter_left_base_1op : #st_a:Type0 -> #st_b:Type0 -> #o_a:eqtype -> #o_b:eqtype -> #m:(json st_a st_b o_a o_b) -> #v:(vc st_a st_b o_a o_b m) -> l:st #st_a #st_b #o_a #o_b #m -> a:st -> b:st -> o1:op -> ob:op -> ol:op ->
-  Lemma (requires Fst_then_snd? (rc #st_a #st_b #o_a #o_b #m ob ol) /\ get_rid ob <> get_rid ol /\
-                  distinct_ops o1 ob /\ distinct_ops o1 ol /\ distinct_ops ob ol /\
-                    eq (merge (do l ol) (do (do a ol) o1) (do b ol)) (do (merge (do l ol) (do a ol) (do b ol)) o1))
-          (ensures eq (merge (do l ol) (do (do (do a ob) ol) o1) (do b ol)) (do (merge (do l ol) (do (do a ob) ol) (do b ol)) o1))
-          
-let inter_left_base_1op #st_a #st_b #o_a #o_b #m #v l a b o1 ob ol =
+val inter_left_base_1op : #sta:Type0 -> #stb:Type0 -> #oa:eqtype -> #ob:eqtype -> #m:(json sta stb oa ob) -> #v:(vc sta stb oa ob m) ->
+                          l:st #sta #stb #oa #ob #m -> a:st -> b:st -> o1:jop -> ob':jop -> ol:jop ->
+  Lemma (requires L.Fst_then_snd? (rc #sta #stb #oa #ob #m ob' ol) /\ L.get_rid ob' <> L.get_rid ol /\
+                  L.distinct_ops o1 ob' /\ L.distinct_ops o1 ol /\ L.distinct_ops ob' ol /\
+                  eq (merge (do l ol) (do (do a ol) o1) (do b ol)) (do (merge (do l ol) (do a ol) (do b ol)) o1))
+        (ensures eq (merge (do l ol) (do (do (do a ob') ol) o1) (do b ol)) (do (merge (do l ol) (do (do a ob') ol) (do b ol)) o1))
+let inter_left_base_1op #sta #stb #oa #ob #m #v l a b o1 ob' ol =
   let k = get_key ol in
   let ka = Alpha_t k in let kb = Beta_t k in
-  if get_key o1 = k && get_key ob = k && is_alpha_op o1 && is_alpha_op ob && is_alpha_op ol && Fst_then_snd? (m.rc_a (get_op_a ob) (get_op_a ol)) then
-      v.inter_left_base_1op_a (sel l ka) (sel a ka) (sel b ka) (get_op_a o1) (get_op_a ob) (get_op_a ol)
-  else if get_key o1 = k && get_key ob = k && is_beta_op o1 && is_beta_op ob && is_beta_op ol && Fst_then_snd? (m.rc_b (get_op_b ob) (get_op_b ol)) then
-      v.inter_left_base_1op_b (sel l kb) (sel a kb) (sel b kb) (get_op_b o1) (get_op_b ob) (get_op_b ol)
+  if get_key o1 = k && get_key ob' = k && is_alpha_op o1 && is_alpha_op ob' && is_alpha_op ol && L.Fst_then_snd? (m.rca (get_opa ob') (get_opa ol)) then
+      v.inter_left_base_1opa (sel l ka) (sel a ka) (sel b ka) (get_opa o1) (get_opa ob') (get_opa ol)
+  else if get_key o1 = k && get_key ob' = k && is_beta_op o1 && is_beta_op ob' && is_beta_op ol && L.Fst_then_snd? (m.rcb (get_opb ob') (get_opb ol)) then
+      v.inter_left_base_1opb (sel l kb) (sel a kb) (sel b kb) (get_opb o1) (get_opb ob') (get_opb ol)
   else ()
 
-val inter_right_1op : #st_a:Type0 -> #st_b:Type0 -> #o_a:eqtype -> #o_b:eqtype -> #m:(json st_a st_b o_a o_b) -> #v:(vc st_a st_b o_a o_b m) -> l:st #st_a #st_b #o_a #o_b #m -> a:st -> b:st -> o1:op -> ob:op -> ol:op -> o:op ->
-  Lemma (requires Fst_then_snd? (rc #st_a #st_b #o_a #o_b #m ob ol) /\ get_rid ob <> get_rid ol /\
-                  (~ (Either? (rc #st_a #st_b #o_a #o_b #m o ob)) \/ Fst_then_snd? (rc #st_a #st_b #o_a #o_b #m o ol)) /\
-                  distinct_ops o1 ob /\ distinct_ops o1 ol /\ distinct_ops o1 o /\ distinct_ops ob ol /\ distinct_ops ob o /\ distinct_ops ol o /\
-                  get_rid o <> get_rid ol /\ //from app.fsti
-                  eq (merge (do l ol) (do (do a ol) o1) (do (do b ob) ol)) (do (merge (do l ol) (do a ol) (do (do b ob) ol)) o1))
-        (ensures eq (merge (do l ol) (do (do a ol) o1) (do (do (do b o) ob) ol)) (do (merge (do l ol) (do a ol) (do (do (do b o) ob) ol)) o1))
-
-let inter_right_1op #st_a #st_b #o_a #o_b #m #v l a b o1 ob ol o =
+val inter_right_1op : #sta:Type0 -> #stb:Type0 -> #oa:eqtype -> #ob:eqtype -> #m:(json sta stb oa ob) -> #v:(vc sta stb oa ob m) -> 
+                      l:st #sta #stb #oa #ob #m -> a:st -> b:st -> o1:jop -> ob':jop -> ol:jop -> o:jop ->
+  Lemma (requires L.Fst_then_snd? (rc #sta #stb #oa #ob #m ob' ol) /\ L.get_rid ob' <> L.get_rid ol /\
+                  (~ (L.Either? (rc #sta #stb #oa #ob #m o ob')) \/ L.Fst_then_snd? (rc #sta #stb #oa #ob #m o ol)) /\
+                  L.distinct_ops o1 ob' /\ L.distinct_ops o1 ol /\ L.distinct_ops o1 o /\ 
+                  L.distinct_ops ob' ol /\ L.distinct_ops ob' o /\ L.distinct_ops ol o /\
+                  L.get_rid o <> L.get_rid ol /\ //from app.L.Fsti
+                  eq (merge (do l ol) (do (do a ol) o1) (do (do b ob') ol)) (do (merge (do l ol) (do a ol) (do (do b ob') ol)) o1))
+        (ensures eq (merge (do l ol) (do (do a ol) o1) (do (do (do b o) ob') ol)) 
+                    (do (merge (do l ol) (do a ol) (do (do (do b o) ob') ol)) o1))
+let inter_right_1op #sta #stb #oa #ob #m #v l a b o1 ob' ol o =
   let k = get_key o in
   let ka = Alpha_t k in let kb = Beta_t k in
-  if get_key o1 = k && get_key ob = k && get_key ol = k && is_alpha_op o1 && is_alpha_op ob && is_alpha_op ol && is_alpha_op o && Fst_then_snd? (m.rc_a (get_op_a ob) (get_op_a ol)) && (Fst_then_snd? (m.rc_a (get_op_a o) (get_op_a ob)) || Snd_then_fst? (m.rc_a (get_op_a o) (get_op_a ob)) || Fst_then_snd? (m.rc_a (get_op_a o) (get_op_a ol))) then 
-    v.inter_right_1op_a (sel l ka) (sel a ka) (sel b ka) (get_op_a o1) (get_op_a ob) (get_op_a ol) (get_op_a o)
-  else if get_key o1 = k && get_key ob = k && get_key ol = k && is_beta_op o1 && is_beta_op ob && is_beta_op ol && is_beta_op o && Fst_then_snd? (m.rc_b (get_op_b ob) (get_op_b ol)) && (Fst_then_snd? (m.rc_b (get_op_b o) (get_op_b ob)) || Snd_then_fst? (m.rc_b (get_op_b o) (get_op_b ob)) || Fst_then_snd? (m.rc_b (get_op_b o) (get_op_b ol))) then
-    v.inter_right_1op_b (sel l kb) (sel a kb) (sel b kb) (get_op_b o1) (get_op_b ob) (get_op_b ol) (get_op_b o)
+  if get_key o1 = k && get_key ob' = k && get_key ol = k && is_alpha_op o1 && is_alpha_op ob' && is_alpha_op ol && is_alpha_op o && L.Fst_then_snd? (m.rca (get_opa ob') (get_opa ol)) && (L.Fst_then_snd? (m.rca (get_opa o) (get_opa ob')) || L.Snd_then_fst? (m.rca (get_opa o) (get_opa ob')) || L.Fst_then_snd? (m.rca (get_opa o) (get_opa ol))) then 
+    v.inter_right_1opa (sel l ka) (sel a ka) (sel b ka) (get_opa o1) (get_opa ob') (get_opa ol) (get_opa o)
+  else if get_key o1 = k && get_key ob' = k && get_key ol = k && is_beta_op o1 && is_beta_op ob' && is_beta_op ol && is_beta_op o && L.Fst_then_snd? (m.rcb (get_opb ob') (get_opb ol)) && (L.Fst_then_snd? (m.rcb (get_opb o) (get_opb ob')) || L.Snd_then_fst? (m.rcb (get_opb o) (get_opb ob')) || L.Fst_then_snd? (m.rcb (get_opb o) (get_opb ol))) then
+    v.inter_right_1opb (sel l kb) (sel a kb) (sel b kb) (get_opb o1) (get_opb ob') (get_opb ol) (get_opb o)
   else ()
 
-val inter_left_1op : #st_a:Type0 -> #st_b:Type0 -> #o_a:eqtype -> #o_b:eqtype -> #m:(json st_a st_b o_a o_b) -> #v:(vc st_a st_b o_a o_b m) -> l:st #st_a #st_b #o_a #o_b #m -> a:st -> b:st -> o1:op -> ob:op -> ol:op -> o:op ->
-  Lemma (requires Fst_then_snd? (rc #st_a #st_b #o_a #o_b #m ob ol) /\ get_rid ob <> get_rid ol /\
-                  (~ (Either? (rc #st_a #st_b #o_a #o_b #m o ob)) \/ Fst_then_snd? (rc #st_a #st_b #o_a #o_b #m o ol)) /\               
-                  distinct_ops o1 ob /\ distinct_ops o1 ol /\ distinct_ops o1 o /\ distinct_ops ob ol /\ distinct_ops ob o /\ distinct_ops ol o /\
-                  get_rid o <> get_rid ol /\ //from app.fsti
-                  eq (merge (do l ol) (do (do (do a ob) ol) o1) (do b ol)) (do (merge (do l ol) (do (do a ob) ol) (do b ol)) o1))
-        (ensures eq (merge (do l ol) (do (do (do (do a o) ob) ol) o1) (do b ol)) (do (merge (do l ol) (do (do (do a o) ob) ol) (do b ol)) o1))
-
-let inter_left_1op #st_a #st_b #o_a #o_b #m #v l a b o1 ob ol o =
+val inter_left_1op : #sta:Type0 -> #stb:Type0 -> #oa:eqtype -> #ob:eqtype -> #m:(json sta stb oa ob) -> #v:(vc sta stb oa ob m) -> 
+                     l:st #sta #stb #oa #ob #m -> a:st -> b:st -> o1:jop -> ob':jop -> ol:jop -> o:jop ->
+  Lemma (requires L.Fst_then_snd? (rc #sta #stb #oa #ob #m ob' ol) /\ L.get_rid ob' <> L.get_rid ol /\
+                  (~ (L.Either? (rc #sta #stb #oa #ob #m o ob')) \/ L.Fst_then_snd? (rc #sta #stb #oa #ob #m o ol)) /\               
+                  L.distinct_ops o1 ob' /\ L.distinct_ops o1 ol /\ L.distinct_ops o1 o /\ 
+                  L.distinct_ops ob' ol /\ L.distinct_ops ob' o /\ L.distinct_ops ol o /\
+                  L.get_rid o <> L.get_rid ol /\ //from app.L.Fsti
+                  eq (merge (do l ol) (do (do (do a ob') ol) o1) (do b ol)) (do (merge (do l ol) (do (do a ob') ol) (do b ol)) o1))
+        (ensures eq (merge (do l ol) (do (do (do (do a o) ob') ol) o1) (do b ol)) 
+                 (do (merge (do l ol) (do (do (do a o) ob') ol) (do b ol)) o1))
+let inter_left_1op #sta #stb #oa #ob #m #v l a b o1 ob' ol o =
   let k = get_key o in
   let ka = Alpha_t k in let kb = Beta_t k in
-  if get_key o1 = k && get_key ob = k && get_key ol = k && is_alpha_op o1 && is_alpha_op ob && is_alpha_op ol && is_alpha_op o && Fst_then_snd? (m.rc_a (get_op_a ob) (get_op_a ol)) && (Fst_then_snd? (m.rc_a (get_op_a o) (get_op_a ob)) || Snd_then_fst? (m.rc_a (get_op_a o) (get_op_a ob)) || Fst_then_snd? (m.rc_a (get_op_a o) (get_op_a ol))) then 
-    v.inter_left_1op_a (sel l ka) (sel a ka) (sel b ka) (get_op_a o1) (get_op_a ob) (get_op_a ol) (get_op_a o)
-  else if get_key o1 = k && get_key ob = k && get_key ol = k && is_beta_op o1 && is_beta_op ob && is_beta_op ol && is_beta_op o && Fst_then_snd? (m.rc_b (get_op_b ob) (get_op_b ol)) && (Fst_then_snd? (m.rc_b (get_op_b o) (get_op_b ob)) || Snd_then_fst? (m.rc_b (get_op_b o) (get_op_b ob)) || Fst_then_snd? (m.rc_b (get_op_b o) (get_op_b ol))) then
-    v.inter_left_1op_b (sel l kb) (sel a kb) (sel b kb) (get_op_b o1) (get_op_b ob) (get_op_b ol) (get_op_b o)
+  if get_key o1 = k && get_key ob' = k && get_key ol = k && is_alpha_op o1 && is_alpha_op ob' && is_alpha_op ol && is_alpha_op o && L.Fst_then_snd? (m.rca (get_opa ob') (get_opa ol)) && (L.Fst_then_snd? (m.rca (get_opa o) (get_opa ob')) || L.Snd_then_fst? (m.rca (get_opa o) (get_opa ob')) || L.Fst_then_snd? (m.rca (get_opa o) (get_opa ol))) then 
+    v.inter_left_1opa (sel l ka) (sel a ka) (sel b ka) (get_opa o1) (get_opa ob') (get_opa ol) (get_opa o)
+  else if get_key o1 = k && get_key ob' = k && get_key ol = k && is_beta_op o1 && is_beta_op ob' && is_beta_op ol && is_beta_op o && L.Fst_then_snd? (m.rcb (get_opb ob') (get_opb ol)) && (L.Fst_then_snd? (m.rcb (get_opb o) (get_opb ob')) || L.Snd_then_fst? (m.rcb (get_opb o) (get_opb ob')) || L.Fst_then_snd? (m.rcb (get_opb o) (get_opb ol))) then
+    v.inter_left_1opb (sel l kb) (sel a kb) (sel b kb) (get_opb o1) (get_opb ob') (get_opb ol) (get_opb o)
   else ()
 
-val ind_right_1op : #st_a:Type0 -> #st_b:Type0 -> #o_a:eqtype -> #o_b:eqtype -> #m:(json st_a st_b o_a o_b) -> #v:(vc st_a st_b o_a o_b m) -> l:st #st_a #st_b #o_a #o_b #m -> a:st -> b:st -> o2:op -> o2':op -> ol:op ->
-  Lemma (requires distinct_ops o2 o2' /\ distinct_ops o2 ol /\ distinct_ops o2' ol /\
+val ind_right_1op : #sta:Type0 -> #stb:Type0 -> #oa:eqtype -> #ob:eqtype -> #m:(json sta stb oa ob) -> #v:(vc sta stb oa ob m) -> 
+                    l:st #sta #stb #oa #ob #m -> a:st -> b:st -> o2:jop -> o2':jop -> ol:jop ->
+  Lemma (requires L.distinct_ops o2 o2' /\ L.distinct_ops o2 ol /\ L.distinct_ops o2' ol /\
                   eq (merge (do l ol) (do a ol) (do b o2)) (do (merge (do l ol) (do a ol) b) o2))
         (ensures eq (merge (do l ol) (do a ol) (do (do b o2') o2)) (do (merge (do l ol) (do a ol) (do b o2')) o2))
-
-let ind_right_1op #st_a #st_b #o_a #o_b #m #v l a b o2 o2' ol =
+let ind_right_1op #sta #stb #oa #ob #m #v l a b o2 o2' ol =
   let k = get_key ol in
   let ka = Alpha_t k in let kb = Beta_t k in
   if get_key o2 = k && get_key o2' = k && is_alpha_op o2 && is_alpha_op o2' && is_alpha_op ol then
-      v.ind_right_1op_a (sel l ka) (sel a ka) (sel b ka) (get_op_a o2) (get_op_a o2') (get_op_a ol)
+      v.ind_right_1opa (sel l ka) (sel a ka) (sel b ka) (get_opa o2) (get_opa o2') (get_opa ol)
   else if get_key o2 = k && get_key o2' = k && is_beta_op o2 && is_beta_op o2' && is_beta_op ol then
-      v.ind_right_1op_b (sel l kb) (sel a kb) (sel b kb) (get_op_b o2) (get_op_b o2') (get_op_b ol)
+      v.ind_right_1opb (sel l kb) (sel a kb) (sel b kb) (get_opb o2) (get_opb o2') (get_opb ol)
   else v.ind_right_1op' l a b o2 o2' ol
 
-val ind_left_1op : #st_a:Type0 -> #st_b:Type0 -> #o_a:eqtype -> #o_b:eqtype -> #m:(json st_a st_b o_a o_b) -> #v:(vc st_a st_b o_a o_b m) -> l:st #st_a #st_b #o_a #o_b #m -> a:st -> b:st -> o1:op -> o1':op -> ol:op ->
-  Lemma (requires distinct_ops o1 o1' /\ distinct_ops o1 ol /\ distinct_ops o1' ol /\
+val ind_left_1op : #sta:Type0 -> #stb:Type0 -> #oa:eqtype -> #ob:eqtype -> #m:(json sta stb oa ob) -> #v:(vc sta stb oa ob m) -> 
+                   l:st #sta #stb #oa #ob #m -> a:st -> b:st -> o1:jop -> o1':jop -> ol:jop ->
+  Lemma (requires L.distinct_ops o1 o1' /\ L.distinct_ops o1 ol /\ L.distinct_ops o1' ol /\
                   eq (merge (do l ol) (do a o1) (do b ol)) (do (merge (do l ol) a (do b ol)) o1))
         (ensures eq (merge (do l ol) (do (do a o1') o1) (do b ol)) (do (merge (do l ol) (do a o1') (do b ol)) o1)) 
-
-let ind_left_1op #st_a #st_b #o_a #o_b #m #v l a b o1 o1' ol =
+let ind_left_1op #sta #stb #oa #ob #m #v l a b o1 o1' ol =
   let k = get_key ol in
   let ka = Alpha_t k in let kb = Beta_t k in
   if get_key o1 = k && get_key o1' = k && is_alpha_op o1 && is_alpha_op o1' && is_alpha_op ol then
-      v.ind_left_1op_a (sel l ka) (sel a ka) (sel b ka) (get_op_a o1) (get_op_a o1') (get_op_a ol)
+      v.ind_left_1opa (sel l ka) (sel a ka) (sel b ka) (get_opa o1) (get_opa o1') (get_opa ol)
   else if get_key o1 = k && get_key o1' = k && is_beta_op o1 && is_beta_op o1' && is_beta_op ol then
-      v.ind_left_1op_b (sel l kb) (sel a kb) (sel b kb) (get_op_b o1) (get_op_b o1') (get_op_b ol)
+      v.ind_left_1opb (sel l kb) (sel a kb) (sel b kb) (get_opb o1) (get_opb o1') (get_opb ol)
   else v.ind_left_1op' l a b o1 o1' ol
 
-val lem_0op : #st_a:Type0 -> #st_b:Type0 -> #o_a:eqtype -> #o_b:eqtype -> #m:(json st_a st_b o_a o_b) -> #v:(vc st_a st_b o_a o_b m) -> l:st #st_a #st_b #o_a #o_b #m -> a:st -> b:st -> ol:op ->
+val lem_0op : #sta:Type0 -> #stb:Type0 -> #oa:eqtype -> #ob:eqtype -> #m:(json sta stb oa ob) -> #v:(vc sta stb oa ob m) -> 
+              l:st #sta #stb #oa #ob #m -> a:st -> b:st -> ol:jop ->
   Lemma (ensures eq (merge (do l ol) (do a ol) (do b ol)) (do (merge l a b) ol))
-
-let lem_0op #st_a #st_b #o_a #o_b #m #v l a b ol =
+let lem_0op #sta #stb #oa #ob #m #v l a b ol =
   let k = get_key ol in
   let ka = Alpha_t k in let kb = Beta_t k in
-  if is_alpha_op ol then v.lem_0op_a (sel l ka) (sel a ka) (sel b ka) (get_op_a ol)
-  else if is_beta_op ol then v.lem_0op_b (sel l kb) (sel a kb) (sel b kb) (get_op_b ol)
+  if is_alpha_op ol then v.lem_0opa (sel l ka) (sel a ka) (sel b ka) (get_opa ol)
+  else if is_beta_op ol then v.lem_0opb (sel l kb) (sel a kb) (sel b kb) (get_opb ol)
   else ()
+
