typeclass/Gset.fst
@@ -49,7 +49,7 @@ let ind_left_1op l a b o1 o1' ol = ()
 let ind_right_1op l a b o2 o2' ol = ()
 let lem_0op l a b ol = ()
 
-instance ictr : mrdt st app_op = {
+instance gset : mrdt st app_op = {
   Library.init_st;
   Library.eq;
   Library.rc;
@@ -58,14 +58,14 @@ instance ictr : mrdt st app_op = {
 }
 
 #set-options "--ifuel 3"
-instance ictr_cond : cond st app_op ictr = {
+instance gset_cond : cond st app_op gset = {
   Library.rc_non_comm;
   Library.no_rc_chain;
   Library.cond_comm_base;
   Library.cond_comm_ind
 }
 
-instance ictr_proof : vc st app_op ictr = {
+instance gset_proof : vc st app_op gset = {
   Library.merge_comm;
   Library.merge_idem;
   Library.base_2op;
