typeclass/Library.fst
@@ -2,11 +2,7 @@ module Library
 
 open FStar.Seq
 
-//type op = pos (*timestamp*) & (nat (*replica ID*) & eqtype)
-
 let get_rid (_,(rid,_)) = rid
-
-type log = seq (pos & (nat & eqtype))
 
 //conflict resolution type
 type rc_res =
@@ -67,106 +63,75 @@ class vc (st:Type0) (app_op:eqtype) (m:mrdt st app_op) = {
 
   base_2op : o1:op -> o2:op ->
     Lemma (requires (Fst_then_snd? (m.rc o2 o1) \/ Either? (m.rc o2 o1)) /\ get_rid o1 <> get_rid o2 /\ distinct_ops o1 o2)
-          (ensures m.eq (m.merge m.init_st (m.do m.init_st o1) (m.do m.init_st o2)) (m.do (m.merge m.init_st m.init_st (m.do m.init_st o2)) o1));
+          (ensures m.eq (m.merge m.init_st (m.do m.init_st o1) (m.do m.init_st o2)) 
+                        (m.do (m.merge m.init_st m.init_st (m.do m.init_st o2)) o1));
 
   ind_lca_2op : l:st -> o1:op -> o2:op -> ol:op ->
   Lemma (requires (Fst_then_snd? (m.rc o2 o1) \/ Either? (m.rc o2 o1)) /\
-                  get_rid o1 <> get_rid o2 /\
-                  distinct_ops o1 o2 /\
-                  distinct_ops o1 ol /\
-                  distinct_ops o2 ol /\
+                  get_rid o1 <> get_rid o2 /\ distinct_ops o1 o2 /\ distinct_ops o1 ol /\ distinct_ops o2 ol /\
                   m.eq (m.merge l (m.do l o1) (m.do l o2)) (m.do (m.merge l l (m.do l o2)) o1))
-        (ensures m.eq (m.merge (m.do l ol) (m.do (m.do l ol) o1) (m.do (m.do l ol) o2)) (m.do (m.merge (m.do l ol) (m.do l ol) (m.do (m.do l ol) o2)) o1));
+        (ensures m.eq (m.merge (m.do l ol) (m.do (m.do l ol) o1) (m.do (m.do l ol) o2)) 
+                      (m.do (m.merge (m.do l ol) (m.do l ol) (m.do (m.do l ol) o2)) o1));
 
   inter_right_base_2op : l:st -> a:st -> b:st -> o1:op -> o2:op -> ob:op -> ol:op ->
-  Lemma (requires (Fst_then_snd? (m.rc o2 o1) \/ Either? (m.rc o2 o1)) /\
-                  get_rid o1 <> get_rid o2 /\
-                  Fst_then_snd? (m.rc ob ol) /\
-                  get_rid ob <> get_rid ol /\
-                  distinct_ops o1 o2 /\
-                  distinct_ops o1 ob /\
-                  distinct_ops o1 ol /\
-                  distinct_ops o2 ob /\
-                  distinct_ops o2 ol /\
-                  distinct_ops ob ol /\
+  Lemma (requires (Fst_then_snd? (m.rc o2 o1) \/ Either? (m.rc o2 o1)) /\ Fst_then_snd? (m.rc ob ol) /\
+                  get_rid o1 <> get_rid o2 /\ get_rid ob <> get_rid ol /\ 
+                  distinct_ops o1 o2 /\ distinct_ops o1 ob /\ distinct_ops o1 ol /\
+                  distinct_ops o2 ob /\ distinct_ops o2 ol /\ distinct_ops ob ol /\
                   m.eq (m.merge l (m.do a o1) (m.do b o2)) (m.do (m.merge l a (m.do b o2)) o1) /\
                   m.eq (m.merge l (m.do a o1) (m.do (m.do b ob) o2)) (m.do (m.merge l a (m.do (m.do b ob) o2)) o1) /\
-                  m.eq (m.merge (m.do l ol) (m.do (m.do a ol) o1) (m.do (m.do b ol) o2)) (m.do (m.merge (m.do l ol) (m.do a ol) (m.do (m.do b ol) o2)) o1))
-        (ensures m.eq (m.merge (m.do l ol) (m.do (m.do a ol) o1) (m.do (m.do (m.do b ob) ol) o2)) (m.do (m.merge (m.do l ol) (m.do a ol) (m.do (m.do (m.do b ob) ol) o2)) o1));
+                  m.eq (m.merge (m.do l ol) (m.do (m.do a ol) o1) (m.do (m.do b ol) o2)) 
+                       (m.do (m.merge (m.do l ol) (m.do a ol) (m.do (m.do b ol) o2)) o1))
+        (ensures m.eq (m.merge (m.do l ol) (m.do (m.do a ol) o1) (m.do (m.do (m.do b ob) ol) o2)) 
+                      (m.do (m.merge (m.do l ol) (m.do a ol) (m.do (m.do (m.do b ob) ol) o2)) o1));
 
 inter_left_base_2op : l:st -> a:st -> b:st -> o1:op -> o2:op -> ob:op -> ol:op ->
-  Lemma (requires Fst_then_snd? (m.rc o2 o1) /\
-                  Fst_then_snd? (m.rc ob ol) /\
-                  get_rid o2 <> get_rid o1 /\
-                  get_rid ob <> get_rid ol /\
-                  distinct_ops o1 o2 /\
-                  distinct_ops o1 ob /\
-                  distinct_ops o1 ol /\
-                  distinct_ops o2 ob /\
-                  distinct_ops o2 ol /\
-                  distinct_ops ob ol /\
-                  m.eq (m.merge (m.do l ol) (m.do (m.do a ol) o1) (m.do (m.do b ol) o2)) (m.do (m.merge (m.do l ol) (m.do a ol) (m.do (m.do b ol) o2)) o1))
-        (ensures m.eq (m.merge (m.do l ol) (m.do (m.do (m.do a ob) ol) o1) (m.do (m.do b ol) o2)) (m.do (m.merge (m.do l ol) (m.do (m.do a ob) ol) (m.do (m.do b ol) o2)) o1));
+  Lemma (requires Fst_then_snd? (m.rc o2 o1) /\ Fst_then_snd? (m.rc ob ol) /\
+                  get_rid o2 <> get_rid o1 /\ get_rid ob <> get_rid ol /\
+                  distinct_ops o1 o2 /\ distinct_ops o1 ob /\ distinct_ops o1 ol /\
+                  distinct_ops o2 ob /\ distinct_ops o2 ol /\ distinct_ops ob ol /\
+                  m.eq (m.merge (m.do l ol) (m.do (m.do a ol) o1) (m.do (m.do b ol) o2)) 
+                       (m.do (m.merge (m.do l ol) (m.do a ol) (m.do (m.do b ol) o2)) o1))
+        (ensures m.eq (m.merge (m.do l ol) (m.do (m.do (m.do a ob) ol) o1) (m.do (m.do b ol) o2)) 
+                      (m.do (m.merge (m.do l ol) (m.do (m.do a ob) ol) (m.do (m.do b ol) o2)) o1));
 
 inter_right_2op : l:st -> a:st -> b:st -> o1:op -> o2:op -> ob:op -> ol:op -> o:op ->
-  Lemma (requires (Fst_then_snd? (m.rc o2 o1) \/ Either? (m.rc o2 o1)) /\
-                  get_rid o1 <> get_rid o2 /\
-                  Fst_then_snd? (m.rc ob ol) /\
-                  get_rid ob <> get_rid ol /\
+  Lemma (requires (Fst_then_snd? (m.rc o2 o1) \/ Either? (m.rc o2 o1)) /\ Fst_then_snd? (m.rc ob ol) /\
+                  get_rid o1 <> get_rid o2 /\ get_rid ob <> get_rid ol /\
                   (~ (Either? (m.rc o ob)) \/ Fst_then_snd? (m.rc o ol)) /\
-                  distinct_ops o1 o2 /\
-                  distinct_ops o1 ob /\
-                  distinct_ops o1 ol /\
-                  distinct_ops o1 o /\
-                  distinct_ops o2 ob /\
-                  distinct_ops o2 ol /\
-                  distinct_ops o2 o /\
-                  distinct_ops ob ol /\
-                  distinct_ops ob o /\
-                  distinct_ops ol o /\
+                  distinct_ops o1 o2 /\ distinct_ops o1 ob /\ distinct_ops o1 ol /\ distinct_ops o1 o /\ distinct_ops o2 ob /\ 
+                  distinct_ops o2 ol /\ distinct_ops o2 o /\ distinct_ops ob ol /\ distinct_ops ob o /\ distinct_ops ol o /\
                   get_rid o <> get_rid ol /\
-                  m.eq (m.merge (m.do l ol) (m.do (m.do a ol) o1) (m.do (m.do (m.do b ob) ol) o2)) (m.do (m.merge (m.do l ol) (m.do a ol) (m.do (m.do (m.do b ob) ol) o2)) o1))
-        (ensures m.eq (m.merge (m.do l ol) (m.do (m.do a ol) o1) (m.do (m.do (m.do (m.do b o) ob) ol) o2)) (m.do (m.merge (m.do l ol) (m.do a ol) (m.do (m.do (m.do (m.do b o) ob) ol) o2)) o1));
+                  m.eq (m.merge (m.do l ol) (m.do (m.do a ol) o1) (m.do (m.do (m.do b ob) ol) o2)) 
+                       (m.do (m.merge (m.do l ol) (m.do a ol) (m.do (m.do (m.do b ob) ol) o2)) o1))
+        (ensures m.eq (m.merge (m.do l ol) (m.do (m.do a ol) o1) (m.do (m.do (m.do (m.do b o) ob) ol) o2)) 
+                      (m.do (m.merge (m.do l ol) (m.do a ol) (m.do (m.do (m.do (m.do b o) ob) ol) o2)) o1));
 
 inter_left_2op : l:st -> a:st -> b:st -> o1:op -> o2:op -> ob:op -> ol:op -> o:op ->
-  Lemma (requires Fst_then_snd? (m.rc o2 o1) /\
-                  Fst_then_snd? (m.rc ob ol) /\
-                  get_rid o2 <> get_rid o1 /\
-                  get_rid ob <> get_rid ol /\
+  Lemma (requires Fst_then_snd? (m.rc o2 o1) /\ Fst_then_snd? (m.rc ob ol) /\
+                  get_rid o2 <> get_rid o1 /\ get_rid ob <> get_rid ol /\
                   (~ (Either? (m.rc o ob)) \/ Fst_then_snd? (m.rc o ol)) /\
-                  distinct_ops o1 o2 /\
-                  distinct_ops o1 ob /\
-                  distinct_ops o1 ol /\
-                  distinct_ops o1 o /\
-                  distinct_ops o2 ob /\
-                  distinct_ops o2 ol /\
-                  distinct_ops o2 o /\
-                  distinct_ops ob ol /\
-                  distinct_ops ob o /\
-                  distinct_ops ol o /\
+                  distinct_ops o1 o2 /\ distinct_ops o1 ob /\ distinct_ops o1 ol /\ distinct_ops o1 o /\ distinct_ops o2 ob /\ 
+                  distinct_ops o2 ol /\ distinct_ops o2 o /\ distinct_ops ob ol /\ distinct_ops ob o /\ distinct_ops ol o /\
                   get_rid o <> get_rid ol /\
-                  m.eq (m.merge (m.do l ol) (m.do (m.do a ol) o1) (m.do (m.do (m.do b ob) ol) o2)) (m.do (m.merge (m.do l ol) (m.do a ol) (m.do (m.do (m.do b ob) ol) o2)) o1))
-        (ensures m.eq (m.merge (m.do l ol) (m.do (m.do (m.do a o) ol) o1) (m.do (m.do (m.do b ob) ol) o2)) (m.do (m.merge (m.do l ol) (m.do (m.do a o) ol) (m.do (m.do (m.do b ob) ol) o2)) o1));
+                  m.eq (m.merge (m.do l ol) (m.do (m.do a ol) o1) (m.do (m.do (m.do b ob) ol) o2)) 
+                       (m.do (m.merge (m.do l ol) (m.do a ol) (m.do (m.do (m.do b ob) ol) o2)) o1))
+        (ensures m.eq (m.merge (m.do l ol) (m.do (m.do (m.do a o) ol) o1) (m.do (m.do (m.do b ob) ol) o2)) 
+                      (m.do (m.merge (m.do l ol) (m.do (m.do a o) ol) (m.do (m.do (m.do b ob) ol) o2)) o1));
 
 ind_right_2op : l:st -> a:st -> b:st -> o1:op -> o2:op -> o2':op ->
   Lemma (requires Fst_then_snd? (m.rc o2 o1) /\
-                  get_rid o1 <> get_rid o2 /\
-                  distinct_ops o1 o2 /\
-                  distinct_ops o1 o2' /\
-                  distinct_ops o2 o2' /\
+                  get_rid o1 <> get_rid o2 /\ distinct_ops o1 o2 /\ distinct_ops o1 o2' /\ distinct_ops o2 o2' /\
                   m.eq (m.merge l (m.do a o1) (m.do b o2)) (m.do (m.merge l a (m.do b o2)) o1))
         (ensures m.eq (m.merge l (m.do a o1) (m.do (m.do b o2') o2)) (m.do (m.merge l a (m.do (m.do b o2') o2)) o1));
 
 ind_left_2op : l:st -> a:st -> b:st -> o1:op -> o2:op -> o1':op ->
   Lemma (requires (Fst_then_snd? (m.rc o2 o1) \/ Either? (m.rc o2 o1)) /\
-                  get_rid o1 <> get_rid o2 /\
-                  distinct_ops o1 o2 /\
-                  distinct_ops o1 o1' /\
-                  distinct_ops o2 o1' /\
+                  get_rid o1 <> get_rid o2 /\ distinct_ops o1 o2 /\ distinct_ops o1 o1' /\ distinct_ops o2 o1' /\
                   m.eq (m.merge l (m.do a o1) (m.do b o2)) (m.do (m.merge l a (m.do b o2)) o1))
         (ensures m.eq (m.merge l (m.do (m.do a o1') o1) (m.do b o2)) (m.do (m.merge l (m.do a o1') (m.do b o2)) o1));
 
-  base_1op : o1:op ->
+base_1op : o1:op ->
   Lemma (ensures m.eq (m.merge m.init_st (m.do m.init_st o1) m.init_st) (m.do (m.merge m.init_st m.init_st m.init_st) o1));
 
 ind_lca_1op : l:st -> o1:op -> ol:op ->
@@ -176,42 +141,48 @@ ind_lca_1op : l:st -> o1:op -> ol:op ->
 
 inter_right_base_1op : l:st -> a:st -> b:st -> o1:op -> ob:op -> ol:op ->
   Lemma (requires Fst_then_snd? (m.rc ob ol) /\ get_rid ob <> get_rid ol /\
-                    distinct_ops o1 ob /\ distinct_ops o1 ol /\ distinct_ops ob ol /\
-                    (Fst_then_snd? (m.rc ob o1) ==> m.eq (m.merge l (m.do a o1) (m.do b ob)) (m.do (m.merge l a (m.do b ob)) o1)) /\
-                    m.eq (m.merge (m.do l ol) (m.do (m.do a ol) o1) (m.do b ol)) (m.do (m.merge (m.do l ol) (m.do a ol) (m.do b ol)) o1))
-          (ensures m.eq (m.merge (m.do l ol) (m.do (m.do a ol) o1) (m.do (m.do b ob) ol)) (m.do (m.merge (m.do l ol) (m.do a ol) (m.do (m.do b ob) ol)) o1));
+                  distinct_ops o1 ob /\ distinct_ops o1 ol /\ distinct_ops ob ol /\
+                  (Fst_then_snd? (m.rc ob o1) ==> m.eq (m.merge l (m.do a o1) (m.do b ob)) (m.do (m.merge l a (m.do b ob)) o1)) /\
+                  m.eq (m.merge (m.do l ol) (m.do (m.do a ol) o1) (m.do b ol)) (m.do (m.merge (m.do l ol) (m.do a ol) (m.do b ol)) o1))
+        (ensures m.eq (m.merge (m.do l ol) (m.do (m.do a ol) o1) (m.do (m.do b ob) ol)) 
+                      (m.do (m.merge (m.do l ol) (m.do a ol) (m.do (m.do b ob) ol)) o1));
 
 inter_left_base_1op : l:st -> a:st -> b:st -> o1:op -> ob:op -> ol:op ->
   Lemma (requires Fst_then_snd? (m.rc ob ol) /\ get_rid ob <> get_rid ol /\
-                    distinct_ops o1 ob /\ distinct_ops o1 ol /\ distinct_ops ob ol /\
-                    m.eq (m.merge (m.do l ol) (m.do (m.do a ol) o1) (m.do b ol)) (m.do (m.merge (m.do l ol) (m.do a ol) (m.do b ol)) o1))
-          (ensures m.eq (m.merge (m.do l ol) (m.do (m.do (m.do a ob) ol) o1) (m.do b ol)) (m.do (m.merge (m.do l ol) (m.do (m.do a ob) ol) (m.do b ol)) o1));
+                  distinct_ops o1 ob /\ distinct_ops o1 ol /\ distinct_ops ob ol /\
+                  m.eq (m.merge (m.do l ol) (m.do (m.do a ol) o1) (m.do b ol)) (m.do (m.merge (m.do l ol) (m.do a ol) (m.do b ol)) o1))
+        (ensures m.eq (m.merge (m.do l ol) (m.do (m.do (m.do a ob) ol) o1) (m.do b ol)) 
+                      (m.do (m.merge (m.do l ol) (m.do (m.do a ob) ol) (m.do b ol)) o1));
           
 inter_right_1op : l:st -> a:st -> b:st -> o1:op -> ob:op -> ol:op -> o:op ->
   Lemma (requires Fst_then_snd? (m.rc ob ol) /\ get_rid ob <> get_rid ol /\
-                    (~ (Either? (m.rc o ob)) \/ Fst_then_snd? (m.rc o ol)) /\
-                    distinct_ops o1 ob /\ distinct_ops o1 ol /\ distinct_ops o1 o /\ distinct_ops ob ol /\ distinct_ops ob o /\ distinct_ops ol o /\
-                    get_rid o <> get_rid ol /\
-                    m.eq (m.merge (m.do l ol) (m.do (m.do a ol) o1) (m.do (m.do b ob) ol)) (m.do (m.merge (m.do l ol) (m.do a ol) (m.do (m.do b ob) ol)) o1))
-          (ensures m.eq (m.merge (m.do l ol) (m.do (m.do a ol) o1) (m.do (m.do (m.do b o) ob) ol)) (m.do (m.merge (m.do l ol) (m.do a ol) (m.do (m.do (m.do b o) ob) ol)) o1));
+                  (~ (Either? (m.rc o ob)) \/ Fst_then_snd? (m.rc o ol)) /\
+                  distinct_ops o1 ob /\ distinct_ops o1 ol /\ distinct_ops o1 o /\ distinct_ops ob ol /\ distinct_ops ob o /\ distinct_ops ol o /\
+                  get_rid o <> get_rid ol /\
+                  m.eq (m.merge (m.do l ol) (m.do (m.do a ol) o1) (m.do (m.do b ob) ol)) 
+                       (m.do (m.merge (m.do l ol) (m.do a ol) (m.do (m.do b ob) ol)) o1))
+        (ensures m.eq (m.merge (m.do l ol) (m.do (m.do a ol) o1) (m.do (m.do (m.do b o) ob) ol)) 
+                      (m.do (m.merge (m.do l ol) (m.do a ol) (m.do (m.do (m.do b o) ob) ol)) o1));
 
 inter_left_1op : l:st -> a:st -> b:st -> o1:op -> ob:op -> ol:op -> o:op ->
   Lemma (requires Fst_then_snd? (m.rc ob ol) /\ get_rid ob <> get_rid ol /\
-                    (~ (Either? (m.rc o ob)) \/ Fst_then_snd? (m.rc o ol)) /\
-                    distinct_ops o1 ob /\ distinct_ops o1 ol /\ distinct_ops o1 o /\ distinct_ops ob ol /\ distinct_ops ob o /\ distinct_ops ol o /\
-                    get_rid o <> get_rid ol /\
-                    m.eq (m.merge (m.do l ol) (m.do (m.do (m.do a ob) ol) o1) (m.do b ol)) (m.do (m.merge (m.do l ol) (m.do (m.do a ob) ol) (m.do b ol)) o1))
-          (ensures m.eq (m.merge (m.do l ol) (m.do (m.do (m.do (m.do a o) ob) ol) o1) (m.do b ol)) (m.do (m.merge (m.do l ol) (m.do (m.do (m.do a o) ob) ol) (m.do b ol)) o1));
+                  (~ (Either? (m.rc o ob)) \/ Fst_then_snd? (m.rc o ol)) /\
+                  distinct_ops o1 ob /\ distinct_ops o1 ol /\ distinct_ops o1 o /\ distinct_ops ob ol /\ distinct_ops ob o /\ distinct_ops ol o /\
+                  get_rid o <> get_rid ol /\
+                  m.eq (m.merge (m.do l ol) (m.do (m.do (m.do a ob) ol) o1) (m.do b ol)) 
+                       (m.do (m.merge (m.do l ol) (m.do (m.do a ob) ol) (m.do b ol)) o1))
+        (ensures m.eq (m.merge (m.do l ol) (m.do (m.do (m.do (m.do a o) ob) ol) o1) (m.do b ol)) 
+                      (m.do (m.merge (m.do l ol) (m.do (m.do (m.do a o) ob) ol) (m.do b ol)) o1));
 
 ind_left_1op : l:st -> a:st -> b:st -> o1:op -> o1':op -> ol:op ->
   Lemma (requires distinct_ops o1 o1' /\ distinct_ops o1 ol /\ distinct_ops o1' ol /\
-                    m.eq (m.merge (m.do l ol) (m.do a o1) (m.do b ol)) (m.do (m.merge (m.do l ol) a (m.do b ol)) o1))
-          (ensures m.eq (m.merge (m.do l ol) (m.do (m.do a o1') o1) (m.do b ol)) (m.do (m.merge (m.do l ol) (m.do a o1') (m.do b ol)) o1));
+                  m.eq (m.merge (m.do l ol) (m.do a o1) (m.do b ol)) (m.do (m.merge (m.do l ol) a (m.do b ol)) o1))
+        (ensures m.eq (m.merge (m.do l ol) (m.do (m.do a o1') o1) (m.do b ol)) (m.do (m.merge (m.do l ol) (m.do a o1') (m.do b ol)) o1));
 
 ind_right_1op : l:st -> a:st -> b:st -> o2:op -> o2':op -> ol:op ->
   Lemma (requires distinct_ops o2 o2' /\ distinct_ops o2 ol /\ distinct_ops o2' ol /\
-                    m.eq (m.merge (m.do l ol) (m.do a ol) (m.do b o2)) (m.do (m.merge (m.do l ol) (m.do a ol) b) o2))
-          (ensures m.eq (m.merge (m.do l ol) (m.do a ol) (m.do (m.do b o2') o2)) (m.do (m.merge (m.do l ol) (m.do a ol) (m.do b o2')) o2));
+                  m.eq (m.merge (m.do l ol) (m.do a ol) (m.do b o2)) (m.do (m.merge (m.do l ol) (m.do a ol) b) o2))
+        (ensures m.eq (m.merge (m.do l ol) (m.do a ol) (m.do (m.do b o2') o2)) (m.do (m.merge (m.do l ol) (m.do a ol) (m.do b o2')) o2));
 
 lem_0op : l:st -> a:st -> b:st -> ol:op ->
   Lemma (ensures m.eq (m.merge (m.do l ol) (m.do a ol) (m.do b ol)) (m.do (m.merge l a b) ol))
